@prefix : <https://semanticdatacharter.com/ontology/sdc4-meta/> .
@prefix owl: <http://www.w3.org/2002/07/owl#> .
@prefix rdf: <http://www.w3.org/1999/02/22-rdf-syntax-ns#> .
@prefix xml: <http://www.w3.org/XML/1998/namespace> .
@prefix xsd: <http://www.w3.org/2001/XMLSchema#> .
@prefix rdfs: <http://www.w3.org/2000/01/rdf-schema#> .
@prefix sdc4: <https://semanticdatacharter.com/ns/sdc4/> .
@prefix sdc4-meta: <https://semanticdatacharter.com/ontology/sdc4-meta/> .
@base <https://semanticdatacharter.com/ontology/sdc4-meta/> .

<https://semanticdatacharter.com/ontology/sdc4-meta/> rdf:type owl:Ontology ;
                                                           rdfs:comment """
            This ontology describes the meta-level concepts and relationships of the
            Semantic Data Charter (SDC) Reference Model, defining how XML Schema
            structures map to conceptual entities and their metadata.
        """@en ;
                                                           rdfs:label "Semantic Data Charter Reference Model Meta-Ontology"@en ;
                                                           owl:versionInfo "1.0" .

#################################################################
#    Datatypes
#################################################################

###  sdc4:BooleanListSimpleType
<sdc4:BooleanListSimpleType> rdf:type rdfs:Datatype ;
                             rdfs:comment "A simple type for a white space-delimited list of boolean values."@en ;
                             rdfs:label "BooleanListSimpleType"@en .


###  sdc4:DecimalListSimpleType
<sdc4:DecimalListSimpleType> rdf:type rdfs:Datatype ;
                             rdfs:comment "A simple type for a white space-delimited list of decimal values."@en ;
                             rdfs:label "DecimalListSimpleType"@en .


###  sdc4:DoubleListSimpleType
<sdc4:DoubleListSimpleType> rdf:type rdfs:Datatype ;
                            rdfs:comment "A simple type for a white space-delimited list of double precision values."@en ;
                            rdfs:label "DoubleListSimpleType"@en .


###  sdc4:IntegerListSimpleType
<sdc4:IntegerListSimpleType> rdf:type rdfs:Datatype ;
                             rdfs:comment "A simple type for a white space-delimited list of integer values."@en ;
                             rdfs:label "IntegerListSimpleType"@en .


###  sdc4:NonNegativeIntegerListSimpleType
<sdc4:NonNegativeIntegerListSimpleType> rdf:type rdfs:Datatype ;
                                        rdfs:comment "A simple type for a white space-delimited list of non-negative integer values."@en ;
                                        rdfs:label "NonNegativeIntegerListSimpleType"@en .


###  sdc4:PositiveIntegerListSimpleType
<sdc4:PositiveIntegerListSimpleType> rdf:type rdfs:Datatype ;
                                     rdfs:comment "A simple type for a white space-delimited list of positive integer values."@en ;
                                     rdfs:label "PositiveIntegerListSimpleType"@en .


###  sdc4:StringListSimpleType
<sdc4:StringListSimpleType> rdf:type rdfs:Datatype ;
                            rdfs:comment "A simple type for a white space-delimited list of string values."@en ;
                            rdfs:label "StringListSimpleType"@en .


###  sdc4:TokenListSimpleType
<sdc4:TokenListSimpleType> rdf:type rdfs:Datatype ;
                           rdfs:comment "A simple type for a white space-delimited list of normalized token values."@en ;
                           rdfs:label "TokenListSimpleType"@en .


#################################################################
#    Object Properties
#################################################################

###  https://semanticdatacharter.com/ontology/sdc4-meta/definesComponent
sdc4-meta:definesComponent rdf:type owl:ObjectProperty ;
                           rdfs:domain sdc4-meta:ReferenceModel ;
                           rdfs:range sdc4-meta:ReferenceModelComponent ;
                           rdfs:comment "Links an SDC Reference Model to its defined Reference Model Components."@en ;
                           rdfs:label "defines component"@en .


###  https://semanticdatacharter.com/ontology/sdc4-meta/describesConceptualAspect
sdc4-meta:describesConceptualAspect rdf:type owl:ObjectProperty ;
                                    rdfs:domain sdc4-meta:ReferenceModelElement ;
                                    rdfs:range sdc4-meta:ConceptualAspect ;
                                    rdfs:comment """
            States that a specific Reference Model Element describes a particular Conceptual Aspect
            of the Conceptual Entity it is associated with.
        """@en ;
                                    rdfs:label "describes conceptual aspect"@en .


###  https://semanticdatacharter.com/ontology/sdc4-meta/hasConceptualLabelValue
sdc4-meta:hasConceptualLabelValue rdf:type owl:ObjectProperty ;
                                  rdfs:domain sdc4-meta:ConceptualEntity .


###  https://semanticdatacharter.com/ontology/sdc4-meta/hasDescriptiveElement
sdc4-meta:hasDescriptiveElement rdf:type owl:ObjectProperty ;
                                rdfs:domain sdc4-meta:ReferenceModelComponent ;
                                rdfs:range sdc4-meta:ReferenceModelElement ;
                                rdfs:comment """
            Links a Reference Model Component to its sub-elements that provide descriptive information.
        """@en ;
                                rdfs:label "has descriptive element"@en .


###  https://semanticdatacharter.com/ontology/sdc4-meta/isComposedOf
sdc4-meta:isComposedOf rdf:type owl:ObjectProperty ;
                       rdfs:domain sdc4-meta:DataModel ;
                       rdfs:range sdc4-meta:ModelComponent ;
                       rdfs:comment "Links a Data Model to its constituent Model Components."@en ;
                       rdfs:label "is composed of"@en .


###  https://semanticdatacharter.com/ontology/sdc4-meta/isConceptualEntityFor
sdc4-meta:isConceptualEntityFor rdf:type owl:ObjectProperty ;
                                rdfs:domain sdc4-meta:ConceptualEntity ;
                                rdfs:range sdc4-meta:ReferenceModelComponent ;
                                rdfs:comment """
            States that a Conceptual Entity (e.g., 'City') is conceptually identified or
            represented by a specific Reference Model Component (e.g., XdStringType when
            its 'label' element is fixed to 'City').
        """@en ;
                                rdfs:label "is conceptual entity for"@en .


###  https://semanticdatacharter.com/ontology/sdc4-meta/isConstrainedByRmComponent
sdc4-meta:isConstrainedByRmComponent rdf:type owl:ObjectProperty ;
                                     rdfs:domain sdc4-meta:ModelComponent ;
                                     rdfs:range sdc4-meta:ReferenceModelComponent ;
                                     rdfs:comment """
            Links a Model Component (from a specific Data Model) to the Reference Model Component
            from which it is derived or by which it is constrained (e.g., via xsd:extension or xsd:restriction).
        """@en ;
                                     rdfs:label "is constrained by RM component"@en .


###  sdc4:xddecimallist-units
<sdc4:xddecimallist-units> rdf:type owl:ObjectProperty ;
                           rdfs:comment "The name or type of the decimal list values. Examples are \"kg\", \"mmHg\", \"ms-1\", \"km/h\". Should come from a standard terminology. All values in the list share these units."@en ;
                           rdfs:label "xddecimallist-units"@en .


###  sdc4:xddoublelist-units
<sdc4:xddoublelist-units> rdf:type owl:ObjectProperty ;
                          rdfs:comment "The name or type of the double list values. Examples are \"kg\", \"mmHg\", \"ms-1\", \"km/h\". Should come from a standard terminology. All values in the list share these units."@en ;
                          rdfs:label "xddoublelist-units"@en .


###  sdc4:xdintegerlist-units
<sdc4:xdintegerlist-units> rdf:type owl:ObjectProperty ;
                           rdfs:comment "The name or type of the integer list values. Examples are \"items\", \"counts\", \"indices\". Should come from a standard terminology. All values in the list share these units."@en ;
                           rdfs:label "xdintegerlist-units"@en .


###  sdc4:xdnonnegativeintegerlist-units
<sdc4:xdnonnegativeintegerlist-units> rdf:type owl:ObjectProperty ;
                                      rdfs:comment "The name or type of the non-negative integer list values. Examples are \"items\", \"counts\", \"indices\". Should come from a standard terminology. All values in the list share these units."@en ;
                                      rdfs:label "xdnonnegativeintegerlist-units"@en .


###  sdc4:xdpositiveintegerlist-units
<sdc4:xdpositiveintegerlist-units> rdf:type owl:ObjectProperty ;
                                   rdfs:comment "The name or type of the positive integer list values. Examples are \"items\", \"counts\", \"indices\". Should come from a standard terminology. All values in the list share these units."@en ;
                                   rdfs:label "xdpositiveintegerlist-units"@en .


#################################################################
#    Data properties
#################################################################

###  https://semanticdatacharter.com/ontology/sdc4-meta/hasConceptualLabelValue
sdc4-meta:hasConceptualLabelValue rdf:type owl:DatatypeProperty .


###  sdc4:xdbooleanlist-value
<sdc4:xdbooleanlist-value> rdf:type owl:DatatypeProperty .


###  sdc4:xddecimallist-value
<sdc4:xddecimallist-value> rdf:type owl:DatatypeProperty .


###  sdc4:xddoublelist-value
<sdc4:xddoublelist-value> rdf:type owl:DatatypeProperty .


###  sdc4:xdintegerlist-value
<sdc4:xdintegerlist-value> rdf:type owl:DatatypeProperty .


###  sdc4:xdnonnegativeintegerlist-value
<sdc4:xdnonnegativeintegerlist-value> rdf:type owl:DatatypeProperty .


###  sdc4:xdpositiveintegerlist-value
<sdc4:xdpositiveintegerlist-value> rdf:type owl:DatatypeProperty .


###  sdc4:xdstringlist-value
<sdc4:xdstringlist-value> rdf:type owl:DatatypeProperty .


###  sdc4:xdtokenlist-value
<sdc4:xdtokenlist-value> rdf:type owl:DatatypeProperty .


#################################################################
#    Classes
#################################################################

###  https://semanticdatacharter.com/ontology/sdc4-meta/ConceptualAspect
sdc4-meta:ConceptualAspect rdf:type owl:Class ;
                           rdfs:comment """
            Represents an abstract characteristic or metadata type that can be associated
            with a Conceptual Entity. (e.g., 'Valid Time Beginning', 'Conceptual Value').
        """@en ;
                           rdfs:label "Conceptual Aspect"@en .


###  https://semanticdatacharter.com/ontology/sdc4-meta/ConceptualEntity
sdc4-meta:ConceptualEntity rdf:type owl:Class ;
                           rdfs:comment """
            This is the meta-level concept representing \"the thing\" that a 'label' element
            describes in an SDC Data Model, regardless of its underlying XML Schema type.
            It's the abstract idea of a \"City,\" \"Person,\" \"Measurement,\" etc., as identified
            by the 'label'.
        """@en ;
                           rdfs:label "Conceptual Entity"@en .


###  https://semanticdatacharter.com/ontology/sdc4-meta/DataModel
sdc4-meta:DataModel rdf:type owl:Class ;
                    rdfs:comment """
            Represents a specific \"Data Model (DM)\" built according to the SDC Reference Model.
            This is the conceptual representation of what DMType in the XML Schema signifies
            at the schema level (not the data instance level).
        """@en ;
                    rdfs:label "Data Model"@en .


###  https://semanticdatacharter.com/ontology/sdc4-meta/ModelComponent
sdc4-meta:ModelComponent rdf:type owl:Class ;
                         rdfs:comment """
            Represents a generic concept of a \"Model Component (MC)\" as described in the SDC
            documentation. These are the reusable building blocks within a Data Model.
            (e.g., XdAnyType, ClusterType, XdAdapterType, and their concrete subtypes).
        """@en ;
                         rdfs:label "Model Component"@en .


###  https://semanticdatacharter.com/ontology/sdc4-meta/ReferenceModel
sdc4-meta:ReferenceModel rdf:type owl:Class ;
                         rdfs:comment """
            Represents the overarching conceptual framework defined by an XML Schema
            like sdc4.xsd itself. It is the blueprint for building concrete data models.
        """@en ;
                         rdfs:label "Reference Model"@en .


###  https://semanticdatacharter.com/ontology/sdc4-meta/ReferenceModelComponent
sdc4-meta:ReferenceModelComponent rdf:type owl:Class ;
                                  rdfs:subClassOf sdc4-meta:ModelComponent ;
                                  rdfs:comment """
            Represents the specific \"core datatypes and structures\" defined within the
            sdc4.xsd file (e.g., XdAnyType, XdStringType, XdLinkType) that act as the
            foundational building blocks for Data Models. These are instances of this class.
        """@en ;
                                  rdfs:label "Reference Model Component"@en .


###  https://semanticdatacharter.com/ontology/sdc4-meta/ReferenceModelElement
sdc4-meta:ReferenceModelElement rdf:type owl:Class ;
                                rdfs:comment """
            Represents a specific XML element defined within a Reference Model Component
            (e.g., 'vtb', 'xdstring-value', 'label'). These are instances of this class.
        """@en ;
                                rdfs:label "Reference Model Element"@en .


###  sdc4:ASKRType
<sdc4:ASKRType> rdf:type owl:Class ;
                rdfs:subClassOf <sdc4:ExceptionalValueType> .


###  sdc4:ASKUType
<sdc4:ASKUType> rdf:type owl:Class ;
                rdfs:subClassOf <sdc4:ExceptionalValueType> .


###  sdc4:ClusterType
<sdc4:ClusterType> rdf:type owl:Class ;
                   rdfs:subClassOf <sdc4:ItemType> .


###  sdc4:DERType
<sdc4:DERType> rdf:type owl:Class ;
               rdfs:subClassOf <sdc4:ExceptionalValueType> .


###  sdc4:ExceptionalValueType
<sdc4:ExceptionalValueType> rdf:type owl:Class .


###  sdc4:INVType
<sdc4:INVType> rdf:type owl:Class ;
               rdfs:subClassOf <sdc4:ExceptionalValueType> .


###  sdc4:ItemType
<sdc4:ItemType> rdf:type owl:Class .


###  sdc4:MSKType
<sdc4:MSKType> rdf:type owl:Class ;
               rdfs:subClassOf <sdc4:ExceptionalValueType> .


###  sdc4:NASKType
<sdc4:NASKType> rdf:type owl:Class ;
                rdfs:subClassOf <sdc4:ExceptionalValueType> .


###  sdc4:NAType
<sdc4:NAType> rdf:type owl:Class ;
              rdfs:subClassOf <sdc4:ExceptionalValueType> .


###  sdc4:NAVType
<sdc4:NAVType> rdf:type owl:Class ;
               rdfs:subClassOf <sdc4:ExceptionalValueType> .


###  sdc4:NINFType
<sdc4:NINFType> rdf:type owl:Class ;
                rdfs:subClassOf <sdc4:ExceptionalValueType> .


###  sdc4:NIType
<sdc4:NIType> rdf:type owl:Class ;
              rdfs:subClassOf <sdc4:ExceptionalValueType> .


###  sdc4:OTHType
<sdc4:OTHType> rdf:type owl:Class ;
               rdfs:subClassOf <sdc4:ExceptionalValueType> .


###  sdc4:PINFType
<sdc4:PINFType> rdf:type owl:Class ;
                rdfs:subClassOf <sdc4:ExceptionalValueType> .


###  sdc4:QSType
<sdc4:QSType> rdf:type owl:Class ;
              rdfs:subClassOf <sdc4:ExceptionalValueType> .


###  sdc4:ReferenceRangeType
<sdc4:ReferenceRangeType> rdf:type owl:Class ;
                          rdfs:subClassOf <sdc4:XdAnyType> .


###  sdc4:TRCType
<sdc4:TRCType> rdf:type owl:Class ;
               rdfs:subClassOf <sdc4:ExceptionalValueType> .


###  sdc4:UNCType
<sdc4:UNCType> rdf:type owl:Class ;
               rdfs:subClassOf <sdc4:ExceptionalValueType> .


###  sdc4:UNKType
<sdc4:UNKType> rdf:type owl:Class ;
               rdfs:subClassOf <sdc4:ExceptionalValueType> .


###  sdc4:XdAdapterType
<sdc4:XdAdapterType> rdf:type owl:Class ;
                     rdfs:subClassOf <sdc4:ItemType> .


###  sdc4:XdAnyType
<sdc4:XdAnyType> rdf:type owl:Class .


###  sdc4:XdBooleanListType
<sdc4:XdBooleanListType> rdf:type owl:Class ;
                         rdfs:subClassOf <sdc4:XdAnyType> .


###  sdc4:XdBooleanType
<sdc4:XdBooleanType> rdf:type owl:Class ;
                     rdfs:subClassOf <sdc4:XdAnyType> .


###  sdc4:XdCountType
<sdc4:XdCountType> rdf:type owl:Class ;
                   rdfs:subClassOf <sdc4:XdQuantifiedType> .


###  sdc4:XdDecimalListType
<sdc4:XdDecimalListType> rdf:type owl:Class ;
                         rdfs:subClassOf <sdc4:XdQuantifiedType> .


###  sdc4:XdDoubleListType
<sdc4:XdDoubleListType> rdf:type owl:Class ;
                        rdfs:subClassOf <sdc4:XdQuantifiedType> .


###  sdc4:XdDoubleType
<sdc4:XdDoubleType> rdf:type owl:Class ;
                    rdfs:subClassOf <sdc4:XdQuantifiedType> .


###  sdc4:XdFileType
<sdc4:XdFileType> rdf:type owl:Class ;
                  rdfs:subClassOf <sdc4:XdAnyType> .


###  sdc4:XdFloatType
<sdc4:XdFloatType> rdf:type owl:Class ;
                   rdfs:subClassOf <sdc4:XdQuantifiedType> .


###  sdc4:XdIntegerListType
<sdc4:XdIntegerListType> rdf:type owl:Class ;
                         rdfs:subClassOf <sdc4:XdQuantifiedType> .


###  sdc4:XdIntervalType
<sdc4:XdIntervalType> rdf:type owl:Class ;
                      rdfs:subClassOf <sdc4:XdAnyType> .


###  sdc4:XdLinkType
<sdc4:XdLinkType> rdf:type owl:Class ;
                  rdfs:subClassOf <sdc4:XdAnyType> .


###  sdc4:XdNonNegativeIntegerListType
<sdc4:XdNonNegativeIntegerListType> rdf:type owl:Class ;
                                    rdfs:subClassOf <sdc4:XdQuantifiedType> .


###  sdc4:XdOrderedType
<sdc4:XdOrderedType> rdf:type owl:Class ;
                     rdfs:subClassOf <sdc4:XdAnyType> .


###  sdc4:XdOrdinalType
<sdc4:XdOrdinalType> rdf:type owl:Class ;
                     rdfs:subClassOf <sdc4:XdOrderedType> .


###  sdc4:XdPositiveIntegerListType
<sdc4:XdPositiveIntegerListType> rdf:type owl:Class ;
                                 rdfs:subClassOf <sdc4:XdQuantifiedType> .


###  sdc4:XdQuantifiedType
<sdc4:XdQuantifiedType> rdf:type owl:Class ;
                        rdfs:subClassOf <sdc4:XdOrderedType> .


###  sdc4:XdQuantityType
<sdc4:XdQuantityType> rdf:type owl:Class ;
                      rdfs:subClassOf <sdc4:XdQuantifiedType> .


###  sdc4:XdStringListType
<sdc4:XdStringListType> rdf:type owl:Class ;
                        rdfs:subClassOf <sdc4:XdAnyType> .


###  sdc4:XdStringType
<sdc4:XdStringType> rdf:type owl:Class ;
                    rdfs:subClassOf <sdc4:XdAnyType> .


###  sdc4:XdTemporalType
<sdc4:XdTemporalType> rdf:type owl:Class ;
                      rdfs:subClassOf <sdc4:XdOrderedType> .


###  sdc4:XdTokenListType
<sdc4:XdTokenListType> rdf:type owl:Class ;
                       rdfs:subClassOf <sdc4:XdAnyType> .


#################################################################
#    Individuals
#################################################################

###  https://semanticdatacharter.com/ns/sdc4/sdc4.xsd
sdc4:sdc4.xsd rdf:type owl:NamedIndividual ,
                       sdc4-meta:ReferenceModel ;
              sdc4-meta:definesComponent <sdc4:ASKRType> ,
                                         <sdc4:ASKUType> ,
                                         <sdc4:AttestationType> ,
                                         <sdc4:AuditType> ,
                                         <sdc4:ClusterType> ,
                                         <sdc4:DERType> ,
                                         <sdc4:DMType> ,
                                         <sdc4:ExceptionalValueType> ,
                                         <sdc4:INVType> ,
                                         <sdc4:InvlType> ,
                                         <sdc4:InvlUnits> ,
                                         <sdc4:ItemType> ,
                                         <sdc4:MSKType> ,
                                         <sdc4:MagnitudeStatus> ,
                                         <sdc4:NASKType> ,
                                         <sdc4:NAType> ,
                                         <sdc4:NAVType> ,
                                         <sdc4:NINFType> ,
                                         <sdc4:NIType> ,
                                         <sdc4:OTHType> ,
                                         <sdc4:PINFType> ,
                                         <sdc4:ParticipationType> ,
                                         <sdc4:PartyType> ,
                                         <sdc4:QSType> ,
                                         <sdc4:ReferenceRangeType> ,
                                         <sdc4:TRCType> ,
                                         <sdc4:UNCType> ,
                                         <sdc4:UNKType> ,
                                         <sdc4:XdAdapterType> ,
                                         <sdc4:XdAnyType> ,
                                         <sdc4:XdBooleanListType> ,
                                         <sdc4:XdBooleanType> ,
                                         <sdc4:XdCountType> ,
                                         <sdc4:XdDecimalListType> ,
                                         <sdc4:XdDoubleListType> ,
                                         <sdc4:XdDoubleType> ,
                                         <sdc4:XdFileType> ,
                                         <sdc4:XdFloatType> ,
                                         <sdc4:XdIntegerListType> ,
                                         <sdc4:XdIntervalType> ,
                                         <sdc4:XdLinkType> ,
                                         <sdc4:XdNonNegativeIntegerListType> ,
                                         <sdc4:XdOrderedType> ,
                                         <sdc4:XdOrdinalType> ,
                                         <sdc4:XdPositiveIntegerListType> ,
                                         <sdc4:XdQuantifiedType> ,
                                         <sdc4:XdQuantityType> ,
                                         <sdc4:XdStringListType> ,
                                         <sdc4:XdStringType> ,
                                         <sdc4:XdTemporalType> ,
                                         <sdc4:XdTokenListType> ;
              rdfs:comment """
            This is the concrete instance of the SDC Reference Model, represented by the sdc4.xsd file.
        """@en ;
              rdfs:label "Semantic Data Charter Release 4 Reference Model XML Schema"@en .


###  https://semanticdatacharter.com/ontology/sdc4-meta/AccessControlSystem
sdc4-meta:AccessControlSystem rdf:type owl:NamedIndividual ,
                                       sdc4-meta:ConceptualAspect ;
                              rdfs:comment "Represents the identifier of an external access control system."@en ;
                              rdfs:label "Access Control System"@en .


###  https://semanticdatacharter.com/ontology/sdc4-meta/AccessControlTag
sdc4-meta:AccessControlTag rdf:type owl:NamedIndividual ,
                                    sdc4-meta:ConceptualAspect ;
                           rdfs:comment "Represents the access control tag aspect of a conceptual entity."@en ;
                           rdfs:label "Access Control Tag"@en .


###  https://semanticdatacharter.com/ontology/sdc4-meta/AccuracyMargin
sdc4-meta:AccuracyMargin rdf:type owl:NamedIndividual ,
                                  sdc4-meta:ConceptualAspect ;
                         rdfs:comment "Represents the margin of systematic error for a measurement."@en ;
                         rdfs:label "Accuracy Margin"@en .


###  https://semanticdatacharter.com/ontology/sdc4-meta/AdaptedValue
sdc4-meta:AdaptedValue rdf:type owl:NamedIndividual ,
                                sdc4-meta:ConceptualAspect ;
                       rdfs:comment "Represents the data value type attached to an XdAdapterType."@en ;
                       rdfs:label "Adapted Value"@en .


###  https://semanticdatacharter.com/ontology/sdc4-meta/AttestationCommittedTimestamp
sdc4-meta:AttestationCommittedTimestamp rdf:type owl:NamedIndividual ,
                                                 sdc4-meta:ConceptualAspect ;
                                        rdfs:comment "Represents the timestamp of committal of the attested item."@en ;
                                        rdfs:label "Attestation Committed Timestamp"@en .


###  https://semanticdatacharter.com/ontology/sdc4-meta/AttestationCommitter
sdc4-meta:AttestationCommitter rdf:type owl:NamedIndividual ,
                                        sdc4-meta:ConceptualAspect ;
                               rdfs:comment "Represents the identity of the person who committed the attested item."@en ;
                               rdfs:label "Attestation Committer"@en .


###  https://semanticdatacharter.com/ontology/sdc4-meta/AttestationLabel
sdc4-meta:AttestationLabel rdf:type owl:NamedIndividual ,
                                    sdc4-meta:ConceptualAspect ;
                           rdfs:comment "Represents the descriptive label for an attestation."@en ;
                           rdfs:label "Attestation Label"@en .


###  https://semanticdatacharter.com/ontology/sdc4-meta/AttestationPendingStatus
sdc4-meta:AttestationPendingStatus rdf:type owl:NamedIndividual ,
                                            sdc4-meta:ConceptualAspect ;
                                   rdfs:comment "Represents whether an attestation is outstanding or completed."@en ;
                                   rdfs:label "Attestation Pending Status"@en .


###  https://semanticdatacharter.com/ontology/sdc4-meta/AttestationProof
sdc4-meta:AttestationProof rdf:type owl:NamedIndividual ,
                                    sdc4-meta:ConceptualAspect ;
                           rdfs:comment "Represents the proof of attestation (e.g., signature)."@en ;
                           rdfs:label "Attestation Proof"@en .


###  https://semanticdatacharter.com/ontology/sdc4-meta/AttestationReason
sdc4-meta:AttestationReason rdf:type owl:NamedIndividual ,
                                     sdc4-meta:ConceptualAspect ;
                            rdfs:comment "Represents the reason for an attestation."@en ;
                            rdfs:label "Attestation Reason"@en .


###  https://semanticdatacharter.com/ontology/sdc4-meta/AttestationView
sdc4-meta:AttestationView rdf:type owl:NamedIndividual ,
                                   sdc4-meta:ConceptualAspect ;
                          rdfs:comment "Represents the visual representation of attested content."@en ;
                          rdfs:label "Attestation View"@en .


###  https://semanticdatacharter.com/ontology/sdc4-meta/AuditLabel
sdc4-meta:AuditLabel rdf:type owl:NamedIndividual ,
                              sdc4-meta:ConceptualAspect ;
                     rdfs:comment "Represents the descriptive label for an audit record."@en ;
                     rdfs:label "Audit Label"@en .


###  https://semanticdatacharter.com/ontology/sdc4-meta/AuditLocation
sdc4-meta:AuditLocation rdf:type owl:NamedIndividual ,
                                 sdc4-meta:ConceptualAspect ;
                        rdfs:comment "Represents the location of an audit event."@en ;
                        rdfs:label "Audit Location"@en .


###  https://semanticdatacharter.com/ontology/sdc4-meta/AuditTimestamp
sdc4-meta:AuditTimestamp rdf:type owl:NamedIndividual ,
                                  sdc4-meta:ConceptualAspect ;
                         rdfs:comment "Represents the timestamp of an audit event."@en ;
                         rdfs:label "Audit Timestamp"@en .


###  https://semanticdatacharter.com/ontology/sdc4-meta/BooleanFalseValue
sdc4-meta:BooleanFalseValue rdf:type owl:NamedIndividual ,
                                     sdc4-meta:ConceptualAspect ;
                            rdfs:comment "Represents the false value aspect for a boolean conceptual entity."@en ;
                            rdfs:label "Boolean False Value"@en .


###  https://semanticdatacharter.com/ontology/sdc4-meta/BooleanTrueValue
sdc4-meta:BooleanTrueValue rdf:type owl:NamedIndividual ,
                                    sdc4-meta:ConceptualAspect ;
                           rdfs:comment "Represents the true value aspect for a boolean conceptual entity."@en ;
                           rdfs:label "Boolean True Value"@en .


###  https://semanticdatacharter.com/ontology/sdc4-meta/ClusterLabel
sdc4-meta:ClusterLabel rdf:type owl:NamedIndividual ,
                                sdc4-meta:ConceptualAspect ;
                       rdfs:comment "Represents the descriptive label for a cluster component."@en ;
                       rdfs:label "Cluster Label"@en .


###  https://semanticdatacharter.com/ontology/sdc4-meta/ConceptualEntityIdentity
sdc4-meta:ConceptualEntityIdentity rdf:type owl:NamedIndividual ,
                                            sdc4-meta:ConceptualAspect ;
                                   rdfs:comment "Represents the aspect of a conceptual entity that identifies it, typically via the 'label' element."@en ;
                                   rdfs:label "Conceptual Entity Identity"@en .


###  https://semanticdatacharter.com/ontology/sdc4-meta/ConceptualValue
sdc4-meta:ConceptualValue rdf:type owl:NamedIndividual ,
                                   sdc4-meta:ConceptualAspect ;
                          rdfs:comment "Represents the primary data value aspect of a conceptual entity (e.g., xdstring-value)."@en ;
                          rdfs:label "Conceptual Value"@en .


###  https://semanticdatacharter.com/ontology/sdc4-meta/ContainedComponents
sdc4-meta:ContainedComponents rdf:type owl:NamedIndividual ,
                                       sdc4-meta:ConceptualAspect ;
                              rdfs:comment "Represents the list of components contained within a cluster."@en ;
                              rdfs:label "Contained Components"@en .


###  https://semanticdatacharter.com/ontology/sdc4-meta/CountUnits
sdc4-meta:CountUnits rdf:type owl:NamedIndividual ,
                              sdc4-meta:ConceptualAspect ;
                     rdfs:comment "Represents the units or type of items being counted."@en ;
                     rdfs:label "Count Units"@en .


###  https://semanticdatacharter.com/ontology/sdc4-meta/CountValue
sdc4-meta:CountValue rdf:type owl:NamedIndividual ,
                              sdc4-meta:ConceptualAspect ;
                     rdfs:comment "Represents the integer value of counted items."@en ;
                     rdfs:label "Count Value"@en .


###  https://semanticdatacharter.com/ontology/sdc4-meta/DataAttestation
sdc4-meta:DataAttestation rdf:type owl:NamedIndividual ,
                                   sdc4-meta:ConceptualAspect ;
                          rdfs:comment "Represents the attestation record of a data instance."@en ;
                          rdfs:label "Data Attestation"@en .


###  https://semanticdatacharter.com/ontology/sdc4-meta/DataAudits
sdc4-meta:DataAudits rdf:type owl:NamedIndividual ,
                              sdc4-meta:ConceptualAspect ;
                     rdfs:comment "Represents a list of audit records for the data."@en ;
                     rdfs:label "Data Audits"@en .


###  https://semanticdatacharter.com/ontology/sdc4-meta/DataModelEncoding
sdc4-meta:DataModelEncoding rdf:type owl:NamedIndividual ,
                                     sdc4-meta:ConceptualAspect ;
                            rdfs:comment "Represents the character set encoding of a Data Model."@en ;
                            rdfs:label "Data Model Encoding"@en .


###  https://semanticdatacharter.com/ontology/sdc4-meta/DataModelLanguage
sdc4-meta:DataModelLanguage rdf:type owl:NamedIndividual ,
                                     sdc4-meta:ConceptualAspect ;
                            rdfs:comment "Represents the language in which a Data Model is written."@en ;
                            rdfs:label "Data Model Language"@en .


###  https://semanticdatacharter.com/ontology/sdc4-meta/DataModelName
sdc4-meta:DataModelName rdf:type owl:NamedIndividual ,
                                 sdc4-meta:ConceptualAspect ;
                        rdfs:comment "Represents the descriptive name of a Data Model."@en ;
                        rdfs:label "Data Model Name"@en .


###  https://semanticdatacharter.com/ontology/sdc4-meta/DataModelPayload
sdc4-meta:DataModelPayload rdf:type owl:NamedIndividual ,
                                    sdc4-meta:ConceptualAspect ;
                           rdfs:comment "Represents the main data structure or payload of a Data Model."@en ;
                           rdfs:label "Data Model Payload"@en .


###  https://semanticdatacharter.com/ontology/sdc4-meta/DataParticipations
sdc4-meta:DataParticipations rdf:type owl:NamedIndividual ,
                                      sdc4-meta:ConceptualAspect ;
                             rdfs:comment "Represents a list of participations related to the data."@en ;
                             rdfs:label "Data Participations"@en .


###  https://semanticdatacharter.com/ontology/sdc4-meta/DataProtocol
sdc4-meta:DataProtocol rdf:type owl:NamedIndividual ,
                                sdc4-meta:ConceptualAspect ;
                       rdfs:comment "Represents the protocol used for data collection."@en ;
                       rdfs:label "Data Protocol"@en .


###  https://semanticdatacharter.com/ontology/sdc4-meta/DataProvider
sdc4-meta:DataProvider rdf:type owl:NamedIndividual ,
                                sdc4-meta:ConceptualAspect ;
                       rdfs:comment "Represents the source or provider of the data."@en ;
                       rdfs:label "Data Provider"@en .


###  https://semanticdatacharter.com/ontology/sdc4-meta/DataQualityStatus
sdc4-meta:DataQualityStatus rdf:type owl:NamedIndividual ,
                                     sdc4-meta:ConceptualAspect ;
                            rdfs:comment "Represents the data quality status (e.g., exceptional value) aspect of a conceptual entity."@en ;
                            rdfs:label "Data Quality Status"@en .


###  https://semanticdatacharter.com/ontology/sdc4-meta/DataSubject
sdc4-meta:DataSubject rdf:type owl:NamedIndividual ,
                               sdc4-meta:ConceptualAspect ;
                      rdfs:comment "Represents the human subject of the data."@en ;
                      rdfs:label "Data Subject"@en .


###  https://semanticdatacharter.com/ontology/sdc4-meta/DoubleUnits
sdc4-meta:DoubleUnits rdf:type owl:NamedIndividual ,
                               sdc4-meta:ConceptualAspect ;
                      rdfs:comment "Represents the units of a double quantity."@en ;
                      rdfs:label "Double Units"@en .


###  https://semanticdatacharter.com/ontology/sdc4-meta/DoubleValue
sdc4-meta:DoubleValue rdf:type owl:NamedIndividual ,
                               sdc4-meta:ConceptualAspect ;
                      rdfs:comment "Represents the double value of a quantity."@en ;
                      rdfs:label "Double Value"@en .


###  https://semanticdatacharter.com/ontology/sdc4-meta/ExceptionalValueName
sdc4-meta:ExceptionalValueName rdf:type owl:NamedIndividual ,
                                        sdc4-meta:ConceptualAspect ;
                               rdfs:comment "Represents the name or type of an exceptional value."@en ;
                               rdfs:label "Exceptional Value Name"@en .


###  https://semanticdatacharter.com/ontology/sdc4-meta/ExternalLinks
sdc4-meta:ExternalLinks rdf:type owl:NamedIndividual ,
                                 sdc4-meta:ConceptualAspect ;
                        rdfs:comment "Represents external links associated with the data model."@en ;
                        rdfs:label "External Links"@en .


###  https://semanticdatacharter.com/ontology/sdc4-meta/FileAltText
sdc4-meta:FileAltText rdf:type owl:NamedIndividual ,
                               sdc4-meta:ConceptualAspect ;
                      rdfs:comment "Represents the alternative text for a file conceptual entity."@en ;
                      rdfs:label "File Alt Text"@en .


###  https://semanticdatacharter.com/ontology/sdc4-meta/FileCompressionType
sdc4-meta:FileCompressionType rdf:type owl:NamedIndividual ,
                                       sdc4-meta:ConceptualAspect ;
                              rdfs:comment "Represents the compression type of a file conceptual entity."@en ;
                              rdfs:label "File Compression Type"@en .


###  https://semanticdatacharter.com/ontology/sdc4-meta/FileEncoding
sdc4-meta:FileEncoding rdf:type owl:NamedIndividual ,
                                sdc4-meta:ConceptualAspect ;
                       rdfs:comment "Represents the character encoding scheme of a file conceptual entity."@en ;
                       rdfs:label "File Encoding"@en .


###  https://semanticdatacharter.com/ontology/sdc4-meta/FileFormalism
sdc4-meta:FileFormalism rdf:type owl:NamedIndividual ,
                                 sdc4-meta:ConceptualAspect ;
                        rdfs:comment "Represents the formalism or syntax of a file conceptual entity."@en ;
                        rdfs:label "File Formalism"@en .


###  https://semanticdatacharter.com/ontology/sdc4-meta/FileHashFunction
sdc4-meta:FileHashFunction rdf:type owl:NamedIndividual ,
                                    sdc4-meta:ConceptualAspect ;
                           rdfs:comment "Represents the hash function used for a file conceptual entity."@en ;
                           rdfs:label "File Hash Function"@en .


###  https://semanticdatacharter.com/ontology/sdc4-meta/FileHashResult
sdc4-meta:FileHashResult rdf:type owl:NamedIndividual ,
                                  sdc4-meta:ConceptualAspect ;
                         rdfs:comment "Represents the hash result of a file conceptual entity."@en ;
                         rdfs:label "File Hash Result"@en .


###  https://semanticdatacharter.com/ontology/sdc4-meta/FileMediaContent
sdc4-meta:FileMediaContent rdf:type owl:NamedIndividual ,
                                    sdc4-meta:ConceptualAspect ;
                           rdfs:comment "Represents the embedded media content of a file conceptual entity."@en ;
                           rdfs:label "File Media Content"@en .


###  https://semanticdatacharter.com/ontology/sdc4-meta/FileMediaType
sdc4-meta:FileMediaType rdf:type owl:NamedIndividual ,
                                 sdc4-meta:ConceptualAspect ;
                        rdfs:comment "Represents the MIME type of a file conceptual entity."@en ;
                        rdfs:label "File Media Type"@en .


###  https://semanticdatacharter.com/ontology/sdc4-meta/FileSize
sdc4-meta:FileSize rdf:type owl:NamedIndividual ,
                            sdc4-meta:ConceptualAspect ;
                   rdfs:comment "Represents the size in bytes of a file conceptual entity."@en ;
                   rdfs:label "File Size"@en .


###  https://semanticdatacharter.com/ontology/sdc4-meta/FileURI
sdc4-meta:FileURI rdf:type owl:NamedIndividual ,
                           sdc4-meta:ConceptualAspect ;
                  rdfs:comment "Represents the URI of a file conceptual entity."@en ;
                  rdfs:label "File URI"@en .


###  https://semanticdatacharter.com/ontology/sdc4-meta/FloatUnits
sdc4-meta:FloatUnits rdf:type owl:NamedIndividual ,
                              sdc4-meta:ConceptualAspect ;
                     rdfs:comment "Represents the units of a float quantity."@en ;
                     rdfs:label "Float Units"@en .


###  https://semanticdatacharter.com/ontology/sdc4-meta/FloatValue
sdc4-meta:FloatValue rdf:type owl:NamedIndividual ,
                              sdc4-meta:ConceptualAspect ;
                     rdfs:comment "Represents the float value of a quantity."@en ;
                     rdfs:label "Float Value"@en .


###  https://semanticdatacharter.com/ontology/sdc4-meta/GeospatialLatitude
sdc4-meta:GeospatialLatitude rdf:type owl:NamedIndividual ,
                                      sdc4-meta:ConceptualAspect ;
                             rdfs:comment "Represents the latitude aspect of a conceptual entity."@en ;
                             rdfs:label "Geospatial Latitude"@en .


###  https://semanticdatacharter.com/ontology/sdc4-meta/GeospatialLongitude
sdc4-meta:GeospatialLongitude rdf:type owl:NamedIndividual ,
                                       sdc4-meta:ConceptualAspect ;
                              rdfs:comment "Represents the longitude aspect of a conceptual entity."@en ;
                              rdfs:label "Geospatial Longitude"@en .


###  https://semanticdatacharter.com/ontology/sdc4-meta/InstanceCreationTimestamp
sdc4-meta:InstanceCreationTimestamp rdf:type owl:NamedIndividual ,
                                             sdc4-meta:ConceptualAspect ;
                                    rdfs:comment "Represents the timestamp of a data instance's creation."@en ;
                                    rdfs:label "Instance Creation Timestamp"@en .


###  https://semanticdatacharter.com/ontology/sdc4-meta/InstanceIdentifier
sdc4-meta:InstanceIdentifier rdf:type owl:NamedIndividual ,
                                      sdc4-meta:ConceptualAspect ;
                             rdfs:comment "Represents the unique identifier for a data instance."@en ;
                             rdfs:label "Instance Identifier"@en .


###  https://semanticdatacharter.com/ontology/sdc4-meta/InstanceVersion
sdc4-meta:InstanceVersion rdf:type owl:NamedIndividual ,
                                   sdc4-meta:ConceptualAspect ;
                          rdfs:comment "Represents the version identifier for a data instance."@en ;
                          rdfs:label "Instance Version"@en .


###  https://semanticdatacharter.com/ontology/sdc4-meta/IntervalLowerBound
sdc4-meta:IntervalLowerBound rdf:type owl:NamedIndividual ,
                                      sdc4-meta:ConceptualAspect ;
                             rdfs:comment "Represents the lower boundary of an interval."@en ;
                             rdfs:label "Interval Lower Bound"@en .


###  https://semanticdatacharter.com/ontology/sdc4-meta/IntervalLowerBounded
sdc4-meta:IntervalLowerBounded rdf:type owl:NamedIndividual ,
                                        sdc4-meta:ConceptualAspect ;
                               rdfs:comment "Represents whether an interval has a lower bound."@en ;
                               rdfs:label "Interval Lower Bounded"@en .


###  https://semanticdatacharter.com/ontology/sdc4-meta/IntervalLowerIncluded
sdc4-meta:IntervalLowerIncluded rdf:type owl:NamedIndividual ,
                                         sdc4-meta:ConceptualAspect ;
                                rdfs:comment "Represents whether the lower boundary of an interval is included."@en ;
                                rdfs:label "Interval Lower Included"@en .


###  https://semanticdatacharter.com/ontology/sdc4-meta/IntervalUnitsDefinition
sdc4-meta:IntervalUnitsDefinition rdf:type owl:NamedIndividual ,
                                           sdc4-meta:ConceptualAspect ;
                                  rdfs:comment "Represents the units definition for an interval."@en ;
                                  rdfs:label "Interval Units Definition"@en .


###  https://semanticdatacharter.com/ontology/sdc4-meta/IntervalUpperBound
sdc4-meta:IntervalUpperBound rdf:type owl:NamedIndividual ,
                                      sdc4-meta:ConceptualAspect ;
                             rdfs:comment "Represents the upper boundary of an interval."@en ;
                             rdfs:label "Interval Upper Bound"@en .


###  https://semanticdatacharter.com/ontology/sdc4-meta/IntervalUpperBounded
sdc4-meta:IntervalUpperBounded rdf:type owl:NamedIndividual ,
                                        sdc4-meta:ConceptualAspect ;
                               rdfs:comment "Represents whether an interval has an upper bound."@en ;
                               rdfs:label "Interval Upper Bounded"@en .


###  https://semanticdatacharter.com/ontology/sdc4-meta/IntervalUpperIncluded
sdc4-meta:IntervalUpperIncluded rdf:type owl:NamedIndividual ,
                                         sdc4-meta:ConceptualAspect ;
                                rdfs:comment "Represents whether the upper boundary of an interval is included."@en ;
                                rdfs:label "Interval Upper Included"@en .


###  https://semanticdatacharter.com/ontology/sdc4-meta/LanguageCode
sdc4-meta:LanguageCode rdf:type owl:NamedIndividual ,
                                sdc4-meta:ConceptualAspect ;
                       rdfs:comment "Represents the language code aspect of a conceptual entity."@en ;
                       rdfs:label "Language Code"@en .


###  https://semanticdatacharter.com/ontology/sdc4-meta/LinkRelationTerm
sdc4-meta:LinkRelationTerm rdf:type owl:NamedIndividual ,
                                    sdc4-meta:ConceptualAspect ;
                           rdfs:comment "Represents the descriptive term for a link's relation."@en ;
                           rdfs:label "Link Relation Term"@en .


###  https://semanticdatacharter.com/ontology/sdc4-meta/LinkRelationURI
sdc4-meta:LinkRelationURI rdf:type owl:NamedIndividual ,
                                   sdc4-meta:ConceptualAspect ;
                          rdfs:comment "Represents the URI defining a link's relation term."@en ;
                          rdfs:label "Link Relation URI"@en .


###  https://semanticdatacharter.com/ontology/sdc4-meta/LinkTargetURI
sdc4-meta:LinkTargetURI rdf:type owl:NamedIndividual ,
                                 sdc4-meta:ConceptualAspect ;
                        rdfs:comment "Represents the target URI of a link conceptual entity."@en ;
                        rdfs:label "Link Target URI"@en .


###  https://semanticdatacharter.com/ontology/sdc4-meta/MagnitudeStatusIndicator
sdc4-meta:MagnitudeStatusIndicator rdf:type owl:NamedIndividual ,
                                            sdc4-meta:ConceptualAspect ;
                                   rdfs:comment "Represents the status of a quantity's magnitude relative to a target."@en ;
                                   rdfs:label "Magnitude Status Indicator"@en .


###  https://semanticdatacharter.com/ontology/sdc4-meta/NormalStatusIndicator
sdc4-meta:NormalStatusIndicator rdf:type owl:NamedIndividual ,
                                         sdc4-meta:ConceptualAspect ;
                                rdfs:comment "Represents the normal status indicator for an ordered value."@en ;
                                rdfs:label "Normal Status Indicator"@en .


###  https://semanticdatacharter.com/ontology/sdc4-meta/OrdinalSymbol
sdc4-meta:OrdinalSymbol rdf:type owl:NamedIndividual ,
                                 sdc4-meta:ConceptualAspect ;
                        rdfs:comment "Represents the symbolic representation of an ordinal value."@en ;
                        rdfs:label "Ordinal Symbol"@en .


###  https://semanticdatacharter.com/ontology/sdc4-meta/OrdinalValue
sdc4-meta:OrdinalValue rdf:type owl:NamedIndividual ,
                                sdc4-meta:ConceptualAspect ;
                       rdfs:comment "Represents the numerical ordinal value."@en ;
                       rdfs:label "Ordinal Value"@en .


###  https://semanticdatacharter.com/ontology/sdc4-meta/ParticipationEndTime
sdc4-meta:ParticipationEndTime rdf:type owl:NamedIndividual ,
                                        sdc4-meta:ConceptualAspect ;
                               rdfs:comment "Represents the end datetime of a participation."@en ;
                               rdfs:label "Participation End Time"@en .


###  https://semanticdatacharter.com/ontology/sdc4-meta/ParticipationFunction
sdc4-meta:ParticipationFunction rdf:type owl:NamedIndividual ,
                                         sdc4-meta:ConceptualAspect ;
                                rdfs:comment "Represents the function of the performer in a participation."@en ;
                                rdfs:label "Participation Function"@en .


###  https://semanticdatacharter.com/ontology/sdc4-meta/ParticipationLabel
sdc4-meta:ParticipationLabel rdf:type owl:NamedIndividual ,
                                      sdc4-meta:ConceptualAspect ;
                             rdfs:comment "Represents the descriptive label for a participation."@en ;
                             rdfs:label "Participation Label"@en .


###  https://semanticdatacharter.com/ontology/sdc4-meta/ParticipationMode
sdc4-meta:ParticipationMode rdf:type owl:NamedIndividual ,
                                     sdc4-meta:ConceptualAspect ;
                            rdfs:comment "Represents the mode of interaction in a participation."@en ;
                            rdfs:label "Participation Mode"@en .


###  https://semanticdatacharter.com/ontology/sdc4-meta/ParticipationPerformer
sdc4-meta:ParticipationPerformer rdf:type owl:NamedIndividual ,
                                          sdc4-meta:ConceptualAspect ;
                                 rdfs:comment "Represents the party performing a participation."@en ;
                                 rdfs:label "Participation Performer"@en .


###  https://semanticdatacharter.com/ontology/sdc4-meta/ParticipationStartTime
sdc4-meta:ParticipationStartTime rdf:type owl:NamedIndividual ,
                                          sdc4-meta:ConceptualAspect ;
                                 rdfs:comment "Represents the start datetime of a participation."@en ;
                                 rdfs:label "Participation Start Time"@en .


###  https://semanticdatacharter.com/ontology/sdc4-meta/PartyDetails
sdc4-meta:PartyDetails rdf:type owl:NamedIndividual ,
                                sdc4-meta:ConceptualAspect ;
                       rdfs:comment "Represents structured details about a party."@en ;
                       rdfs:label "Party Details"@en .


###  https://semanticdatacharter.com/ontology/sdc4-meta/PartyLabel
sdc4-meta:PartyLabel rdf:type owl:NamedIndividual ,
                              sdc4-meta:ConceptualAspect ;
                     rdfs:comment "Represents the descriptive label for a party."@en ;
                     rdfs:label "Party Label"@en .


###  https://semanticdatacharter.com/ontology/sdc4-meta/PartyName
sdc4-meta:PartyName rdf:type owl:NamedIndividual ,
                             sdc4-meta:ConceptualAspect ;
                    rdfs:comment "Represents the human-readable name of a party."@en ;
                    rdfs:label "Party Name"@en .


###  https://semanticdatacharter.com/ontology/sdc4-meta/PartyReference
sdc4-meta:PartyReference rdf:type owl:NamedIndividual ,
                                  sdc4-meta:ConceptualAspect ;
                         rdfs:comment "Represents a reference to more detailed information about a party."@en ;
                         rdfs:label "Party Reference"@en .


###  https://semanticdatacharter.com/ontology/sdc4-meta/PrecisionDigits
sdc4-meta:PrecisionDigits rdf:type owl:NamedIndividual ,
                                   sdc4-meta:ConceptualAspect ;
                          rdfs:comment "Represents the number of significant decimal digits for a measurement."@en ;
                          rdfs:label "Precision Digits"@en .


###  https://semanticdatacharter.com/ontology/sdc4-meta/QuantityUnits
sdc4-meta:QuantityUnits rdf:type owl:NamedIndividual ,
                                 sdc4-meta:ConceptualAspect ;
                        rdfs:comment "Represents the units of a quantity."@en ;
                        rdfs:label "Quantity Units"@en .


###  https://semanticdatacharter.com/ontology/sdc4-meta/QuantityValue
sdc4-meta:QuantityValue rdf:type owl:NamedIndividual ,
                                 sdc4-meta:ConceptualAspect ;
                        rdfs:comment "Represents the numeric decimal value of a quantity."@en ;
                        rdfs:label "Quantity Value"@en .


###  https://semanticdatacharter.com/ontology/sdc4-meta/ReferenceRangeDefinition
sdc4-meta:ReferenceRangeDefinition rdf:type owl:NamedIndividual ,
                                            sdc4-meta:ConceptualAspect ;
                                   rdfs:comment "Represents the definition of a reference range."@en ;
                                   rdfs:label "Reference Range Definition"@en .


###  https://semanticdatacharter.com/ontology/sdc4-meta/ReferenceRangeDefinitionTerm
sdc4-meta:ReferenceRangeDefinitionTerm rdf:type owl:NamedIndividual ,
                                                sdc4-meta:ConceptualAspect ;
                                       rdfs:comment "Represents the term defining the meaning of a reference range."@en ;
                                       rdfs:label "Reference Range Definition Term"@en .


###  https://semanticdatacharter.com/ontology/sdc4-meta/ReferenceRangeInterval
sdc4-meta:ReferenceRangeInterval rdf:type owl:NamedIndividual ,
                                          sdc4-meta:ConceptualAspect ;
                                 rdfs:comment "Represents the data range for a reference range."@en ;
                                 rdfs:label "Reference Range Interval"@en .


###  https://semanticdatacharter.com/ontology/sdc4-meta/ReferenceRangeIsNormal
sdc4-meta:ReferenceRangeIsNormal rdf:type owl:NamedIndividual ,
                                          sdc4-meta:ConceptualAspect ;
                                 rdfs:comment "Represents whether a reference range is considered normal."@en ;
                                 rdfs:label "Reference Range Is Normal"@en .


###  https://semanticdatacharter.com/ontology/sdc4-meta/StructuralComponent
sdc4-meta:StructuralComponent rdf:type owl:NamedIndividual ,
                                       sdc4-meta:ConceptualAspect ;
                              rdfs:comment "Represents a generic structural component within a data model (e.g., Item, Cluster, XdAdapter)."@en ;
                              rdfs:label "Structural Component"@en .


###  https://semanticdatacharter.com/ontology/sdc4-meta/SystemIdentifier
sdc4-meta:SystemIdentifier rdf:type owl:NamedIndividual ,
                                    sdc4-meta:ConceptualAspect ;
                           rdfs:comment "Represents the identifier of a system involved in an audit."@en ;
                           rdfs:label "System Identifier"@en .


###  https://semanticdatacharter.com/ontology/sdc4-meta/SystemUser
sdc4-meta:SystemUser rdf:type owl:NamedIndividual ,
                              sdc4-meta:ConceptualAspect ;
                     rdfs:comment "Represents the user involved in an audit."@en ;
                     rdfs:label "System User"@en .


###  https://semanticdatacharter.com/ontology/sdc4-meta/TemporalDate
sdc4-meta:TemporalDate rdf:type owl:NamedIndividual ,
                                sdc4-meta:ConceptualAspect ;
                       rdfs:comment "Represents a specific calendar date."@en ;
                       rdfs:label "Temporal Date"@en .


###  https://semanticdatacharter.com/ontology/sdc4-meta/TemporalDateTime
sdc4-meta:TemporalDateTime rdf:type owl:NamedIndividual ,
                                    sdc4-meta:ConceptualAspect ;
                           rdfs:comment "Represents a specific instant in time."@en ;
                           rdfs:label "Temporal Date Time"@en .


###  https://semanticdatacharter.com/ontology/sdc4-meta/TemporalDay
sdc4-meta:TemporalDay rdf:type owl:NamedIndividual ,
                               sdc4-meta:ConceptualAspect ;
                      rdfs:comment "Represents a recurring Gregorian day."@en ;
                      rdfs:label "Temporal Day"@en .


###  https://semanticdatacharter.com/ontology/sdc4-meta/TemporalDuration
sdc4-meta:TemporalDuration rdf:type owl:NamedIndividual ,
                                    sdc4-meta:ConceptualAspect ;
                           rdfs:comment "Represents a duration of time."@en ;
                           rdfs:label "Temporal Duration"@en .


###  https://semanticdatacharter.com/ontology/sdc4-meta/TemporalMonth
sdc4-meta:TemporalMonth rdf:type owl:NamedIndividual ,
                                 sdc4-meta:ConceptualAspect ;
                        rdfs:comment "Represents a recurring Gregorian month."@en ;
                        rdfs:label "Temporal Month"@en .


###  https://semanticdatacharter.com/ontology/sdc4-meta/TemporalMonthDay
sdc4-meta:TemporalMonthDay rdf:type owl:NamedIndividual ,
                                    sdc4-meta:ConceptualAspect ;
                           rdfs:comment "Represents a recurring Gregorian day in a recurring month."@en ;
                           rdfs:label "Temporal Month Day"@en .


###  https://semanticdatacharter.com/ontology/sdc4-meta/TemporalTime
sdc4-meta:TemporalTime rdf:type owl:NamedIndividual ,
                                sdc4-meta:ConceptualAspect ;
                       rdfs:comment "Represents a recurring time of day."@en ;
                       rdfs:label "Temporal Time"@en .


###  https://semanticdatacharter.com/ontology/sdc4-meta/TemporalYear
sdc4-meta:TemporalYear rdf:type owl:NamedIndividual ,
                                sdc4-meta:ConceptualAspect ;
                       rdfs:comment "Represents a specific Gregorian calendar year."@en ;
                       rdfs:label "Temporal Year"@en .


###  https://semanticdatacharter.com/ontology/sdc4-meta/TemporalYearMonth
sdc4-meta:TemporalYearMonth rdf:type owl:NamedIndividual ,
                                     sdc4-meta:ConceptualAspect ;
                            rdfs:comment "Represents a specific Gregorian month in a specific year."@en ;
                            rdfs:label "Temporal Year Month"@en .


###  https://semanticdatacharter.com/ontology/sdc4-meta/TimeModified
sdc4-meta:TimeModified rdf:type owl:NamedIndividual ,
                                sdc4-meta:ConceptualAspect ;
                       rdfs:comment "Represents the aspect of a conceptual entity related to when its data was last modified."@en ;
                       rdfs:label "Time Modified"@en .


###  https://semanticdatacharter.com/ontology/sdc4-meta/TimeRecorded
sdc4-meta:TimeRecorded rdf:type owl:NamedIndividual ,
                                sdc4-meta:ConceptualAspect ;
                       rdfs:comment "Represents the aspect of a conceptual entity related to when its data was recorded."@en ;
                       rdfs:label "Time Recorded"@en .


###  https://semanticdatacharter.com/ontology/sdc4-meta/UnitsName
sdc4-meta:UnitsName rdf:type owl:NamedIndividual ,
                             sdc4-meta:ConceptualAspect ;
                    rdfs:comment "Represents the name of units."@en ;
                    rdfs:label "Units Name"@en .


###  https://semanticdatacharter.com/ontology/sdc4-meta/UnitsURI
sdc4-meta:UnitsURI rdf:type owl:NamedIndividual ,
                            sdc4-meta:ConceptualAspect ;
                   rdfs:comment "Represents the URI for units definition."@en ;
                   rdfs:label "Units URI"@en .


###  https://semanticdatacharter.com/ontology/sdc4-meta/ValidTimeBeginning
sdc4-meta:ValidTimeBeginning rdf:type owl:NamedIndividual ,
                                      sdc4-meta:ConceptualAspect ;
                             rdfs:comment "Represents the aspect of a conceptual entity related to its valid start time."@en ;
                             rdfs:label "Valid Time Beginning"@en .


###  https://semanticdatacharter.com/ontology/sdc4-meta/ValidTimeEnd
sdc4-meta:ValidTimeEnd rdf:type owl:NamedIndividual ,
                                sdc4-meta:ConceptualAspect ;
                       rdfs:comment "Represents the aspect of a conceptual entity related to its valid end time."@en ;
                       rdfs:label "Valid Time End"@en .


###  https://semanticdatacharter.com/ontology/sdc4-meta/WorkflowIdentifier
sdc4-meta:WorkflowIdentifier rdf:type owl:NamedIndividual ,
                                      sdc4-meta:ConceptualAspect ;
                             rdfs:comment "Represents the identifier of an external workflow engine."@en ;
                             rdfs:label "Workflow Identifier"@en .


###  https://semanticdatacharter.com/ontology/sdc4-meta/WorkflowState
sdc4-meta:WorkflowState rdf:type owl:NamedIndividual ,
                                 sdc4-meta:ConceptualAspect ;
                        rdfs:comment "Represents the current state within a workflow."@en ;
                        rdfs:label "Workflow State"@en .


###  sdc4:ASKRType
<sdc4:ASKRType> rdf:type owl:NamedIndividual ,
                         sdc4-meta:ReferenceModelComponent ;
                sdc4-meta:hasDescriptiveElement <sdc4:ASKRType/ev-name> .


###  sdc4:ASKUType
<sdc4:ASKUType> rdf:type owl:NamedIndividual ,
                         sdc4-meta:ReferenceModelComponent ;
                sdc4-meta:hasDescriptiveElement <sdc4:ASKUType/ev-name> .


###  sdc4:AttestationType
<sdc4:AttestationType> rdf:type owl:NamedIndividual ,
                                sdc4-meta:ReferenceModelComponent ;
                       sdc4-meta:hasDescriptiveElement <sdc4:AttestationType/committed> ,
                                                       <sdc4:AttestationType/committer> ,
                                                       <sdc4:AttestationType/label> ,
                                                       <sdc4:AttestationType/pending> ,
                                                       <sdc4:AttestationType/proof> ,
                                                       <sdc4:AttestationType/reason> ,
                                                       <sdc4:AttestationType/view> ;
                       rdfs:comment "Record an attestation by a party of the DM content."@en ;
                       rdfs:label "AttestationType"@en .


###  sdc4:AuditType
<sdc4:AuditType> rdf:type owl:NamedIndividual ,
                          sdc4-meta:ReferenceModelComponent ;
                 sdc4-meta:hasDescriptiveElement <sdc4:AuditType/label> ,
                                                 <sdc4:AuditType/location> ,
                                                 <sdc4:AuditType/system-id> ,
                                                 <sdc4:AuditType/system-user> ,
                                                 <sdc4:AuditType/timestamp> ;
                 rdfs:comment "AuditType provides a mechanism to identify the who/where/when tracking of instances as they move from system to system."@en ;
                 rdfs:label "AuditType"@en .


###  sdc4:ClusterType
<sdc4:ClusterType> rdf:type owl:NamedIndividual ,
                            sdc4-meta:ReferenceModelComponent ;
                   sdc4-meta:hasDescriptiveElement <sdc4:ClusterType/Items> ,
                                                   <sdc4:ClusterType/label> .


###  sdc4:DERType
<sdc4:DERType> rdf:type owl:NamedIndividual ,
                        sdc4-meta:ReferenceModelComponent ;
               sdc4-meta:hasDescriptiveElement <sdc4:DERType/ev-name> .


###  sdc4:DMType
<sdc4:DMType> rdf:type owl:NamedIndividual ,
                       sdc4-meta:ReferenceModelComponent ;
              sdc4-meta:hasDescriptiveElement <sdc4:DMType/acs> ,
                                              <sdc4:DMType/attestation> ,
                                              <sdc4:DMType/audit> ,
                                              <sdc4:DMType/creation_timestamp> ,
                                              <sdc4:DMType/current-state> ,
                                              <sdc4:DMType/data> ,
                                              <sdc4:DMType/dm-encoding> ,
                                              <sdc4:DMType/dm-language> ,
                                              <sdc4:DMType/instance_id> ,
                                              <sdc4:DMType/instance_version> ,
                                              <sdc4:DMType/label> ,
                                              <sdc4:DMType/links> ,
                                              <sdc4:DMType/participations> ,
                                              <sdc4:DMType/protocol> ,
                                              <sdc4:DMType/provider> ,
                                              <sdc4:DMType/subject> ,
                                              <sdc4:DMType/workflow> ;
              rdfs:comment "This is the root node of a Data Model (DM)."@en ;
              rdfs:label "DMType"@en .


###  sdc4:ExceptionalValue
<sdc4:ExceptionalValue> rdf:type owl:NamedIndividual ,
                                 sdc4-meta:ReferenceModelElement ;
                        sdc4-meta:describesConceptualAspect sdc4-meta:DataQualityStatus ;
                        rdfs:comment "In an invalid instance, the application can indicate here why data is missing or invalid."@en ;
                        rdfs:label "ExceptionalValue"@en .


###  sdc4:ExceptionalValueType
<sdc4:ExceptionalValueType> rdf:type owl:NamedIndividual ,
                                     sdc4-meta:ReferenceModelComponent ;
                            sdc4-meta:hasDescriptiveElement <sdc4:ExceptionalValueType/ev-name> .


###  sdc4:INVType
<sdc4:INVType> rdf:type owl:NamedIndividual ,
                        sdc4-meta:ReferenceModelComponent ;
               sdc4-meta:hasDescriptiveElement <sdc4:INVType/ev-name> .


###  sdc4:InvlType
<sdc4:InvlType> rdf:type owl:NamedIndividual ,
                         sdc4-meta:ReferenceModelComponent ;
                rdfs:comment "Defines the set of permissible, comparable datatypes that can be used as the boundary for an interval."@en ;
                rdfs:label "InvlType"@en .


###  sdc4:InvlUnits
<sdc4:InvlUnits> rdf:type owl:NamedIndividual ,
                          sdc4-meta:ReferenceModelComponent ;
                 sdc4-meta:hasDescriptiveElement <sdc4:InvlUnits/units-name> ,
                                                 <sdc4:InvlUnits/units-uri> ;
                 rdfs:comment "The units designation for an Interval."@en ;
                 rdfs:label "InvlUnits"@en .


###  sdc4:Item
<sdc4:Item> rdf:type owl:NamedIndividual ,
                     sdc4-meta:ReferenceModelElement ;
            sdc4-meta:describesConceptualAspect sdc4-meta:StructuralComponent ;
            rdfs:comment "The abstract parent of ClusterType and XdAdapterType structural representation types, used as a substitution group."@en ;
            rdfs:label "Item (Element)"@en .


###  sdc4:ItemType
<sdc4:ItemType> rdf:type owl:NamedIndividual ,
                         sdc4-meta:ReferenceModelComponent .


###  sdc4:MSKType
<sdc4:MSKType> rdf:type owl:NamedIndividual ,
                        sdc4-meta:ReferenceModelComponent ;
               sdc4-meta:hasDescriptiveElement <sdc4:MSKType/ev-name> .


###  sdc4:MagnitudeStatus
<sdc4:MagnitudeStatus> rdf:type owl:NamedIndividual ,
                                sdc4-meta:ReferenceModelComponent ;
                       rdfs:comment "MagnitudeStatus provides a general indication of the accuracy of the magnitude expressed in the XdQuantified subtypes."@en ;
                       rdfs:label "MagnitudeStatus"@en .


###  sdc4:NASKType
<sdc4:NASKType> rdf:type owl:NamedIndividual ,
                         sdc4-meta:ReferenceModelComponent ;
                sdc4-meta:hasDescriptiveElement <sdc4:NASKType/ev-name> .


###  sdc4:NAType
<sdc4:NAType> rdf:type owl:NamedIndividual ,
                       sdc4-meta:ReferenceModelComponent ;
              sdc4-meta:hasDescriptiveElement <sdc4:NAType/ev-name> .


###  sdc4:NAVType
<sdc4:NAVType> rdf:type owl:NamedIndividual ,
                        sdc4-meta:ReferenceModelComponent ;
               sdc4-meta:hasDescriptiveElement <sdc4:NAVType/ev-name> .


###  sdc4:NINFType
<sdc4:NINFType> rdf:type owl:NamedIndividual ,
                         sdc4-meta:ReferenceModelComponent ;
                sdc4-meta:hasDescriptiveElement <sdc4:NINFType/ev-name> .


###  sdc4:NIType
<sdc4:NIType> rdf:type owl:NamedIndividual ,
                       sdc4-meta:ReferenceModelComponent ;
              sdc4-meta:hasDescriptiveElement <sdc4:NIType/ev-name> .


###  sdc4:OTHType
<sdc4:OTHType> rdf:type owl:NamedIndividual ,
                        sdc4-meta:ReferenceModelComponent ;
               sdc4-meta:hasDescriptiveElement <sdc4:OTHType/ev-name> .


###  sdc4:PINFType
<sdc4:PINFType> rdf:type owl:NamedIndividual ,
                         sdc4-meta:ReferenceModelComponent ;
                sdc4-meta:hasDescriptiveElement <sdc4:PINFType/ev-name> .


###  sdc4:ParticipationType
<sdc4:ParticipationType> rdf:type owl:NamedIndividual ,
                                  sdc4-meta:ReferenceModelComponent ;
                         sdc4-meta:hasDescriptiveElement <sdc4:ParticipationType/end> ,
                                                         <sdc4:ParticipationType/function> ,
                                                         <sdc4:ParticipationType/label> ,
                                                         <sdc4:ParticipationType/mode> ,
                                                         <sdc4:ParticipationType/performer> ,
                                                         <sdc4:ParticipationType/start> ;
                         rdfs:comment "Model of a participation of a Party (any Actor or Role) in an activity."@en ;
                         rdfs:label "ParticipationType"@en .


###  sdc4:PartyType
<sdc4:PartyType> rdf:type owl:NamedIndividual ,
                          sdc4-meta:ReferenceModelComponent ;
                 sdc4-meta:hasDescriptiveElement <sdc4:PartyType/label> ,
                                                 <sdc4:PartyType/party-details> ,
                                                 <sdc4:PartyType/party-name> ,
                                                 <sdc4:PartyType/party-ref> ;
                 rdfs:comment "Description of a party, including an optional external link to data for this party."@en ;
                 rdfs:label "PartyType"@en .


###  sdc4:QSType
<sdc4:QSType> rdf:type owl:NamedIndividual ,
                       sdc4-meta:ReferenceModelComponent ;
              sdc4-meta:hasDescriptiveElement <sdc4:QSType/ev-name> .


###  sdc4:ReferenceRange
<sdc4:ReferenceRange> rdf:type owl:NamedIndividual ,
                               sdc4-meta:ReferenceModelElement ;
                      sdc4-meta:describesConceptualAspect sdc4-meta:ReferenceRangeDefinition ;
                      rdfs:comment "Optional list of ReferenceRanges for this value in its particular measurement context."@en ;
                      rdfs:label "ReferenceRange"@en .


###  sdc4:ReferenceRangeType
<sdc4:ReferenceRangeType> rdf:type owl:NamedIndividual ,
                                   sdc4-meta:ReferenceModelComponent ;
                          sdc4-meta:hasDescriptiveElement <sdc4:ReferenceRangeType/definition> ,
                                                          <sdc4:ReferenceRangeType/interval> ,
                                                          <sdc4:ReferenceRangeType/is-normal> .


###  sdc4:TRCType
<sdc4:TRCType> rdf:type owl:NamedIndividual ,
                        sdc4-meta:ReferenceModelComponent ;
               sdc4-meta:hasDescriptiveElement <sdc4:TRCType/ev-name> .


###  sdc4:UNCType
<sdc4:UNCType> rdf:type owl:NamedIndividual ,
                        sdc4-meta:ReferenceModelComponent ;
               sdc4-meta:hasDescriptiveElement <sdc4:UNCType/ev-name> .


###  sdc4:UNKType
<sdc4:UNKType> rdf:type owl:NamedIndividual ,
                        sdc4-meta:ReferenceModelComponent ;
               sdc4-meta:hasDescriptiveElement <sdc4:UNKType/ev-name> .


###  sdc4:XdAdapterType
<sdc4:XdAdapterType> rdf:type owl:NamedIndividual ,
                              sdc4-meta:ReferenceModelComponent ;
                     sdc4-meta:hasDescriptiveElement <sdc4:XdAdapterType/XdAdapter-value> .


###  sdc4:XdAnyType
<sdc4:XdAnyType> rdf:type owl:NamedIndividual ,
                          sdc4-meta:ReferenceModelComponent ;
                 sdc4-meta:hasDescriptiveElement <sdc4:ExceptionalValue> ,
                                                 <sdc4:XdAnyType/act> ,
                                                 <sdc4:XdAnyType/label> ,
                                                 <sdc4:XdAnyType/latitude> ,
                                                 <sdc4:XdAnyType/longitude> ,
                                                 <sdc4:XdAnyType/modified> ,
                                                 <sdc4:XdAnyType/tr> ,
                                                 <sdc4:XdAnyType/vtb> ,
                                                 <sdc4:XdAnyType/vte> .


###  sdc4:XdBooleanListType
<sdc4:XdBooleanListType> rdf:type owl:NamedIndividual ,
                                  sdc4-meta:ReferenceModelComponent ;
                         sdc4-meta:hasDescriptiveElement <sdc4:XdBooleanListType/xdbooleanlist-value> .


###  sdc4:XdBooleanType
<sdc4:XdBooleanType> rdf:type owl:NamedIndividual ,
                              sdc4-meta:ReferenceModelComponent ;
                     sdc4-meta:hasDescriptiveElement <sdc4:XdBooleanType/false-value> ,
                                                     <sdc4:XdBooleanType/true-value> .


###  sdc4:XdCountType
<sdc4:XdCountType> rdf:type owl:NamedIndividual ,
                            sdc4-meta:ReferenceModelComponent ;
                   sdc4-meta:hasDescriptiveElement <sdc4:XdCountType/xdcount-units> ,
                                                   <sdc4:XdCountType/xdcount-value> .


###  sdc4:XdDecimalListType
<sdc4:XdDecimalListType> rdf:type owl:NamedIndividual ,
                                  sdc4-meta:ReferenceModelComponent ;
                         sdc4-meta:hasDescriptiveElement <sdc4:XdDecimalListType/xddecimallist-value> .


###  sdc4:XdDoubleListType
<sdc4:XdDoubleListType> rdf:type owl:NamedIndividual ,
                                 sdc4-meta:ReferenceModelComponent ;
                        sdc4-meta:hasDescriptiveElement <sdc4:XdDoubleListType/xddoublelist-value> .


###  sdc4:XdDoubleType
<sdc4:XdDoubleType> rdf:type owl:NamedIndividual ,
                             sdc4-meta:ReferenceModelComponent ;
                    sdc4-meta:hasDescriptiveElement <sdc4:XdDoubleType/xddouble-units> ,
                                                    <sdc4:XdDoubleType/xddouble-value> .


###  sdc4:XdFileType
<sdc4:XdFileType> rdf:type owl:NamedIndividual ,
                           sdc4-meta:ReferenceModelComponent ;
                  sdc4-meta:hasDescriptiveElement <sdc4:XdFileType/alt-txt> ,
                                                  <sdc4:XdFileType/compression-type> ,
                                                  <sdc4:XdFileType/encoding> ,
                                                  <sdc4:XdFileType/formalism> ,
                                                  <sdc4:XdFileType/hash-function> ,
                                                  <sdc4:XdFileType/hash-result> ,
                                                  <sdc4:XdFileType/media-content> ,
                                                  <sdc4:XdFileType/media-type> ,
                                                  <sdc4:XdFileType/size> ,
                                                  <sdc4:XdFileType/uri> ,
                                                  <sdc4:XdFileType/xdfile-language> .


###  sdc4:XdFloatType
<sdc4:XdFloatType> rdf:type owl:NamedIndividual ,
                            sdc4-meta:ReferenceModelComponent ;
                   sdc4-meta:hasDescriptiveElement <sdc4:XdFloatType/xdfloat-units> ,
                                                   <sdc4:XdFloatType/xdfloat-value> .


###  sdc4:XdIntegerListType
<sdc4:XdIntegerListType> rdf:type owl:NamedIndividual ,
                                  sdc4-meta:ReferenceModelComponent ;
                         sdc4-meta:hasDescriptiveElement <sdc4:XdIntegerListType/xdintegerlist-value> .


###  sdc4:XdIntervalType
<sdc4:XdIntervalType> rdf:type owl:NamedIndividual ,
                               sdc4-meta:ReferenceModelComponent ;
                      sdc4-meta:hasDescriptiveElement <sdc4:XdIntervalType/interval-units> ,
                                                      <sdc4:XdIntervalType/lower> ,
                                                      <sdc4:XdIntervalType/lower_bounded> ,
                                                      <sdc4:XdIntervalType/lower_included> ,
                                                      <sdc4:XdIntervalType/upper> ,
                                                      <sdc4:XdIntervalType/upper_bounded> ,
                                                      <sdc4:XdIntervalType/upper_included> .


###  sdc4:XdLinkType
<sdc4:XdLinkType> rdf:type owl:NamedIndividual ,
                           sdc4-meta:ReferenceModelComponent ;
                  sdc4-meta:hasDescriptiveElement <sdc4:XdLinkType/link> ,
                                                  <sdc4:XdLinkType/relation> ,
                                                  <sdc4:XdLinkType/relation-uri> .


###  sdc4:XdNonNegativeIntegerListType
<sdc4:XdNonNegativeIntegerListType> rdf:type owl:NamedIndividual ,
                                             sdc4-meta:ReferenceModelComponent ;
                                    sdc4-meta:hasDescriptiveElement <sdc4:XdNonNegativeIntegerListType/xdnonnegativeintegerlist-value> .


###  sdc4:XdOrderedType
<sdc4:XdOrderedType> rdf:type owl:NamedIndividual ,
                              sdc4-meta:ReferenceModelComponent ;
                     sdc4-meta:hasDescriptiveElement <sdc4:ReferenceRange> ,
                                                     <sdc4:XdOrderedType/normal-status> .


###  sdc4:XdOrdinalType
<sdc4:XdOrdinalType> rdf:type owl:NamedIndividual ,
                              sdc4-meta:ReferenceModelComponent ;
                     sdc4-meta:hasDescriptiveElement <sdc4:XdOrdinalType/ordinal> ,
                                                     <sdc4:XdOrdinalType/symbol> .


###  sdc4:XdPositiveIntegerListType
<sdc4:XdPositiveIntegerListType> rdf:type owl:NamedIndividual ,
                                          sdc4-meta:ReferenceModelComponent ;
                                 sdc4-meta:hasDescriptiveElement <sdc4:XdPositiveIntegerListType/xdpositiveintegerlist-value> .


###  sdc4:XdQuantifiedType
<sdc4:XdQuantifiedType> rdf:type owl:NamedIndividual ,
                                 sdc4-meta:ReferenceModelComponent ;
                        sdc4-meta:hasDescriptiveElement <sdc4:XdQuantifiedType/accuracy_margin> ,
                                                        <sdc4:XdQuantifiedType/magnitude-status> ,
                                                        <sdc4:XdQuantifiedType/precision_digits> .


###  sdc4:XdQuantityType
<sdc4:XdQuantityType> rdf:type owl:NamedIndividual ,
                               sdc4-meta:ReferenceModelComponent ;
                      sdc4-meta:hasDescriptiveElement <sdc4:XdQuantityType/xdquantity-units> ,
                                                      <sdc4:XdQuantityType/xdquantity-value> .


###  sdc4:XdStringListType
<sdc4:XdStringListType> rdf:type owl:NamedIndividual ,
                                 sdc4-meta:ReferenceModelComponent ;
                        sdc4-meta:hasDescriptiveElement <sdc4:XdStringListType/xdstringlist-value> .


###  sdc4:XdStringType
<sdc4:XdStringType> rdf:type owl:NamedIndividual ,
                             sdc4-meta:ReferenceModelComponent ;
                    sdc4-meta:hasDescriptiveElement <sdc4:XdStringType/xdstring-language> ,
                                                    <sdc4:XdStringType/xdstring-value> .


###  sdc4:XdTemporalType
<sdc4:XdTemporalType> rdf:type owl:NamedIndividual ,
                               sdc4-meta:ReferenceModelComponent ;
                      sdc4-meta:hasDescriptiveElement <sdc4:XdTemporalType/xdtemporal-date> ,
                                                      <sdc4:XdTemporalType/xdtemporal-datetime> ,
                                                      <sdc4:XdTemporalType/xdtemporal-day> ,
                                                      <sdc4:XdTemporalType/xdtemporal-duration> ,
                                                      <sdc4:XdTemporalType/xdtemporal-month> ,
                                                      <sdc4:XdTemporalType/xdtemporal-month-day> ,
                                                      <sdc4:XdTemporalType/xdtemporal-time> ,
                                                      <sdc4:XdTemporalType/xdtemporal-year> ,
                                                      <sdc4:XdTemporalType/xdtemporal-year-month> .


###  sdc4:XdTokenListType
<sdc4:XdTokenListType> rdf:type owl:NamedIndividual ,
                                sdc4-meta:ReferenceModelComponent ;
                       sdc4-meta:hasDescriptiveElement <sdc4:XdTokenListType/xdtokenlist-value> .


###  sdc4:ASKRType/ev-name
<sdc4:ASKRType/ev-name> rdf:type owl:NamedIndividual ,
                                 sdc4-meta:ReferenceModelElement ;
                        sdc4-meta:describesConceptualAspect sdc4-meta:ExceptionalValueName ;
                        rdfs:comment "Fixed value \"Asked and Refused\" for ASKRType."@en ;
                        rdfs:label "ev-name (ASKR)"@en .


###  sdc4:ASKUType/ev-name
<sdc4:ASKUType/ev-name> rdf:type owl:NamedIndividual ,
                                 sdc4-meta:ReferenceModelElement ;
                        sdc4-meta:describesConceptualAspect sdc4-meta:ExceptionalValueName ;
                        rdfs:comment "Fixed value \"Asked but Unknown\" for ASKUType."@en ;
                        rdfs:label "ev-name (ASKU)"@en .


###  sdc4:AttestationType/committed
<sdc4:AttestationType/committed> rdf:type owl:NamedIndividual ,
                                          sdc4-meta:ReferenceModelElement ;
                                 sdc4-meta:describesConceptualAspect sdc4-meta:AttestationCommittedTimestamp ;
                                 rdfs:comment "Timestamp of committal of the item."@en ;
                                 rdfs:label "committed"@en .


###  sdc4:AttestationType/committer
<sdc4:AttestationType/committer> rdf:type owl:NamedIndividual ,
                                          sdc4-meta:ReferenceModelElement ;
                                 sdc4-meta:describesConceptualAspect sdc4-meta:AttestationCommitter ;
                                 rdfs:comment "Identity of person who committed the item."@en ;
                                 rdfs:label "committer"@en .


###  sdc4:AttestationType/label
<sdc4:AttestationType/label> rdf:type owl:NamedIndividual ,
                                      sdc4-meta:ReferenceModelElement ;
                             sdc4-meta:describesConceptualAspect sdc4-meta:AttestationLabel ;
                             rdfs:comment "Descriptive name of this datatype model for AttestationType."@en ;
                             rdfs:label "label (AttestationType)"@en .


###  sdc4:AttestationType/pending
<sdc4:AttestationType/pending> rdf:type owl:NamedIndividual ,
                                        sdc4-meta:ReferenceModelElement ;
                               sdc4-meta:describesConceptualAspect sdc4-meta:AttestationPendingStatus ;
                               rdfs:comment "True if this attestation is outstanding; 'false' means it has been completed."@en ;
                               rdfs:label "pending"@en .


###  sdc4:AttestationType/proof
<sdc4:AttestationType/proof> rdf:type owl:NamedIndividual ,
                                      sdc4-meta:ReferenceModelElement ;
                             sdc4-meta:describesConceptualAspect sdc4-meta:AttestationProof ;
                             rdfs:comment "Proof of attestation such as an GPG signature."@en ;
                             rdfs:label "proof"@en .


###  sdc4:AttestationType/reason
<sdc4:AttestationType/reason> rdf:type owl:NamedIndividual ,
                                       sdc4-meta:ReferenceModelElement ;
                              sdc4-meta:describesConceptualAspect sdc4-meta:AttestationReason ;
                              rdfs:comment "Reason of this attestation. Usually coded from a standardized vocabulary."@en ;
                              rdfs:label "reason (AttestationType)"@en .


###  sdc4:AttestationType/view
<sdc4:AttestationType/view> rdf:type owl:NamedIndividual ,
                                     sdc4-meta:ReferenceModelElement ;
                            sdc4-meta:describesConceptualAspect sdc4-meta:AttestationView ;
                            rdfs:comment "Optional visual representation of content attested e.g. screen image."@en ;
                            rdfs:label "view"@en .


###  sdc4:AuditType/label
<sdc4:AuditType/label> rdf:type owl:NamedIndividual ,
                                sdc4-meta:ReferenceModelElement ;
                       sdc4-meta:describesConceptualAspect sdc4-meta:AuditLabel ;
                       rdfs:comment "Descriptive name of this datatype model for AuditType."@en ;
                       rdfs:label "label (AuditType)"@en .


###  sdc4:AuditType/location
<sdc4:AuditType/location> rdf:type owl:NamedIndividual ,
                                   sdc4-meta:ReferenceModelElement ;
                          sdc4-meta:describesConceptualAspect sdc4-meta:AuditLocation ;
                          rdfs:comment "Location information of the particular site/facility within an organisation which handled the item."@en ;
                          rdfs:label "location (AuditType)"@en .


###  sdc4:AuditType/system-id
<sdc4:AuditType/system-id> rdf:type owl:NamedIndividual ,
                                    sdc4-meta:ReferenceModelElement ;
                           sdc4-meta:describesConceptualAspect sdc4-meta:SystemIdentifier ;
                           rdfs:comment "Identifier of systems which created or handled the information item."@en ;
                           rdfs:label "system-id"@en .


###  sdc4:AuditType/system-user
<sdc4:AuditType/system-user> rdf:type owl:NamedIndividual ,
                                      sdc4-meta:ReferenceModelElement ;
                             sdc4-meta:describesConceptualAspect sdc4-meta:SystemUser ;
                             rdfs:comment "User(s) who created, committed, forwarded or otherwise handled the item."@en ;
                             rdfs:label "system-user"@en .


###  sdc4:AuditType/timestamp
<sdc4:AuditType/timestamp> rdf:type owl:NamedIndividual ,
                                    sdc4-meta:ReferenceModelElement ;
                           sdc4-meta:describesConceptualAspect sdc4-meta:AuditTimestamp ;
                           rdfs:comment "Timestamp of handling the item."@en ;
                           rdfs:label "timestamp (AuditType)"@en .


###  sdc4:ClusterType/Items
<sdc4:ClusterType/Items> rdf:type owl:NamedIndividual ,
                                  sdc4-meta:ReferenceModelElement ;
                         sdc4-meta:describesConceptualAspect sdc4-meta:ContainedComponents ;
                         rdfs:comment "List of ItemTypes which may be XdAdapterTypes and/or ClusterTypes."@en ;
                         rdfs:label "Items (ClusterType)"@en .


###  sdc4:ClusterType/label
<sdc4:ClusterType/label> rdf:type owl:NamedIndividual ,
                                  sdc4-meta:ReferenceModelElement ;
                         sdc4-meta:describesConceptualAspect sdc4-meta:ClusterLabel ;
                         rdfs:comment "Descriptive subject line for this group of CMCs."@en ;
                         rdfs:label "label (ClusterType)"@en .


###  sdc4:DERType/ev-name
<sdc4:DERType/ev-name> rdf:type owl:NamedIndividual ,
                                sdc4-meta:ReferenceModelElement ;
                       sdc4-meta:describesConceptualAspect sdc4-meta:ExceptionalValueName ;
                       rdfs:comment "Fixed value \"Derived\" for DERType."@en ;
                       rdfs:label "ev-name (DER)"@en .


###  sdc4:DMType/acs
<sdc4:DMType/acs> rdf:type owl:NamedIndividual ,
                           sdc4-meta:ReferenceModelElement ;
                  sdc4-meta:describesConceptualAspect sdc4-meta:AccessControlSystem ;
                  rdfs:comment "Identifier of an externally held access control system."@en ;
                  rdfs:label "acs (DMType)"@en .


###  sdc4:DMType/attestation
<sdc4:DMType/attestation> rdf:type owl:NamedIndividual ,
                                   sdc4-meta:ReferenceModelElement ;
                          sdc4-meta:describesConceptualAspect sdc4-meta:DataAttestation ;
                          rdfs:comment "Attestation record of an instance of data."@en ;
                          rdfs:label "attestation (DMType)"@en .


###  sdc4:DMType/audit
<sdc4:DMType/audit> rdf:type owl:NamedIndividual ,
                             sdc4-meta:ReferenceModelElement ;
                    sdc4-meta:describesConceptualAspect sdc4-meta:DataAudits ;
                    rdfs:comment "List of audits from the system of original commit of information forming the content."@en ;
                    rdfs:label "audit (DMType)"@en .


###  sdc4:DMType/creation_timestamp
<sdc4:DMType/creation_timestamp> rdf:type owl:NamedIndividual ,
                                          sdc4-meta:ReferenceModelElement ;
                                 sdc4-meta:describesConceptualAspect sdc4-meta:InstanceCreationTimestamp ;
                                 rdfs:comment "An optional run-time timestamp that indicates the exact moment this specific data instance was created or generated."@en ;
                                 rdfs:label "creation_timestamp"@en .


###  sdc4:DMType/current-state
<sdc4:DMType/current-state> rdf:type owl:NamedIndividual ,
                                     sdc4-meta:ReferenceModelElement ;
                            sdc4-meta:describesConceptualAspect sdc4-meta:WorkflowState ;
                            rdfs:comment "The current state according to the state machine / workflow engine."@en ;
                            rdfs:label "current-state"@en .


###  sdc4:DMType/data
<sdc4:DMType/data> rdf:type owl:NamedIndividual ,
                            sdc4-meta:ReferenceModelElement ;
                   sdc4-meta:describesConceptualAspect sdc4-meta:DataModelPayload ;
                   rdfs:comment "The data structure of the model."@en ;
                   rdfs:label "data (DMType)"@en .


###  sdc4:DMType/dm-encoding
<sdc4:DMType/dm-encoding> rdf:type owl:NamedIndividual ,
                                   sdc4-meta:ReferenceModelElement ;
                          sdc4-meta:describesConceptualAspect sdc4-meta:DataModelEncoding ;
                          rdfs:comment "Name of character set encoding in which text values in this DM are encoded."@en ;
                          rdfs:label "dm-encoding"@en .


###  sdc4:DMType/dm-language
<sdc4:DMType/dm-language> rdf:type owl:NamedIndividual ,
                                   sdc4-meta:ReferenceModelElement ;
                          sdc4-meta:describesConceptualAspect sdc4-meta:DataModelLanguage ;
                          rdfs:comment "Mandatory indicator of the localised language in which this DM is written."@en ;
                          rdfs:label "dm-language"@en .


###  sdc4:DMType/instance_id
<sdc4:DMType/instance_id> rdf:type owl:NamedIndividual ,
                                   sdc4-meta:ReferenceModelElement ;
                          sdc4-meta:describesConceptualAspect sdc4-meta:InstanceIdentifier ;
                          rdfs:comment "An optional, globally unique identifier for this specific data instance."@en ;
                          rdfs:label "instance_id"@en .


###  sdc4:DMType/instance_version
<sdc4:DMType/instance_version> rdf:type owl:NamedIndividual ,
                                        sdc4-meta:ReferenceModelElement ;
                               sdc4-meta:describesConceptualAspect sdc4-meta:InstanceVersion ;
                               rdfs:comment "An optional identifier for the specific version of this data instance."@en ;
                               rdfs:label "instance_version"@en .


###  sdc4:DMType/label
<sdc4:DMType/label> rdf:type owl:NamedIndividual ,
                             sdc4-meta:ReferenceModelElement ;
                    sdc4-meta:describesConceptualAspect sdc4-meta:DataModelName ;
                    rdfs:comment "Descriptive name of this datatype model. Provides the semantic 'name' for the model."@en ;
                    rdfs:label "label (DMType)"@en .


###  sdc4:DMType/links
<sdc4:DMType/links> rdf:type owl:NamedIndividual ,
                             sdc4-meta:ReferenceModelElement ;
                    sdc4-meta:describesConceptualAspect sdc4-meta:ExternalLinks ;
                    rdfs:comment "Optional link(s) to other locatable structures or external entities."@en ;
                    rdfs:label "links (DMType)"@en .


###  sdc4:DMType/participations
<sdc4:DMType/participations> rdf:type owl:NamedIndividual ,
                                      sdc4-meta:ReferenceModelElement ;
                             sdc4-meta:describesConceptualAspect sdc4-meta:DataParticipations ;
                             rdfs:comment "List of other participations in the data."@en ;
                             rdfs:label "participations (DMType)"@en .


###  sdc4:DMType/protocol
<sdc4:DMType/protocol> rdf:type owl:NamedIndividual ,
                                sdc4-meta:ReferenceModelElement ;
                       sdc4-meta:describesConceptualAspect sdc4-meta:DataProtocol ;
                       rdfs:comment "Optional external identifier of protocol used when collecting the data."@en ;
                       rdfs:label "protocol (DMType)"@en .


###  sdc4:DMType/provider
<sdc4:DMType/provider> rdf:type owl:NamedIndividual ,
                                sdc4-meta:ReferenceModelElement ;
                       sdc4-meta:describesConceptualAspect sdc4-meta:DataProvider ;
                       rdfs:comment "Optional identification of the source of the information."@en ;
                       rdfs:label "provider (DMType)"@en .


###  sdc4:DMType/subject
<sdc4:DMType/subject> rdf:type owl:NamedIndividual ,
                               sdc4-meta:ReferenceModelElement ;
                      sdc4-meta:describesConceptualAspect sdc4-meta:DataSubject ;
                      rdfs:comment "Id of human subject of the data."@en ;
                      rdfs:label "subject (DMType)"@en .


###  sdc4:DMType/workflow
<sdc4:DMType/workflow> rdf:type owl:NamedIndividual ,
                                sdc4-meta:ReferenceModelElement ;
                       sdc4-meta:describesConceptualAspect sdc4-meta:WorkflowIdentifier ;
                       rdfs:comment "Identifier of externally held workflow engine (state machine) data for this workflow execution."@en ;
                       rdfs:label "workflow (DMType)"@en .


###  sdc4:ExceptionalValueType/ev-name
<sdc4:ExceptionalValueType/ev-name> rdf:type owl:NamedIndividual ,
                                             sdc4-meta:ReferenceModelElement ;
                                    sdc4-meta:describesConceptualAspect sdc4-meta:ExceptionalValueName ;
                                    rdfs:comment "A short title or phase for the exceptional type value."@en ;
                                    rdfs:label "ev-name"@en .


###  sdc4:INVType/ev-name
<sdc4:INVType/ev-name> rdf:type owl:NamedIndividual ,
                                sdc4-meta:ReferenceModelElement ;
                       sdc4-meta:describesConceptualAspect sdc4-meta:ExceptionalValueName ;
                       rdfs:comment "Fixed value \"Invalid\" for INVType."@en ;
                       rdfs:label "ev-name (INV)"@en .


###  sdc4:InvlUnits/units-name
<sdc4:InvlUnits/units-name> rdf:type owl:NamedIndividual ,
                                     sdc4-meta:ReferenceModelElement ;
                            sdc4-meta:describesConceptualAspect sdc4-meta:UnitsName ;
                            rdfs:comment "The units name for an Interval."@en ;
                            rdfs:label "units-name"@en .


###  sdc4:InvlUnits/units-uri
<sdc4:InvlUnits/units-uri> rdf:type owl:NamedIndividual ,
                                    sdc4-meta:ReferenceModelElement ;
                           sdc4-meta:describesConceptualAspect sdc4-meta:UnitsURI ;
                           rdfs:comment "The units URI for an Interval."@en ;
                           rdfs:label "units-uri"@en .


###  sdc4:MSKType/ev-name
<sdc4:MSKType/ev-name> rdf:type owl:NamedIndividual ,
                                sdc4-meta:ReferenceModelElement ;
                       sdc4-meta:describesConceptualAspect sdc4-meta:ExceptionalValueName ;
                       rdfs:comment "Fixed value \"Masked\" for MSKType."@en ;
                       rdfs:label "ev-name (MSK)"@en .


###  sdc4:NASKType/ev-name
<sdc4:NASKType/ev-name> rdf:type owl:NamedIndividual ,
                                 sdc4-meta:ReferenceModelElement ;
                        sdc4-meta:describesConceptualAspect sdc4-meta:ExceptionalValueName ;
                        rdfs:comment "Fixed value \"Not Asked\" for NASKType."@en ;
                        rdfs:label "ev-name (NASK)"@en .


###  sdc4:NAType/ev-name
<sdc4:NAType/ev-name> rdf:type owl:NamedIndividual ,
                               sdc4-meta:ReferenceModelElement ;
                      sdc4-meta:describesConceptualAspect sdc4-meta:ExceptionalValueName ;
                      rdfs:comment "Fixed value \"Not Applicable\" for NAType."@en ;
                      rdfs:label "ev-name (NA)"@en .


###  sdc4:NAVType/ev-name
<sdc4:NAVType/ev-name> rdf:type owl:NamedIndividual ,
                                sdc4-meta:ReferenceModelElement ;
                       sdc4-meta:describesConceptualAspect sdc4-meta:ExceptionalValueName ;
                       rdfs:comment "Fixed value \"Not Available\" for NAVType."@en ;
                       rdfs:label "ev-name (NAV)"@en .


###  sdc4:NINFType/ev-name
<sdc4:NINFType/ev-name> rdf:type owl:NamedIndividual ,
                                 sdc4-meta:ReferenceModelElement ;
                        sdc4-meta:describesConceptualAspect sdc4-meta:ExceptionalValueName ;
                        rdfs:comment "Fixed value \"Negative Infinity\" for NINFType."@en ;
                        rdfs:label "ev-name (NINF)"@en .


###  sdc4:NIType/ev-name
<sdc4:NIType/ev-name> rdf:type owl:NamedIndividual ,
                               sdc4-meta:ReferenceModelElement ;
                      sdc4-meta:describesConceptualAspect sdc4-meta:ExceptionalValueName ;
                      rdfs:comment "Fixed value \"No Information\" for NIType."@en ;
                      rdfs:label "ev-name (NI)"@en .


###  sdc4:OTHType/ev-name
<sdc4:OTHType/ev-name> rdf:type owl:NamedIndividual ,
                                sdc4-meta:ReferenceModelElement ;
                       sdc4-meta:describesConceptualAspect sdc4-meta:ExceptionalValueName ;
                       rdfs:comment "Fixed value \"Other\" for OTHType."@en ;
                       rdfs:label "ev-name (OTH)"@en .


###  sdc4:PINFType/ev-name
<sdc4:PINFType/ev-name> rdf:type owl:NamedIndividual ,
                                 sdc4-meta:ReferenceModelElement ;
                        sdc4-meta:describesConceptualAspect sdc4-meta:ExceptionalValueName ;
                        rdfs:comment "Fixed value \"Positive Infinity\" for PINFType."@en ;
                        rdfs:label "ev-name (PINF)"@en .


###  sdc4:ParticipationType/end
<sdc4:ParticipationType/end> rdf:type owl:NamedIndividual ,
                                      sdc4-meta:ReferenceModelElement ;
                             sdc4-meta:describesConceptualAspect sdc4-meta:ParticipationEndTime ;
                             rdfs:comment "The ending datetime when the participation took place."@en ;
                             rdfs:label "end (ParticipationType)"@en .


###  sdc4:ParticipationType/function
<sdc4:ParticipationType/function> rdf:type owl:NamedIndividual ,
                                           sdc4-meta:ReferenceModelElement ;
                                  sdc4-meta:describesConceptualAspect sdc4-meta:ParticipationFunction ;
                                  rdfs:comment "The function of the performer in this participation."@en ;
                                  rdfs:label "function (ParticipationType)"@en .


###  sdc4:ParticipationType/label
<sdc4:ParticipationType/label> rdf:type owl:NamedIndividual ,
                                        sdc4-meta:ReferenceModelElement ;
                               sdc4-meta:describesConceptualAspect sdc4-meta:ParticipationLabel ;
                               rdfs:comment "Descriptive name of this datatype model for ParticipationType."@en ;
                               rdfs:label "label (ParticipationType)"@en .


###  sdc4:ParticipationType/mode
<sdc4:ParticipationType/mode> rdf:type owl:NamedIndividual ,
                                       sdc4-meta:ReferenceModelElement ;
                              sdc4-meta:describesConceptualAspect sdc4-meta:ParticipationMode ;
                              rdfs:comment "The mode of the performer / activity interaction."@en ;
                              rdfs:label "mode (ParticipationType)"@en .


###  sdc4:ParticipationType/performer
<sdc4:ParticipationType/performer> rdf:type owl:NamedIndividual ,
                                            sdc4-meta:ReferenceModelElement ;
                                   sdc4-meta:describesConceptualAspect sdc4-meta:ParticipationPerformer ;
                                   rdfs:comment "The id and possibly demographic system link of the party that represents the primary provider of services in the activity."@en ;
                                   rdfs:label "performer"@en .


###  sdc4:ParticipationType/start
<sdc4:ParticipationType/start> rdf:type owl:NamedIndividual ,
                                        sdc4-meta:ReferenceModelElement ;
                               sdc4-meta:describesConceptualAspect sdc4-meta:ParticipationStartTime ;
                               rdfs:comment "The beginning datetime when the participation took place."@en ;
                               rdfs:label "start (ParticipationType)"@en .


###  sdc4:PartyType/label
<sdc4:PartyType/label> rdf:type owl:NamedIndividual ,
                                sdc4-meta:ReferenceModelElement ;
                       sdc4-meta:describesConceptualAspect sdc4-meta:PartyLabel ;
                       rdfs:comment "Descriptive name of this datatype model for PartyType."@en ;
                       rdfs:label "label (PartyType)"@en .


###  sdc4:PartyType/party-details
<sdc4:PartyType/party-details> rdf:type owl:NamedIndividual ,
                                        sdc4-meta:ReferenceModelElement ;
                               sdc4-meta:describesConceptualAspect sdc4-meta:PartyDetails ;
                               rdfs:comment "A structured element for details about the party."@en ;
                               rdfs:label "party-details"@en .


###  sdc4:PartyType/party-name
<sdc4:PartyType/party-name> rdf:type owl:NamedIndividual ,
                                     sdc4-meta:ReferenceModelElement ;
                            sdc4-meta:describesConceptualAspect sdc4-meta:PartyName ;
                            rdfs:comment "Optional human-readable name (in String form) of the party."@en ;
                            rdfs:label "party-name"@en .


###  sdc4:PartyType/party-ref
<sdc4:PartyType/party-ref> rdf:type owl:NamedIndividual ,
                                    sdc4-meta:ReferenceModelElement ;
                           sdc4-meta:describesConceptualAspect sdc4-meta:PartyReference ;
                           rdfs:comment "Optional reference to more detailed demographic or identification information for this party."@en ;
                           rdfs:label "party-ref"@en .


###  sdc4:QSType/ev-name
<sdc4:QSType/ev-name> rdf:type owl:NamedIndividual ,
                               sdc4-meta:ReferenceModelElement ;
                      sdc4-meta:describesConceptualAspect sdc4-meta:ExceptionalValueName ;
                      rdfs:comment "Fixed value \"Sufficient Quantity\" for QSType."@en ;
                      rdfs:label "ev-name (QS)"@en .


###  sdc4:ReferenceRangeType/definition
<sdc4:ReferenceRangeType/definition> rdf:type owl:NamedIndividual ,
                                              sdc4-meta:ReferenceModelElement ;
                                     sdc4-meta:describesConceptualAspect sdc4-meta:ReferenceRangeDefinitionTerm ;
                                     rdfs:comment "Term whose value indicates the meaning of this range, e.g. 'normal', 'critical', 'therapeutic'."@en ;
                                     rdfs:label "definition"@en .


###  sdc4:ReferenceRangeType/interval
<sdc4:ReferenceRangeType/interval> rdf:type owl:NamedIndividual ,
                                            sdc4-meta:ReferenceModelElement ;
                                   sdc4-meta:describesConceptualAspect sdc4-meta:ReferenceRangeInterval ;
                                   rdfs:comment "The data range for this reference range."@en ;
                                   rdfs:label "interval"@en .


###  sdc4:ReferenceRangeType/is-normal
<sdc4:ReferenceRangeType/is-normal> rdf:type owl:NamedIndividual ,
                                             sdc4-meta:ReferenceModelElement ;
                                    sdc4-meta:describesConceptualAspect sdc4-meta:ReferenceRangeIsNormal ;
                                    rdfs:comment "True if this reference range defines values that are considered to be normal."@en ;
                                    rdfs:label "is-normal"@en .


###  sdc4:TRCType/ev-name
<sdc4:TRCType/ev-name> rdf:type owl:NamedIndividual ,
                                sdc4-meta:ReferenceModelElement ;
                       sdc4-meta:describesConceptualAspect sdc4-meta:ExceptionalValueName ;
                       rdfs:comment "Fixed value \"Trace\" for TRCType."@en ;
                       rdfs:label "ev-name (TRC)"@en .


###  sdc4:UNCType/ev-name
<sdc4:UNCType/ev-name> rdf:type owl:NamedIndividual ,
                                sdc4-meta:ReferenceModelElement ;
                       sdc4-meta:describesConceptualAspect sdc4-meta:ExceptionalValueName ;
                       rdfs:comment "Fixed value \"Unencoded\" for UNCType."@en ;
                       rdfs:label "ev-name (UNC)"@en .


###  sdc4:UNKType/ev-name
<sdc4:UNKType/ev-name> rdf:type owl:NamedIndividual ,
                                sdc4-meta:ReferenceModelElement ;
                       sdc4-meta:describesConceptualAspect sdc4-meta:ExceptionalValueName ;
                       rdfs:comment "Fixed value \"Unknown\" for UNKType."@en ;
                       rdfs:label "ev-name (UNK)"@en .


###  sdc4:XdAdapterType/XdAdapter-value
<sdc4:XdAdapterType/XdAdapter-value> rdf:type owl:NamedIndividual ,
                                              sdc4-meta:ReferenceModelElement ;
                                     sdc4-meta:describesConceptualAspect sdc4-meta:AdaptedValue ;
                                     rdfs:comment "Data value type of this leaf. By rule, there must only be one XdAnyType subtype defined here."@en ;
                                     rdfs:label "XdAdapter-value"@en .


###  sdc4:XdAnyType/act
<sdc4:XdAnyType/act> rdf:type owl:NamedIndividual ,
                              sdc4-meta:ReferenceModelElement ;
                     sdc4-meta:describesConceptualAspect sdc4-meta:AccessControlTag ;
                     rdfs:comment "Access Control Tag. If this is used it must contain a valid term from the Access Control System."@en ;
                     rdfs:label "act"@en .


###  sdc4:XdAnyType/label
<sdc4:XdAnyType/label> rdf:type owl:NamedIndividual ,
                                sdc4-meta:ReferenceModelElement ;
                       sdc4-meta:describesConceptualAspect sdc4-meta:ConceptualEntityIdentity ;
                       rdfs:comment "The 'label' element within XdAnyType and its subtypes, which defines the conceptual entity."@en ;
                       rdfs:label "label"@en .


###  sdc4:XdAnyType/latitude
<sdc4:XdAnyType/latitude> rdf:type owl:NamedIndividual ,
                                   sdc4-meta:ReferenceModelElement ;
                          sdc4-meta:describesConceptualAspect sdc4-meta:GeospatialLatitude ;
                          rdfs:comment "Latitude in decimal format."@en ;
                          rdfs:label "latitude"@en .


###  sdc4:XdAnyType/longitude
<sdc4:XdAnyType/longitude> rdf:type owl:NamedIndividual ,
                                    sdc4-meta:ReferenceModelElement ;
                           sdc4-meta:describesConceptualAspect sdc4-meta:GeospatialLongitude ;
                           rdfs:comment "Longitude in decimal format."@en ;
                           rdfs:label "longitude"@en .


###  sdc4:XdAnyType/modified
<sdc4:XdAnyType/modified> rdf:type owl:NamedIndividual ,
                                   sdc4-meta:ReferenceModelElement ;
                          sdc4-meta:describesConceptualAspect sdc4-meta:TimeModified ;
                          rdfs:comment "Time Modified. Indicates the actual date and time the data was last changed."@en ;
                          rdfs:label "modified"@en .


###  sdc4:XdAnyType/tr
<sdc4:XdAnyType/tr> rdf:type owl:NamedIndividual ,
                             sdc4-meta:ReferenceModelElement ;
                    sdc4-meta:describesConceptualAspect sdc4-meta:TimeRecorded ;
                    rdfs:comment "Time Recorded. Indicates the actual date and time the data was recorded."@en ;
                    rdfs:label "tr"@en .


###  sdc4:XdAnyType/vtb
<sdc4:XdAnyType/vtb> rdf:type owl:NamedIndividual ,
                              sdc4-meta:ReferenceModelElement ;
                     sdc4-meta:describesConceptualAspect sdc4-meta:ValidTimeBeginning ;
                     rdfs:comment "Valid Time Begin. Indicates the beginning time that information is considered valid."@en ;
                     rdfs:label "vtb"@en .


###  sdc4:XdAnyType/vte
<sdc4:XdAnyType/vte> rdf:type owl:NamedIndividual ,
                              sdc4-meta:ReferenceModelElement ;
                     sdc4-meta:describesConceptualAspect sdc4-meta:ValidTimeEnd ;
                     rdfs:comment "Valid Time End. Indicates the ending time that information is considered valid or expired."@en ;
                     rdfs:label "vte"@en .


###  sdc4:XdBooleanListType/xdbooleanlist-value
<sdc4:XdBooleanListType/xdbooleanlist-value> rdf:type owl:NamedIndividual ,
                                                      sdc4-meta:ReferenceModelElement .


###  sdc4:XdBooleanType/false-value
<sdc4:XdBooleanType/false-value> rdf:type owl:NamedIndividual ,
                                          sdc4-meta:ReferenceModelElement ;
                                 sdc4-meta:describesConceptualAspect sdc4-meta:BooleanFalseValue ;
                                 rdfs:comment "A string that represents a boolean False in the implementation."@en ;
                                 rdfs:label "false-value"@en .


###  sdc4:XdBooleanType/true-value
<sdc4:XdBooleanType/true-value> rdf:type owl:NamedIndividual ,
                                         sdc4-meta:ReferenceModelElement ;
                                sdc4-meta:describesConceptualAspect sdc4-meta:BooleanTrueValue ;
                                rdfs:comment "A string that represents a boolean True in the implementation."@en ;
                                rdfs:label "true-value"@en .


###  sdc4:XdCountType/xdcount-units
<sdc4:XdCountType/xdcount-units> rdf:type owl:NamedIndividual ,
                                          sdc4-meta:ReferenceModelElement ;
                                 sdc4-meta:describesConceptualAspect sdc4-meta:CountUnits ;
                                 rdfs:comment "The name or type of the items counted."@en ;
                                 rdfs:label "xdcount-units"@en .


###  sdc4:XdCountType/xdcount-value
<sdc4:XdCountType/xdcount-value> rdf:type owl:NamedIndividual ,
                                          sdc4-meta:ReferenceModelElement ;
                                 sdc4-meta:describesConceptualAspect sdc4-meta:CountValue ;
                                 rdfs:comment "Integer value of the counted items."@en ;
                                 rdfs:label "xdcount-value"@en .


###  sdc4:XdDecimalListType/xddecimallist-value
<sdc4:XdDecimalListType/xddecimallist-value> rdf:type owl:NamedIndividual ,
                                                      sdc4-meta:ReferenceModelElement .


###  sdc4:XdDoubleListType/xddoublelist-value
<sdc4:XdDoubleListType/xddoublelist-value> rdf:type owl:NamedIndividual ,
                                                    sdc4-meta:ReferenceModelElement .


###  sdc4:XdDoubleType/xddouble-units
<sdc4:XdDoubleType/xddouble-units> rdf:type owl:NamedIndividual ,
                                            sdc4-meta:ReferenceModelElement ;
                                   sdc4-meta:describesConceptualAspect sdc4-meta:DoubleUnits ;
                                   rdfs:comment "The name or type of the double value."@en ;
                                   rdfs:label "xddouble-units"@en .


###  sdc4:XdDoubleType/xddouble-value
<sdc4:XdDoubleType/xddouble-value> rdf:type owl:NamedIndividual ,
                                            sdc4-meta:ReferenceModelElement ;
                                   sdc4-meta:describesConceptualAspect sdc4-meta:DoubleValue ;
                                   rdfs:comment "Double value."@en ;
                                   rdfs:label "xddouble-value"@en .


###  sdc4:XdFileType/alt-txt
<sdc4:XdFileType/alt-txt> rdf:type owl:NamedIndividual ,
                                   sdc4-meta:ReferenceModelElement ;
                          sdc4-meta:describesConceptualAspect sdc4-meta:FileAltText ;
                          rdfs:comment "Text to display in lieu of multimedia display or execution."@en ;
                          rdfs:label "alt-txt"@en .


###  sdc4:XdFileType/compression-type
<sdc4:XdFileType/compression-type> rdf:type owl:NamedIndividual ,
                                            sdc4-meta:ReferenceModelElement ;
                                   sdc4-meta:describesConceptualAspect sdc4-meta:FileCompressionType ;
                                   rdfs:comment "Compression/archiving mime-type."@en ;
                                   rdfs:label "compression-type"@en .


###  sdc4:XdFileType/encoding
<sdc4:XdFileType/encoding> rdf:type owl:NamedIndividual ,
                                    sdc4-meta:ReferenceModelElement ;
                           sdc4-meta:describesConceptualAspect sdc4-meta:FileEncoding ;
                           rdfs:comment "Name of character encoding scheme in which this value is encoded."@en ;
                           rdfs:label "encoding"@en .


###  sdc4:XdFileType/formalism
<sdc4:XdFileType/formalism> rdf:type owl:NamedIndividual ,
                                     sdc4-meta:ReferenceModelElement ;
                            sdc4-meta:describesConceptualAspect sdc4-meta:FileFormalism ;
                            rdfs:comment "Name of the formalism or syntax used to inform an application regarding a candidate parser to use on the content."@en ;
                            rdfs:label "formalism"@en .


###  sdc4:XdFileType/hash-function
<sdc4:XdFileType/hash-function> rdf:type owl:NamedIndividual ,
                                         sdc4-meta:ReferenceModelElement ;
                                sdc4-meta:describesConceptualAspect sdc4-meta:FileHashFunction ;
                                rdfs:comment "Hash function used to compute hash-result."@en ;
                                rdfs:label "hash-function"@en .


###  sdc4:XdFileType/hash-result
<sdc4:XdFileType/hash-result> rdf:type owl:NamedIndividual ,
                                       sdc4-meta:ReferenceModelElement ;
                              sdc4-meta:describesConceptualAspect sdc4-meta:FileHashResult ;
                              rdfs:comment "Hash function result of the 'media-content'."@en ;
                              rdfs:label "hash-result"@en .


###  sdc4:XdFileType/media-content
<sdc4:XdFileType/media-content> rdf:type owl:NamedIndividual ,
                                         sdc4-meta:ReferenceModelElement ;
                                sdc4-meta:describesConceptualAspect sdc4-meta:FileMediaContent ;
                                rdfs:comment "The content, if stored locally."@en ;
                                rdfs:label "media-content"@en .


###  sdc4:XdFileType/media-type
<sdc4:XdFileType/media-type> rdf:type owl:NamedIndividual ,
                                      sdc4-meta:ReferenceModelElement ;
                             sdc4-meta:describesConceptualAspect sdc4-meta:FileMediaType ;
                             rdfs:comment "Media (MIME) type of the original media-content w/o any compression."@en ;
                             rdfs:label "media-type"@en .


###  sdc4:XdFileType/size
<sdc4:XdFileType/size> rdf:type owl:NamedIndividual ,
                                sdc4-meta:ReferenceModelElement ;
                       sdc4-meta:describesConceptualAspect sdc4-meta:FileSize ;
                       rdfs:comment "Original size in bytes of unencoded encapsulated data."@en ;
                       rdfs:label "size"@en .


###  sdc4:XdFileType/uri
<sdc4:XdFileType/uri> rdf:type owl:NamedIndividual ,
                               sdc4-meta:ReferenceModelElement ;
                      sdc4-meta:describesConceptualAspect sdc4-meta:FileURI ;
                      rdfs:comment "URI reference to electronic information stored outside the record as a file, database entry etc, if supplied as a reference."@en ;
                      rdfs:label "uri"@en .


###  sdc4:XdFileType/xdfile-language
<sdc4:XdFileType/xdfile-language> rdf:type owl:NamedIndividual ,
                                           sdc4-meta:ReferenceModelElement ;
                                  sdc4-meta:describesConceptualAspect sdc4-meta:LanguageCode ;
                                  rdfs:comment "Optional indicator of the localised language of the content."@en ;
                                  rdfs:label "xdfile-language"@en .


###  sdc4:XdFloatType/xdfloat-units
<sdc4:XdFloatType/xdfloat-units> rdf:type owl:NamedIndividual ,
                                          sdc4-meta:ReferenceModelElement ;
                                 sdc4-meta:describesConceptualAspect sdc4-meta:FloatUnits ;
                                 rdfs:comment "The name or type of the float value."@en ;
                                 rdfs:label "xdfloat-units"@en .


###  sdc4:XdFloatType/xdfloat-value
<sdc4:XdFloatType/xdfloat-value> rdf:type owl:NamedIndividual ,
                                          sdc4-meta:ReferenceModelElement ;
                                 sdc4-meta:describesConceptualAspect sdc4-meta:FloatValue ;
                                 rdfs:comment "Float value."@en ;
                                 rdfs:label "xdfloat-value"@en .


###  sdc4:XdIntegerListType/xdintegerlist-value
<sdc4:XdIntegerListType/xdintegerlist-value> rdf:type owl:NamedIndividual ,
                                                      sdc4-meta:ReferenceModelElement .


###  sdc4:XdIntervalType/interval-units
<sdc4:XdIntervalType/interval-units> rdf:type owl:NamedIndividual ,
                                              sdc4-meta:ReferenceModelElement ;
                                     sdc4-meta:describesConceptualAspect sdc4-meta:IntervalUnitsDefinition ;
                                     rdfs:comment "The units designation for an Interval."@en ;
                                     rdfs:label "interval-units"@en .


###  sdc4:XdIntervalType/lower
<sdc4:XdIntervalType/lower> rdf:type owl:NamedIndividual ,
                                     sdc4-meta:ReferenceModelElement ;
                            sdc4-meta:describesConceptualAspect sdc4-meta:IntervalLowerBound ;
                            rdfs:comment "The lower boundary of the interval."@en ;
                            rdfs:label "lower"@en .


###  sdc4:XdIntervalType/lower_bounded
<sdc4:XdIntervalType/lower_bounded> rdf:type owl:NamedIndividual ,
                                             sdc4-meta:ReferenceModelElement ;
                                    sdc4-meta:describesConceptualAspect sdc4-meta:IntervalLowerBounded ;
                                    rdfs:comment "True if the interval has a lower bound."@en ;
                                    rdfs:label "lower_bounded"@en .


###  sdc4:XdIntervalType/lower_included
<sdc4:XdIntervalType/lower_included> rdf:type owl:NamedIndividual ,
                                              sdc4-meta:ReferenceModelElement ;
                                     sdc4-meta:describesConceptualAspect sdc4-meta:IntervalLowerIncluded ;
                                     rdfs:comment "True if the lower boundary is included in the interval."@en ;
                                     rdfs:label "lower_included"@en .


###  sdc4:XdIntervalType/upper
<sdc4:XdIntervalType/upper> rdf:type owl:NamedIndividual ,
                                     sdc4-meta:ReferenceModelElement ;
                            sdc4-meta:describesConceptualAspect sdc4-meta:IntervalUpperBound ;
                            rdfs:comment "The upper boundary of the interval."@en ;
                            rdfs:label "upper"@en .


###  sdc4:XdIntervalType/upper_bounded
<sdc4:XdIntervalType/upper_bounded> rdf:type owl:NamedIndividual ,
                                             sdc4-meta:ReferenceModelElement ;
                                    sdc4-meta:describesConceptualAspect sdc4-meta:IntervalUpperBounded ;
                                    rdfs:comment "True if the interval has an upper bound."@en ;
                                    rdfs:label "upper_bounded"@en .


###  sdc4:XdIntervalType/upper_included
<sdc4:XdIntervalType/upper_included> rdf:type owl:NamedIndividual ,
                                              sdc4-meta:ReferenceModelElement ;
                                     sdc4-meta:describesConceptualAspect sdc4-meta:IntervalUpperIncluded ;
                                     rdfs:comment "True if the upper boundary is included in the interval."@en ;
                                     rdfs:label "upper_included"@en .


###  sdc4:XdLinkType/link
<sdc4:XdLinkType/link> rdf:type owl:NamedIndividual ,
                                sdc4-meta:ReferenceModelElement ;
                       sdc4-meta:describesConceptualAspect sdc4-meta:LinkTargetURI ;
                       rdfs:comment "A dereferenceable (or not) URL to another CMC or other model like entity."@en ;
                       rdfs:label "link"@en .


###  sdc4:XdLinkType/relation
<sdc4:XdLinkType/relation> rdf:type owl:NamedIndividual ,
                                    sdc4-meta:ReferenceModelElement ;
                           sdc4-meta:describesConceptualAspect sdc4-meta:LinkRelationTerm ;
                           rdfs:comment "A required term, normally drawn from a vocabulary or ontology such as the OBO RO."@en ;
                           rdfs:label "relation"@en .


###  sdc4:XdLinkType/relation-uri
<sdc4:XdLinkType/relation-uri> rdf:type owl:NamedIndividual ,
                                        sdc4-meta:ReferenceModelElement ;
                               sdc4-meta:describesConceptualAspect sdc4-meta:LinkRelationURI ;
                               rdfs:comment "A URI where the definition of the relation element term can be found."@en ;
                               rdfs:label "relation-uri"@en .


###  sdc4:XdNonNegativeIntegerListType/xdnonnegativeintegerlist-value
<sdc4:XdNonNegativeIntegerListType/xdnonnegativeintegerlist-value> rdf:type owl:NamedIndividual ,
                                                                            sdc4-meta:ReferenceModelElement .


###  sdc4:XdOrderedType/normal-status
<sdc4:XdOrderedType/normal-status> rdf:type owl:NamedIndividual ,
                                            sdc4-meta:ReferenceModelElement ;
                                   sdc4-meta:describesConceptualAspect sdc4-meta:NormalStatusIndicator ;
                                   rdfs:comment "Optional normal status indicator of value with respect to normal range for this value."@en ;
                                   rdfs:label "normal-status"@en .


###  sdc4:XdOrdinalType/ordinal
<sdc4:XdOrdinalType/ordinal> rdf:type owl:NamedIndividual ,
                                      sdc4-meta:ReferenceModelElement ;
                             sdc4-meta:describesConceptualAspect sdc4-meta:OrdinalValue ;
                             rdfs:comment "Value in ordered enumeration of values."@en ;
                             rdfs:label "ordinal"@en .


###  sdc4:XdOrdinalType/symbol
<sdc4:XdOrdinalType/symbol> rdf:type owl:NamedIndividual ,
                                     sdc4-meta:ReferenceModelElement ;
                            sdc4-meta:describesConceptualAspect sdc4-meta:OrdinalSymbol ;
                            rdfs:comment "Coded textual representation of this value in the enumeration."@en ;
                            rdfs:label "symbol"@en .


###  sdc4:XdPositiveIntegerListType/xdpositiveintegerlist-value
<sdc4:XdPositiveIntegerListType/xdpositiveintegerlist-value> rdf:type owl:NamedIndividual ,
                                                                      sdc4-meta:ReferenceModelElement .


###  sdc4:XdQuantifiedType/accuracy_margin
<sdc4:XdQuantifiedType/accuracy_margin> rdf:type owl:NamedIndividual ,
                                                 sdc4-meta:ReferenceModelElement ;
                                        sdc4-meta:describesConceptualAspect sdc4-meta:AccuracyMargin ;
                                        rdfs:comment "Models ACCURACY. Defines the margin of systematic error."@en ;
                                        rdfs:label "accuracy_margin"@en .


###  sdc4:XdQuantifiedType/magnitude-status
<sdc4:XdQuantifiedType/magnitude-status> rdf:type owl:NamedIndividual ,
                                                  sdc4-meta:ReferenceModelElement ;
                                         sdc4-meta:describesConceptualAspect sdc4-meta:MagnitudeStatusIndicator ;
                                         rdfs:comment "An optional status that describes the relationship of this quantity's value to a contextual target or expected value."@en ;
                                         rdfs:label "magnitude-status"@en .


###  sdc4:XdQuantifiedType/precision_digits
<sdc4:XdQuantifiedType/precision_digits> rdf:type owl:NamedIndividual ,
                                                  sdc4-meta:ReferenceModelElement ;
                                         sdc4-meta:describesConceptualAspect sdc4-meta:PrecisionDigits ;
                                         rdfs:comment "Models PRECISION. Defines the resolution of the measurement by specifying the number of significant digits after the decimal point."@en ;
                                         rdfs:label "precision_digits"@en .


###  sdc4:XdQuantityType/xdquantity-units
<sdc4:XdQuantityType/xdquantity-units> rdf:type owl:NamedIndividual ,
                                                sdc4-meta:ReferenceModelElement ;
                                       sdc4-meta:describesConceptualAspect sdc4-meta:QuantityUnits ;
                                       rdfs:comment "The name or type of the quantity."@en ;
                                       rdfs:label "xdquantity-units"@en .


###  sdc4:XdQuantityType/xdquantity-value
<sdc4:XdQuantityType/xdquantity-value> rdf:type owl:NamedIndividual ,
                                                sdc4-meta:ReferenceModelElement ;
                                       sdc4-meta:describesConceptualAspect sdc4-meta:QuantityValue ;
                                       rdfs:comment "Numeric decimal value of the quantity."@en ;
                                       rdfs:label "xdquantity-value"@en .


###  sdc4:XdStringListType/xdstringlist-value
<sdc4:XdStringListType/xdstringlist-value> rdf:type owl:NamedIndividual ,
                                                    sdc4-meta:ReferenceModelElement .


###  sdc4:XdStringType/xdstring-language
<sdc4:XdStringType/xdstring-language> rdf:type owl:NamedIndividual ,
                                               sdc4-meta:ReferenceModelElement ;
                                      sdc4-meta:describesConceptualAspect sdc4-meta:LanguageCode ;
                                      rdfs:comment "Optional indicator of the localised language in which this data-type is written."@en ;
                                      rdfs:label "xdstring-language"@en .


###  sdc4:XdStringType/xdstring-value
<sdc4:XdStringType/xdstring-value> rdf:type owl:NamedIndividual ,
                                            sdc4-meta:ReferenceModelElement ;
                                   sdc4-meta:describesConceptualAspect sdc4-meta:ConceptualValue ;
                                   rdfs:comment "The string value of the item."@en ;
                                   rdfs:label "xdstring-value"@en .


###  sdc4:XdTemporalType/xdtemporal-date
<sdc4:XdTemporalType/xdtemporal-date> rdf:type owl:NamedIndividual ,
                                               sdc4-meta:ReferenceModelElement ;
                                      sdc4-meta:describesConceptualAspect sdc4-meta:TemporalDate ;
                                      rdfs:comment "Represents a specific calendar date (YYYY-MM-DD), with an optional timezone."@en ;
                                      rdfs:label "xdtemporal-date"@en .


###  sdc4:XdTemporalType/xdtemporal-datetime
<sdc4:XdTemporalType/xdtemporal-datetime> rdf:type owl:NamedIndividual ,
                                                   sdc4-meta:ReferenceModelElement ;
                                          sdc4-meta:describesConceptualAspect sdc4-meta:TemporalDateTime ;
                                          rdfs:comment "Represents a specific instant in time (YYYY-MM-DDThh:mm:ss.sss), with an optional timezone."@en ;
                                          rdfs:label "xdtemporal-datetime"@en .


###  sdc4:XdTemporalType/xdtemporal-day
<sdc4:XdTemporalType/xdtemporal-day> rdf:type owl:NamedIndividual ,
                                              sdc4-meta:ReferenceModelElement ;
                                     sdc4-meta:describesConceptualAspect sdc4-meta:TemporalDay ;
                                     rdfs:comment "Represents a recurring Gregorian day (---DD)."@en ;
                                     rdfs:label "xdtemporal-day"@en .


###  sdc4:XdTemporalType/xdtemporal-duration
<sdc4:XdTemporalType/xdtemporal-duration> rdf:type owl:NamedIndividual ,
                                                   sdc4-meta:ReferenceModelElement ;
                                          sdc4-meta:describesConceptualAspect sdc4-meta:TemporalDuration ;
                                          rdfs:comment "Represents a duration of time as defined by ISO 8601 (e.g., P1Y2M3D)."@en ;
                                          rdfs:label "xdtemporal-duration"@en .


###  sdc4:XdTemporalType/xdtemporal-month
<sdc4:XdTemporalType/xdtemporal-month> rdf:type owl:NamedIndividual ,
                                                sdc4-meta:ReferenceModelElement ;
                                       sdc4-meta:describesConceptualAspect sdc4-meta:TemporalMonth ;
                                       rdfs:comment "Represents a recurring Gregorian month (--MM--)."@en ;
                                       rdfs:label "xdtemporal-month"@en .


###  sdc4:XdTemporalType/xdtemporal-month-day
<sdc4:XdTemporalType/xdtemporal-month-day> rdf:type owl:NamedIndividual ,
                                                    sdc4-meta:ReferenceModelElement ;
                                           sdc4-meta:describesConceptualAspect sdc4-meta:TemporalMonthDay ;
                                           rdfs:comment "Represents a recurring Gregorian day in a recurring month (--MM-DD)."@en ;
                                           rdfs:label "xdtemporal-month-day"@en .


###  sdc4:XdTemporalType/xdtemporal-time
<sdc4:XdTemporalType/xdtemporal-time> rdf:type owl:NamedIndividual ,
                                               sdc4-meta:ReferenceModelElement ;
                                      sdc4-meta:describesConceptualAspect sdc4-meta:TemporalTime ;
                                      rdfs:comment "Represents a recurring time of day (hh:mm:ss.sss), with an optional timezone."@en ;
                                      rdfs:label "xdtemporal-time"@en .


###  sdc4:XdTemporalType/xdtemporal-year
<sdc4:XdTemporalType/xdtemporal-year> rdf:type owl:NamedIndividual ,
                                               sdc4-meta:ReferenceModelElement ;
                                      sdc4-meta:describesConceptualAspect sdc4-meta:TemporalYear ;
                                      rdfs:comment "Represents a specific Gregorian calendar year (YYYY)."@en ;
                                      rdfs:label "xdtemporal-year"@en .


###  sdc4:XdTemporalType/xdtemporal-year-month
<sdc4:XdTemporalType/xdtemporal-year-month> rdf:type owl:NamedIndividual ,
                                                     sdc4-meta:ReferenceModelElement ;
                                            sdc4-meta:describesConceptualAspect sdc4-meta:TemporalYearMonth ;
                                            rdfs:comment "Represents a specific Gregorian month in a specific year (YYYY-MM)."@en ;
                                            rdfs:label "xdtemporal-year-month"@en .


###  sdc4:XdTokenListType/xdtokenlist-value
<sdc4:XdTokenListType/xdtokenlist-value> rdf:type owl:NamedIndividual ,
                                                  sdc4-meta:ReferenceModelElement .


#################################################################
#    Annotations
#################################################################

sdc4-meta:hasConceptualLabelValue rdfs:comment "Holds the literal string value of the conceptual entity's label (e.g., \"City\")."@en ;
                                  rdfs:label "has conceptual label value"@en .


<sdc4:ASKRType> rdfs:comment "Asked and Refused : Information was sought but refused to be provided."@en ;
                rdfs:label "ASKRType"@en .


<sdc4:ASKUType> rdfs:comment "Asked but Unknown : Information was sought but not found."@en ;
                rdfs:label "ASKUType"@en .


<sdc4:ClusterType> rdfs:comment "The grouping component, which may contain further instances of itself or any eXtended datatype, in an ordered list."@en ;
                   rdfs:label "ClusterType"@en .


<sdc4:DERType> rdfs:comment "Derived : An actual value may exist, but it must be derived from the provided information."@en ;
               rdfs:label "DERType"@en .


<sdc4:ExceptionalValueType> rdfs:comment "Subtypes are used to indicate why a value is missing (Null) or is outside a measurable range."@en ;
                            rdfs:label "ExceptionalValueType"@en .


<sdc4:INVType> rdfs:comment "Invalid : The value as represented in the instance is not a member of the set of permitted data values in the constrained value domain of a variable."@en ;
               rdfs:label "INVType"@en .


<sdc4:ItemType> rdfs:comment "The abstract parent of ClusterType and XdAdapterType structural representation types."@en ;
                rdfs:label "ItemType"@en .


<sdc4:MSKType> rdfs:comment "Masked : There is information on this item available but it has not been provided by the sender due to security, privacy or other reasons."@en ;
               rdfs:label "MSKType"@en .


<sdc4:NASKType> rdfs:comment "Not Asked : This information has not been sought."@en ;
                rdfs:label "NASKType"@en .


<sdc4:NAType> rdfs:comment "Not Applicable : No proper value is applicable in this context."@en ;
              rdfs:label "NAType"@en .


<sdc4:NAVType> rdfs:comment "Not Available: This information is not available and the specific reason is not known."@en ;
               rdfs:label "NAVType"@en .


<sdc4:NINFType> rdfs:comment "Negative Infinity : Negative infinity of numbers"@en ;
                rdfs:label "NINFType"@en .


<sdc4:NIType> rdfs:comment "No Information : The value is exceptional (missing, omitted, incomplete, improper)."@en ;
              rdfs:label "NIType"@en .


<sdc4:OTHType> rdfs:comment "Other: The actual value is not a member of the permitted data values in the variable."@en ;
               rdfs:label "OTHType"@en .


<sdc4:PINFType> rdfs:comment "Positive Infinity : Positive infinity of numbers"@en ;
                rdfs:label "PINFType"@en .


<sdc4:QSType> rdfs:comment "Sufficient Quantity : The specific quantity is not known, but is known to non-zero and it makes up the bulk of the material."@en ;
              rdfs:label "QSType"@en .


<sdc4:ReferenceRangeType> rdfs:comment "Defines a named range to be associated with any ORDERED datatype."@en ;
                          rdfs:label "ReferenceRangeType"@en .


<sdc4:TRCType> rdfs:comment "Trace : The content is greater or less than zero but too small to be quantified."@en ;
               rdfs:label "TRCType"@en .


<sdc4:UNCType> rdfs:comment "Unencoded : No attempt has been made to encode the information correctly but the raw source information is represented."@en ;
               rdfs:label "UNCType"@en .


<sdc4:UNKType> rdfs:comment "Unknown : A proper value is applicable, but not known."@en ;
               rdfs:label "UNKType"@en .


<sdc4:XdAdapterType> rdfs:comment "The leaf variant of Item, to which any XdAnyType subtype instance is attached for use in a Cluster."@en ;
                     rdfs:label "XdAdapterType"@en .


<sdc4:XdAnyType> rdfs:comment "Serves as the common ancestor of all eXtended data-types (Xd*) in Semantic Data Charter."@en ;
                 rdfs:label "XdAnyType"@en .


<sdc4:XdBooleanType> rdfs:comment "An enumerated type which represents boolean decisions."@en ;
                     rdfs:label "XdBooleanType"@en .


<sdc4:XdCountType> rdfs:comment "Countable quantities. Used for countable types such as pregnancies and steps."@en ;
                   rdfs:label "XdCountType"@en .


<sdc4:XdDoubleType> rdfs:comment "Quantified type representing specific a value as a 64 bit number and optional units."@en ;
                    rdfs:label "XdDoubleType"@en .


<sdc4:XdFileType> rdfs:comment "A type to use for encapsulated content (aka. files) for image, audio and other media types with a defined MIME type."@en ;
                  rdfs:label "XdFileType"@en .


<sdc4:XdFloatType> rdfs:comment "Quantified type representing specific a value as a floating point (32 bit) number and optional units."@en ;
                   rdfs:label "XdFloatType"@en .


<sdc4:XdIntervalType> rdfs:comment "A generic type for defining an interval (i.e., range) of ordered values."@en ;
                      rdfs:label "XdIntervalType"@en .


<sdc4:XdLinkType> rdfs:comment "Used to specify a Universal Resource Identifier."@en ;
                  rdfs:label "XdLinkType"@en .


<sdc4:XdOrderedType> rdfs:comment "Abstract type defining the concept of ordered values, which includes ordinals as well as true quantities."@en ;
                     rdfs:label "XdOrderedType"@en .


<sdc4:XdOrdinalType> rdfs:comment "Models rankings and scores, e.g., pain, Apgar values, educational level, and the Likert Scale."@en ;
                     rdfs:label "XdOrdinalType"@en .


<sdc4:XdQuantifiedType> rdfs:comment "Abstract type defining the concept of true quantified values, i.e. values which are not only ordered, but which have a precise magnitude."@en ;
                        rdfs:label "XdQuantifiedType"@en .


<sdc4:XdQuantityType> rdfs:comment "Quantified type representing specific quantities, i.e. quantities expressed as a magnitude and units."@en ;
                      rdfs:label "XdQuantityType"@en .


<sdc4:XdStringType> rdfs:comment "The string data type can contain characters, line feeds, carriage returns, and tab characters."@en ;
                    rdfs:label "XdStringType"@en .


<sdc4:XdTemporalType> rdfs:comment "Type defining a temporal value. It allows for varying levels of precision."@en ;
                      rdfs:label "XdTemporalType"@en .


###  Generated by the OWL API (version 4.5.29.2024-05-13T12:11:03Z) https://github.com/owlcs/owlapi
