@prefix : <https://semanticdatacharter.com/ns/sdc4#> .
@prefix owl: <http://www.w3.org/2002/07/owl#> .
@prefix rdf: <http://www.w3.org/1999/02/22-rdf-syntax-ns#> .
@prefix xml: <http://www.w3.org/XML/1998/namespace> .
@prefix xsd: <http://www.w3.org/2001/XMLSchema#> .
@prefix rdfs: <http://www.w3.org/2000/01/rdf-schema#> .
@prefix sdc4: <https://semanticdatacharter.com/ns/sdc4/> .
@base <https://semanticdatacharter.com/ns/sdc4#> .

<https://semanticdatacharter.com/ns/sdc4/> rdf:type owl:Ontology ;
                                                rdfs:comment "This work is Copyright 2016 - 2026 Axius-SDC, Inc., All Rights Reserved. This ontology represents the Semantic Data Charter (SDC4) Reference Model (RM). It defines the classes and properties for building SDC4-compliant data models."@en-us ;
                                                rdfs:label "Semantic Data Charter (SDC4) Release 4.0.0; Reference Model Ontology"@en-us ;
                                                owl:versionInfo "4.0.0" .

#################################################################
#    Datatypes
#################################################################

###  http://www.w3.org/2001/XMLSchema#date
xsd:date rdf:type rdfs:Datatype .


###  http://www.w3.org/2001/XMLSchema#duration
xsd:duration rdf:type rdfs:Datatype .


###  http://www.w3.org/2001/XMLSchema#gDay
xsd:gDay rdf:type rdfs:Datatype .


###  http://www.w3.org/2001/XMLSchema#gMonth
xsd:gMonth rdf:type rdfs:Datatype .


###  http://www.w3.org/2001/XMLSchema#gMonthDay
xsd:gMonthDay rdf:type rdfs:Datatype .


###  http://www.w3.org/2001/XMLSchema#gYear
xsd:gYear rdf:type rdfs:Datatype .


###  http://www.w3.org/2001/XMLSchema#gYearMonth
xsd:gYearMonth rdf:type rdfs:Datatype .


###  http://www.w3.org/2001/XMLSchema#time
xsd:time rdf:type rdfs:Datatype .


###  https://semanticdatacharter.com/ns/sdc4/BooleanListSimpleType
sdc4:BooleanListSimpleType rdf:type rdfs:Datatype ;
                           rdfs:comment "A simple type for a white space-delimited list of boolean values." .


###  https://semanticdatacharter.com/ns/sdc4/DecimalListSimpleType
sdc4:DecimalListSimpleType rdf:type rdfs:Datatype ;
                           rdfs:comment "A simple type for a white space-delimited list of decimal values." .


###  https://semanticdatacharter.com/ns/sdc4/DoubleListSimpleType
sdc4:DoubleListSimpleType rdf:type rdfs:Datatype ;
                          rdfs:comment "A simple type for a white space-delimited list of double precision values." .


###  https://semanticdatacharter.com/ns/sdc4/IntegerListSimpleType
sdc4:IntegerListSimpleType rdf:type rdfs:Datatype ;
                           rdfs:comment "A simple type for a white space-delimited list of integer values." .


###  https://semanticdatacharter.com/ns/sdc4/NonNegativeIntegerListSimpleType
sdc4:NonNegativeIntegerListSimpleType rdf:type rdfs:Datatype ;
                                      rdfs:comment "A simple type for a white space-delimited list of non-negative integer values." .


###  https://semanticdatacharter.com/ns/sdc4/PositiveIntegerListSimpleType
sdc4:PositiveIntegerListSimpleType rdf:type rdfs:Datatype ;
                                   rdfs:comment "A simple type for a white space-delimited list of positive integer values." .


###  https://semanticdatacharter.com/ns/sdc4/StringListSimpleType
sdc4:StringListSimpleType rdf:type rdfs:Datatype ;
                          rdfs:comment "A simple type for a white space-delimited list of string values." .


###  https://semanticdatacharter.com/ns/sdc4/TokenListSimpleType
sdc4:TokenListSimpleType rdf:type rdfs:Datatype ;
                         rdfs:comment "A simple type for a white space-delimited list of normalized token values." .


#################################################################
#    Object Properties
#################################################################

###  https://semanticdatacharter.com/ns/sdc4/acs
sdc4:acs rdf:type owl:ObjectProperty ;
         rdfs:domain sdc4:DMType ;
         rdfs:range sdc4:XdLinkType ;
         rdfs:comment "Identifier of an externally held access control system. This URI can be an ontology, vocabulary or descriptive document URI link." .


###  https://semanticdatacharter.com/ns/sdc4/hasAttestation
sdc4:hasAttestation rdf:type owl:ObjectProperty ;
                    rdfs:domain sdc4:DMType ;
                    rdfs:range sdc4:AttestationType ;
                    rdfs:comment "Attestation record of an instance of data." .


###  https://semanticdatacharter.com/ns/sdc4/hasAudit
sdc4:hasAudit rdf:type owl:ObjectProperty ;
              rdfs:domain sdc4:DMType ;
              rdfs:range sdc4:AuditType ;
              rdfs:comment "List of audits from the system of original commit of information forming the content, or from a conversion gateway which has processed this data." .


###  https://semanticdatacharter.com/ns/sdc4/hasCommitter
sdc4:hasCommitter rdf:type owl:ObjectProperty ;
                  rdfs:domain sdc4:AttestationType ;
                  rdfs:range sdc4:PartyType ;
                  rdfs:comment "Identity of person who committed the item." .


###  https://semanticdatacharter.com/ns/sdc4/hasDataItem
sdc4:hasDataItem rdf:type owl:ObjectProperty ;
                 rdfs:domain sdc4:DMType ;
                 rdfs:range sdc4:ClusterType ;
                 rdfs:comment "The data structure of the model." .


###  https://semanticdatacharter.com/ns/sdc4/hasExceptionalValue
sdc4:hasExceptionalValue rdf:type owl:ObjectProperty ;
                         rdfs:domain sdc4:XdAnyType ;
                         rdfs:range sdc4:ExceptionalValueType .


###  https://semanticdatacharter.com/ns/sdc4/hasFunction
sdc4:hasFunction rdf:type owl:ObjectProperty ;
                 rdfs:domain sdc4:ParticipationType ;
                 rdfs:range sdc4:XdStringType ;
                 rdfs:comment "The function of the performer in this participation. In some applications this might be called a Role." .


###  https://semanticdatacharter.com/ns/sdc4/hasInterval
sdc4:hasInterval rdf:type owl:ObjectProperty ;
                 rdfs:domain sdc4:ReferenceRangeType ;
                 rdfs:range sdc4:XdIntervalType ;
                 rdfs:comment "The data range for this reference range." .


###  https://semanticdatacharter.com/ns/sdc4/hasIntervalUnits
sdc4:hasIntervalUnits rdf:type owl:ObjectProperty ;
                      rdfs:domain sdc4:XdIntervalType ;
                      rdfs:range sdc4:InvlUnits .


###  https://semanticdatacharter.com/ns/sdc4/hasItems
sdc4:hasItems rdf:type owl:ObjectProperty ;
              rdfs:domain sdc4:ClusterType ;
              rdfs:range sdc4:ItemType ;
              rdfs:comment "List of ItemTypes which may be XdAdapterTypes and/or ClusterTypes." .


###  https://semanticdatacharter.com/ns/sdc4/hasLink
sdc4:hasLink rdf:type owl:ObjectProperty ;
             rdfs:domain sdc4:DMType ;
             rdfs:range sdc4:XdLinkType ;
             rdfs:comment "Optional link(s) to other locatable structures or external entities." .


###  https://semanticdatacharter.com/ns/sdc4/hasLocation
sdc4:hasLocation rdf:type owl:ObjectProperty ;
                 rdfs:domain sdc4:AuditType ;
                 rdfs:range sdc4:ClusterType ;
                 rdfs:comment "Location information of the particular site/facility within an organisation which handled the item." .


###  https://semanticdatacharter.com/ns/sdc4/hasLower
sdc4:hasLower rdf:type owl:ObjectProperty ;
              rdfs:domain sdc4:XdIntervalType ;
              rdfs:range sdc4:InvlType ;
              rdfs:comment "The lower boundary of the interval. Must be of the same datatype as the 'upper' boundary." .


###  https://semanticdatacharter.com/ns/sdc4/hasMagnitudeStatus
sdc4:hasMagnitudeStatus rdf:type owl:ObjectProperty ;
                        rdfs:domain sdc4:XdQuantifiedType ;
                        rdfs:range sdc4:MagnitudeStatus ;
                        rdfs:comment """An optional status that describes the relationship of this quantity's value to a contextual target or expected value.The target value itself is not defined here but is known from the context of the measurement, such as a process control limit, a clinical reference range, or a business rule.
Example: A temperature sensor reports a value of 140C. If the system's target operational temperature is 160C,  the magnitude-status for the 140C reading would be 'less_than'.""" .


###  https://semanticdatacharter.com/ns/sdc4/hasMode
sdc4:hasMode rdf:type owl:ObjectProperty ;
             rdfs:domain sdc4:ParticipationType ;
             rdfs:range sdc4:XdStringType ;
             rdfs:comment "The mode of the performer / activity interaction, e.g. present, by telephone, by email etc. If the participation is by device or software it may contain a protocol standard or interface definition." .


###  https://semanticdatacharter.com/ns/sdc4/hasParticipation
sdc4:hasParticipation rdf:type owl:ObjectProperty ;
                      rdfs:domain sdc4:DMType ;
                      rdfs:range sdc4:ParticipationType ;
                      rdfs:comment "List of other participations in the data." .


###  https://semanticdatacharter.com/ns/sdc4/hasPartyDetails
sdc4:hasPartyDetails rdf:type owl:ObjectProperty ;
                     rdfs:domain sdc4:PartyType ;
                     rdfs:range sdc4:ClusterType ;
                     rdfs:comment "A structured element for details about the party." .


###  https://semanticdatacharter.com/ns/sdc4/hasPartyRef
sdc4:hasPartyRef rdf:type owl:ObjectProperty ;
                 rdfs:domain sdc4:PartyType ;
                 rdfs:range sdc4:XdLinkType ;
                 rdfs:comment "Optional reference to more detailed demographic or identification information for this party, in an external system." .


###  https://semanticdatacharter.com/ns/sdc4/hasPerformer
sdc4:hasPerformer rdf:type owl:ObjectProperty ;
                  rdfs:domain sdc4:ParticipationType ;
                  rdfs:range sdc4:PartyType ;
                  rdfs:comment "The id and possibly demographic system link of the party that represents the primary provider of services in the activity." .


###  https://semanticdatacharter.com/ns/sdc4/hasProof
sdc4:hasProof rdf:type owl:ObjectProperty ;
              rdfs:domain sdc4:AttestationType ;
              rdfs:range sdc4:XdFileType ;
              rdfs:comment "Proof of attestation such as an GPG signature." .


###  https://semanticdatacharter.com/ns/sdc4/hasProvider
sdc4:hasProvider rdf:type owl:ObjectProperty ;
                 rdfs:domain sdc4:DMType ;
                 rdfs:range sdc4:PartyType ;
                 rdfs:comment "Optional identification of the source of the information, which might be: • a patient • a patient agent, e.g. parent, guardian • a clinician • a technician • a device or software" .


###  https://semanticdatacharter.com/ns/sdc4/hasReason
sdc4:hasReason rdf:type owl:ObjectProperty ;
               rdfs:domain sdc4:AttestationType ;
               rdfs:range sdc4:XdStringType ;
               rdfs:comment "Reason of this attestation. Usually coded from a standardized vocabulary." .


###  https://semanticdatacharter.com/ns/sdc4/hasReferenceRange
sdc4:hasReferenceRange rdf:type owl:ObjectProperty ;
                       rdfs:domain sdc4:XdOrderedType ;
                       rdfs:range sdc4:ReferenceRangeType ;
                       rdfs:comment "Optional list of ReferenceRanges for this value in its particular measurement context." .


###  https://semanticdatacharter.com/ns/sdc4/hasSubject
sdc4:hasSubject rdf:type owl:ObjectProperty ;
                rdfs:domain sdc4:DMType ;
                rdfs:range sdc4:PartyType ;
                rdfs:comment "Id of human subject of the data, e.g.: • subject of record (patient, customer, etc.) • a family member • another clinically relevant person." .


###  https://semanticdatacharter.com/ns/sdc4/hasSystemId
sdc4:hasSystemId rdf:type owl:ObjectProperty ;
                 rdfs:domain sdc4:AuditType ;
                 rdfs:range sdc4:XdStringType ;
                 rdfs:comment "Identifier of systems which created or handled the information item. 'Systems' can also be defined as an individual application or a data repository in which the data was manipulated." .


###  https://semanticdatacharter.com/ns/sdc4/hasSystemUser
sdc4:hasSystemUser rdf:type owl:ObjectProperty ;
                   rdfs:domain sdc4:AuditType ;
                   rdfs:range sdc4:PartyType ;
                   rdfs:comment "User(s) who created, committed, forwarded or otherwise handled the item." .


###  https://semanticdatacharter.com/ns/sdc4/hasUpper
sdc4:hasUpper rdf:type owl:ObjectProperty ;
              rdfs:domain sdc4:XdIntervalType ;
              rdfs:range sdc4:InvlType ;
              rdfs:comment "The upper boundary of the interval. Must be of the same datatype as the 'lower' boundary." .


###  https://semanticdatacharter.com/ns/sdc4/hasView
sdc4:hasView rdf:type owl:ObjectProperty ;
             rdfs:domain sdc4:AttestationType ;
             rdfs:range sdc4:XdFileType ;
             rdfs:comment "Optional visual representation of content attested e.g. screen image." .


###  https://semanticdatacharter.com/ns/sdc4/hasXdCountUnits
sdc4:hasXdCountUnits rdf:type owl:ObjectProperty ;
                     rdfs:domain sdc4:XdCountType ;
                     rdfs:range sdc4:XdStringType .


###  https://semanticdatacharter.com/ns/sdc4/hasXdDoubleUnits
sdc4:hasXdDoubleUnits rdf:type owl:ObjectProperty ;
                      rdfs:domain sdc4:XdDoubleType ;
                      rdfs:range sdc4:XdStringType .


###  https://semanticdatacharter.com/ns/sdc4/hasXdFloatUnits
sdc4:hasXdFloatUnits rdf:type owl:ObjectProperty ;
                     rdfs:domain sdc4:XdFloatType ;
                     rdfs:range sdc4:XdStringType ;
                     rdfs:comment "The name or type of the float value. May or may not come from a standardized vocabulary." .


###  https://semanticdatacharter.com/ns/sdc4/hasXdQuantityUnits
sdc4:hasXdQuantityUnits rdf:type owl:ObjectProperty ;
                        rdfs:domain sdc4:XdQuantityType ;
                        rdfs:range sdc4:XdStringType ;
                        rdfs:comment "The name or type of the quantity. Examples are \"kg\", \"mmHg\", \"ms-1\", \"km/h\". Should come from a standard terminology." .


###  https://semanticdatacharter.com/ns/sdc4/protocol
sdc4:protocol rdf:type owl:ObjectProperty ;
              rdfs:domain sdc4:DMType ;
              rdfs:range sdc4:XdStringType ;
              rdfs:comment "Optional external identifier of protocol used when collecting the data. This could be a clinical guideline, an operations protocol,etc." .


###  https://semanticdatacharter.com/ns/sdc4/workflow
sdc4:workflow rdf:type owl:ObjectProperty ;
              rdfs:domain sdc4:DMType ;
              rdfs:range sdc4:XdLinkType ;
              rdfs:comment "Identifier of externally held workflow engine (state machine) data for this workflow execution." .


###  https://semanticdatacharter.com/ns/sdc4/xddecimallist-units
sdc4:xddecimallist-units rdf:type owl:ObjectProperty ;
                         rdfs:domain sdc4:XdDecimalListType ;
                         rdfs:range sdc4:XdStringType ;
                         rdfs:comment "The name or type of the decimal list values. Examples are \"kg\", \"mmHg\", \"ms-1\", \"km/h\". Should come from a standard terminology. All values in the list share these units." .


###  https://semanticdatacharter.com/ns/sdc4/xddoublelist-units
sdc4:xddoublelist-units rdf:type owl:ObjectProperty ;
                        rdfs:domain sdc4:XdDoubleListType ;
                        rdfs:range sdc4:XdStringType ;
                        rdfs:comment "The name or type of the double list values. Examples are \"kg\", \"mmHg\", \"ms-1\", \"km/h\". Should come from a standard terminology. All values in the list share these units." .


###  https://semanticdatacharter.com/ns/sdc4/xdintegerlist-units
sdc4:xdintegerlist-units rdf:type owl:ObjectProperty ;
                         rdfs:domain sdc4:XdIntegerListType ;
                         rdfs:range sdc4:XdStringType ;
                         rdfs:comment "The name or type of the integer list values. Examples are \"items\", \"counts\", \"indices\". Should come from a standard terminology. All values in the list share these units." .


###  https://semanticdatacharter.com/ns/sdc4/xdnonnegativeintegerlist-units
sdc4:xdnonnegativeintegerlist-units rdf:type owl:ObjectProperty ;
                                    rdfs:domain sdc4:XdNonNegativeIntegerListType ;
                                    rdfs:range sdc4:XdStringType ;
                                    rdfs:comment "The name or type of the non-negative integer list values. Examples are \"items\", \"counts\", \"indices\". Should come from a standard terminology. All values in the list share these units." .


###  https://semanticdatacharter.com/ns/sdc4/xdpositiveintegerlist-units
sdc4:xdpositiveintegerlist-units rdf:type owl:ObjectProperty ;
                                 rdfs:domain sdc4:XdPositiveIntegerListType ;
                                 rdfs:range sdc4:XdStringType ;
                                 rdfs:comment "The name or type of the positive integer list values. Examples are \"items\", \"counts\", \"indices\". Should come from a standard terminology. All values in the list share these units." .


#################################################################
#    Data properties
#################################################################

###  https://semanticdatacharter.com/ns/sdc4/accuracy_margin
sdc4:accuracy_margin rdf:type owl:DatatypeProperty ;
                     rdfs:domain sdc4:XdQuantifiedType ;
                     rdfs:range xsd:decimal ;
                     rdfs:comment """Models ACCURACY. Defines the margin of systematic error, representing how close a measurement is to the true value. 
                This value is expressed as a plus-or-minus percentage of the magnitude. For example, a value of '2.5' indicates the true value is within +/- 2.5% of the stated magnitude.""" .


###  https://semanticdatacharter.com/ns/sdc4/act
sdc4:act rdf:type owl:DatatypeProperty ;
         rdfs:domain sdc4:XdAnyType ;
         rdfs:range xsd:string ;
         rdfs:comment """Access Control Tag: 

Descriptive name of this datatype model. Provides the semantic 'name' for the model. Replaces what would be a global XML element name or class name in conventional modeling."""@en-us ;
         rdfs:label "act" .


###  https://semanticdatacharter.com/ns/sdc4/alt-text
sdc4:alt-text rdf:type owl:DatatypeProperty ;
              rdfs:domain sdc4:XdFileType ;
              rdfs:range xsd:string ;
              rdfs:comment "Text to display in lieu of multimedia display or execution." .


###  https://semanticdatacharter.com/ns/sdc4/committed
sdc4:committed rdf:type owl:DatatypeProperty ;
               rdfs:domain sdc4:AttestationType ;
               rdfs:range xsd:dateTime ;
               rdfs:comment "Timestamp of committal of the item." .


###  https://semanticdatacharter.com/ns/sdc4/compression-type
sdc4:compression-type rdf:type owl:DatatypeProperty ;
                      rdfs:domain sdc4:XdFileType ;
                      rdfs:range xsd:string ;
                      rdfs:comment "Compression/archiving mime-type. If this elements does not exist then it means there is no compression/archiving. For a list of common mime-types for compression/archiving see: http://en.wikipedia.org/wiki/List_of_archive_formats." .


###  https://semanticdatacharter.com/ns/sdc4/creation_timestamp
sdc4:creation_timestamp rdf:type owl:DatatypeProperty ;
                        rdfs:domain sdc4:DMType ;
                        rdfs:range xsd:dateTime ;
                        rdfs:comment """An optional run-time timestamp that indicates the exact moment this specific data instance was created or generated. 
            This element provides a definitive point-in-time reference for the data payload itself. 
            It is distinct from the design-time Dublin Core metadata which describes the model definition.
            This timestamp is crucial for data versioning, caching, and synchronization in distributed systems.""" .


###  https://semanticdatacharter.com/ns/sdc4/current-state
sdc4:current-state rdf:type owl:DatatypeProperty ;
                   rdfs:domain sdc4:DMType ;
                   rdfs:comment "The data structure of the model." .


###  https://semanticdatacharter.com/ns/sdc4/definition
sdc4:definition rdf:type owl:DatatypeProperty ;
                rdfs:domain sdc4:ReferenceRangeType ;
                rdfs:range xsd:string ;
                rdfs:comment "Term whose value indicates the meaning of this range, e.g. 'normal', 'critical', 'therapeutic' etc." .


###  https://semanticdatacharter.com/ns/sdc4/dm-encoding
sdc4:dm-encoding rdf:type owl:DatatypeProperty ;
                 rdfs:domain sdc4:DMType ;
                 rdfs:range xsd:string ;
                 rdfs:comment "Name of character set encoding in which text values in this DM are encoded. Default is utf-8." .


###  https://semanticdatacharter.com/ns/sdc4/dm-language
sdc4:dm-language rdf:type owl:DatatypeProperty ;
                 rdfs:domain sdc4:DMType ;
                 rdfs:range xsd:language ;
                 rdfs:comment "Mandatory indicator of the localised language in which this DM is written. The value space of language is the set of all strings that are valid language identifiers as defined [RFC 3066]." .


###  https://semanticdatacharter.com/ns/sdc4/encoding
sdc4:encoding rdf:type owl:DatatypeProperty ;
              rdfs:domain sdc4:XdFileType ;
              rdfs:range xsd:short ;
              rdfs:comment "Name of character encoding scheme in which this value is encoded. Coded from the IANA charcater set table: http://www.iana.org/assignments/character-sets Unicode is the default assumption in S3Model, with UTF-8 being the assumed encoding. This                element allows for variations from these assumptions." .


###  https://semanticdatacharter.com/ns/sdc4/end
sdc4:end rdf:type owl:DatatypeProperty ;
         rdfs:domain sdc4:ParticipationType ;
         rdfs:range xsd:dateTime ;
         rdfs:comment "The ending datetime when the participation took place." .


###  https://semanticdatacharter.com/ns/sdc4/ev-name
sdc4:ev-name rdf:type owl:DatatypeProperty ;
             rdfs:domain sdc4:ExceptionalValueType ;
             rdfs:range xsd:string ;
             rdfs:comment "A short title or phase for the exceptional type value." .


###  https://semanticdatacharter.com/ns/sdc4/false-value
sdc4:false-value rdf:type owl:DatatypeProperty ;
                 rdfs:subPropertyOf owl:topDataProperty ;
                 rdfs:domain sdc4:XdBooleanType ;
                 rdfs:range xsd:string ;
                 rdfs:comment "A string that represents a boolean False in the implementation. These are constrained by a set of enumerations in the model." ;
                 rdfs:label "false-value" .


###  https://semanticdatacharter.com/ns/sdc4/formalism
sdc4:formalism rdf:type owl:DatatypeProperty ;
               rdfs:domain sdc4:XdFileType ;
               rdfs:range xsd:string ;
               rdfs:comment "Name of the formalism or syntax used to inform an application regarding a candidate parser to use on the content. Examples might include: 'ATL', 'MOLA', 'QVT', 'GDL', 'GLIF', etc." .


###  https://semanticdatacharter.com/ns/sdc4/hash-function
sdc4:hash-function rdf:type owl:DatatypeProperty ;
                   rdfs:domain sdc4:XdFileType ;
                   rdfs:range xsd:string ;
                   rdfs:comment "Hash function used to compute hash-result. See: http://en.wikipedia.org/wiki/List_of_hash_functions#Cryptographic_hash_functions" .


###  https://semanticdatacharter.com/ns/sdc4/hash-result
sdc4:hash-result rdf:type owl:DatatypeProperty ;
                 rdfs:domain sdc4:XdFileType ;
                 rdfs:range xsd:string ;
                 rdfs:comment "Hash function result of the 'media-content'. There must be a corresponding hash function type listed for this to have any meaning. See: http://en.wikipedia.org/wiki/List_of_hash_functions#Cryptographic_hash_functions" .


###  https://semanticdatacharter.com/ns/sdc4/instance_id
sdc4:instance_id rdf:type owl:DatatypeProperty ;
                 rdfs:domain sdc4:DMType ;
                 rdfs:range xsd:string ;
                 rdfs:comment """An optional, globally unique identifier for this specific data instance. It is strongly recommended to use a UUID (Universally Unique Identifier).
            This ID provides a persistent identity for the data that is decoupled from any storage or transport mechanism (e.g., filename, database primary key). 
            It is essential for reliably tracking, updating, and referencing data in distributed systems, message queues, and data aggregation platforms.""" .


###  https://semanticdatacharter.com/ns/sdc4/instance_version
sdc4:instance_version rdf:type owl:DatatypeProperty ;
                      rdfs:domain sdc4:DMType ;
                      rdfs:range xsd:string ;
                      rdfs:comment """An optional identifier for the specific version of this data instance. 
            When paired with instance_id, it allows for a complete version history of a single data record.
            The type is a string to accommodate various versioning schemes, such as simple integers ('1', '2'), semantic versioning ('1.2.1'), or timestamps.""" .


###  https://semanticdatacharter.com/ns/sdc4/invl-date
sdc4:invl-date rdf:type owl:DatatypeProperty ;
               rdfs:domain sdc4:InvlType ;
               rdfs:range xsd:date .


###  https://semanticdatacharter.com/ns/sdc4/invl-dateTime
sdc4:invl-dateTime rdf:type owl:DatatypeProperty ;
                   rdfs:domain sdc4:InvlType ;
                   rdfs:range xsd:dateTime .


###  https://semanticdatacharter.com/ns/sdc4/invl-decimal
sdc4:invl-decimal rdf:type owl:DatatypeProperty ;
                  rdfs:domain sdc4:InvlType ;
                  rdfs:range xsd:decimal .


###  https://semanticdatacharter.com/ns/sdc4/invl-double
sdc4:invl-double rdf:type owl:DatatypeProperty ;
                 rdfs:domain sdc4:InvlType ;
                 rdfs:range xsd:double .


###  https://semanticdatacharter.com/ns/sdc4/invl-duration
sdc4:invl-duration rdf:type owl:DatatypeProperty ;
                   rdfs:domain sdc4:InvlType ;
                   rdfs:range xsd:duration .


###  https://semanticdatacharter.com/ns/sdc4/invl-float
sdc4:invl-float rdf:type owl:DatatypeProperty ;
                rdfs:domain sdc4:InvlType ;
                rdfs:range xsd:float .


###  https://semanticdatacharter.com/ns/sdc4/invl-int
sdc4:invl-int rdf:type owl:DatatypeProperty ;
              rdfs:domain sdc4:InvlType ;
              rdfs:range xsd:integer .


###  https://semanticdatacharter.com/ns/sdc4/invl-time
sdc4:invl-time rdf:type owl:DatatypeProperty ;
               rdfs:domain sdc4:InvlType ;
               rdfs:range xsd:time .


###  https://semanticdatacharter.com/ns/sdc4/is-normal
sdc4:is-normal rdf:type owl:DatatypeProperty ;
               rdfs:domain sdc4:ReferenceRangeType ;
               rdfs:range xsd:boolean ;
               rdfs:comment "True if this reference range defines values that are considered to be normal. In the context of the value in the definition element." .


###  https://semanticdatacharter.com/ns/sdc4/label
sdc4:label rdf:type owl:DatatypeProperty ;
           rdfs:domain sdc4:AttestationType ,
                       sdc4:AuditType ,
                       sdc4:ClusterType ,
                       sdc4:DMType ,
                       sdc4:ParticipationType ,
                       sdc4:PartyType ,
                       sdc4:XdAnyType ;
           rdfs:range xsd:string ;
           rdfs:comment "Descriptive name of this datatype model. Provides the semantic 'name' for the model."@en-us ;
           rdfs:label "label" .


###  https://semanticdatacharter.com/ns/sdc4/latitude
sdc4:latitude rdf:type owl:DatatypeProperty ;
              rdfs:domain sdc4:XdAnyType ;
              rdfs:range [ rdf:type rdfs:Datatype ;
                           owl:onDatatype xsd:decimal ;
                           owl:withRestrictions ( [ xsd:minInclusive -90.000000
                                                  ]
                                                  [ xsd:maxInclusive 90.000000
                                                  ]
                                                )
                         ] ;
              rdfs:comment "Latitude in decimal format. Value range -90.000000 to 90.000000."@en-us .


###  https://semanticdatacharter.com/ns/sdc4/link
sdc4:link rdf:type owl:DatatypeProperty ;
          rdfs:domain sdc4:XdLinkType ;
          rdfs:range xsd:anyURI ;
          rdfs:comment "A dereferenceable (or not) URL to another CMC or other model like entity." ;
          rdfs:label "link" .


###  https://semanticdatacharter.com/ns/sdc4/longitude
sdc4:longitude rdf:type owl:DatatypeProperty ;
               rdfs:domain sdc4:XdAnyType ;
               rdfs:range [ rdf:type rdfs:Datatype ;
                            owl:onDatatype xsd:decimal ;
                            owl:withRestrictions ( [ xsd:minInclusive -180.000000
                                                   ]
                                                   [ xsd:maxInclusive 180.000000
                                                   ]
                                                 )
                          ] ;
               rdfs:comment "Longitude in decimal format. Value range -180.000000 to 180.000000."@en-us .


###  https://semanticdatacharter.com/ns/sdc4/lower-bounded
sdc4:lower-bounded rdf:type owl:DatatypeProperty ;
                   rdfs:domain sdc4:XdIntervalType ;
                   rdfs:range xsd:boolean .


###  https://semanticdatacharter.com/ns/sdc4/lower-included
sdc4:lower-included rdf:type owl:DatatypeProperty ;
                    rdfs:domain sdc4:XdIntervalType ;
                    rdfs:range xsd:boolean .


###  https://semanticdatacharter.com/ns/sdc4/magnitude-status
sdc4:magnitude-status rdf:type owl:DatatypeProperty ;
                      rdfs:domain sdc4:XdQuantifiedType ;
                      rdfs:comment """An optional status that describes the relationship of this quantity's value to a contextual target or expected value.
The target value itself is not defined here but is known from the context of the measurement, such as a process control limit, a clinical reference range, or a business rule.
Example: A temperature sensor reports a value of 140C. If the system's target operational temperature is 160C, the magnitude-status for the 140C reading would be 'less_than'.""" .


###  https://semanticdatacharter.com/ns/sdc4/media-content
sdc4:media-content rdf:type owl:DatatypeProperty ;
                   rdfs:domain sdc4:XdFileType ;
                   rdfs:range xsd:base64Binary ;
                   rdfs:comment "The content, if stored locally. The CMC modeler chooses either a uri or local content element." .


###  https://semanticdatacharter.com/ns/sdc4/media-type
sdc4:media-type rdf:type owl:DatatypeProperty ;
                rdfs:domain sdc4:XdFileType ;
                rdfs:range xsd:string ;
                rdfs:comment "Media (MIME) type of the original media-content w/o any compression. See IANA registered types: http://www.iana.org/assignments/media-types/media-types.xhtml" .


###  https://semanticdatacharter.com/ns/sdc4/mode
sdc4:mode rdf:type owl:DatatypeProperty ;
          rdfs:domain sdc4:ParticipationType ;
          rdfs:range xsd:string ;
          rdfs:comment "The mode of the performer / activity interaction, e.g. present, by telephone, by email etc. If the participation is by device or software it may contain a protocol standard or interface definition." .


###  https://semanticdatacharter.com/ns/sdc4/modified
sdc4:modified rdf:type owl:DatatypeProperty ;
              rdfs:domain sdc4:XdAnyType ;
              rdfs:range xsd:dateTime ;
              rdfs:comment "Time Modified. If present this must be a valid date-time stamp. It is used to indicate the the actual date and time the data was last changed."@en-us .


###  https://semanticdatacharter.com/ns/sdc4/normal-status
sdc4:normal-status rdf:type owl:DatatypeProperty ;
                   rdfs:domain sdc4:XdOrderedType ;
                   rdfs:range xsd:string ;
                   rdfs:comment "Optional normal status indicator of value with respect to normal range for this value. Often included by lab, even if the normal range itself is not included. Coded by ordinals in series HHH, HH, H, (nothing), L, LL, LLL, etc." .


###  https://semanticdatacharter.com/ns/sdc4/ordinal
sdc4:ordinal rdf:type owl:DatatypeProperty ;
             rdfs:domain sdc4:XdOrdinalType ;
             rdfs:range xsd:decimal ;
             rdfs:comment "Value in ordered enumeration of values. The base integer is zero with any number of integer values used to order the symbols. Example 1: 0 = Trace, 1 = +, 2 = ++, 3 = +++, etc. Example 2: 0 = Mild, 1 = Moderate, 2 = Severe" .


###  https://semanticdatacharter.com/ns/sdc4/party-name
sdc4:party-name rdf:type owl:DatatypeProperty ;
                rdfs:domain sdc4:PartyType ;
                rdfs:range xsd:string ;
                rdfs:comment "Optional human-readable name (in String form)." .


###  https://semanticdatacharter.com/ns/sdc4/pending
sdc4:pending rdf:type owl:DatatypeProperty ;
             rdfs:domain sdc4:AttestationType ;
             rdfs:range xsd:boolean ;
             rdfs:comment "True if this attestation is outstanding; 'false' means it has been completed." .


###  https://semanticdatacharter.com/ns/sdc4/precision_digits
sdc4:precision_digits rdf:type owl:DatatypeProperty ;
                      rdfs:domain sdc4:XdQuantifiedType ;
                      rdfs:range xsd:nonNegativeInteger ;
                      rdfs:comment """Models PRECISION. Defines the resolution of the measurement by specifying the number of significant digits after the decimal point.
                This is especially useful for decimal-based quantities where trailing zeros are significant. For example, a magnitude of '10.50' with a precision_digits of '2' indicates the measurement is precise to the hundredths place.""" .


###  https://semanticdatacharter.com/ns/sdc4/relation
sdc4:relation rdf:type owl:DatatypeProperty ;
              rdfs:domain sdc4:XdLinkType ;
              rdfs:range xsd:string ;
              rdfs:comment "A required term, normally drawn from a vocabulary or ontology such as the OBO RO." ;
              rdfs:label "relation" .


###  https://semanticdatacharter.com/ns/sdc4/relation-uri
sdc4:relation-uri rdf:type owl:DatatypeProperty ;
                  rdfs:domain sdc4:XdLinkType ;
                  rdfs:range xsd:anyURI ;
                  rdfs:comment "A URI where the definition of the relation element term can be found. Normally points to an ontology such as the OBO RO http://purl.obolibrary.org/obo/ro.owl" ;
                  rdfs:label "relation-uri" .


###  https://semanticdatacharter.com/ns/sdc4/size
sdc4:size rdf:type owl:DatatypeProperty ;
          rdfs:domain sdc4:XdFileType ;
          rdfs:range xsd:integer ;
          rdfs:comment "Original size in bytes of unencoded encapsulated data. I.e. encodings such as base64, hexadecimal, etc. do not change the value of this element." .


###  https://semanticdatacharter.com/ns/sdc4/start
sdc4:start rdf:type owl:DatatypeProperty ;
           rdfs:domain sdc4:ParticipationType ;
           rdfs:range xsd:dateTime ;
           rdfs:comment "The beginning datetime when the participation took place." .


###  https://semanticdatacharter.com/ns/sdc4/symbol
sdc4:symbol rdf:type owl:DatatypeProperty ;
            rdfs:domain sdc4:XdOrdinalType ;
            rdfs:range xsd:string ;
            rdfs:comment "Coded textual representation of this value in the enumeration, which may be strings made from \"+\" symbols, or other enumerations of terms such as \"mild\", \"moderate\", \"severe\", or even the same number series as the values, e.g. \"1\", \"2\", \"3\"." .


###  https://semanticdatacharter.com/ns/sdc4/timestamp
sdc4:timestamp rdf:type owl:DatatypeProperty ;
               rdfs:domain sdc4:AuditType ;
               rdfs:range xsd:dateTime ;
               rdfs:comment "Timestamp of handling the item." .


###  https://semanticdatacharter.com/ns/sdc4/tr
sdc4:tr rdf:type owl:DatatypeProperty ;
        rdfs:domain sdc4:XdAnyType ;
        rdfs:range xsd:dateTime ;
        rdfs:comment "Time Recorded. If present this must be a valid date-time. It is used to indicate the the actual date and time the data was recorded."@en-us .


###  https://semanticdatacharter.com/ns/sdc4/units-name
sdc4:units-name rdf:type owl:DatatypeProperty ;
                rdfs:domain sdc4:InvlUnits ;
                rdfs:range xsd:string .


###  https://semanticdatacharter.com/ns/sdc4/units-uri
sdc4:units-uri rdf:type owl:DatatypeProperty ;
               rdfs:domain sdc4:InvlUnits ;
               rdfs:range xsd:anyURI .


###  https://semanticdatacharter.com/ns/sdc4/upper-bounded
sdc4:upper-bounded rdf:type owl:DatatypeProperty ;
                   rdfs:domain sdc4:XdIntervalType ;
                   rdfs:range xsd:boolean .


###  https://semanticdatacharter.com/ns/sdc4/upper-included
sdc4:upper-included rdf:type owl:DatatypeProperty ;
                    rdfs:domain sdc4:XdIntervalType ;
                    rdfs:range xsd:boolean .


###  https://semanticdatacharter.com/ns/sdc4/uri
sdc4:uri rdf:type owl:DatatypeProperty ;
         rdfs:domain sdc4:XdFileType ;
         rdfs:range xsd:anyURI ;
         rdfs:comment "URI reference to electronic information stored outside the record as a file, database entry etc, if supplied as a reference." .


###  https://semanticdatacharter.com/ns/sdc4/value
sdc4:value rdf:type owl:DatatypeProperty ;
           rdfs:domain sdc4:XdBooleanType ;
           rdfs:range xsd:string ;
           rdfs:comment "A string that represents a boolean True in the implementation. These are constrained by a set of enumerations in the datamodel." ;
           rdfs:label "true-value" .


###  https://semanticdatacharter.com/ns/sdc4/vtb
sdc4:vtb rdf:type owl:DatatypeProperty ;
         rdfs:domain sdc4:XdAnyType ;
         rdfs:range xsd:dateTime ;
         rdfs:comment "Valid Time Begin. If present this must be a valid datetime including timezone. It is used to indicate the beginning time that information is considered valid."@en-us .


###  https://semanticdatacharter.com/ns/sdc4/vte
sdc4:vte rdf:type owl:DatatypeProperty ;
         rdfs:domain sdc4:XdAnyType ;
         rdfs:range xsd:dateTime ;
         rdfs:comment "Valid Time End. If present this must be a valid date-time including timezone. It is used to indicate the ending time that information is considered valid or the time the information expired or will expire."@en-us .


###  https://semanticdatacharter.com/ns/sdc4/xdbooleanlist-value
sdc4:xdbooleanlist-value rdf:type owl:DatatypeProperty ;
                         rdfs:domain sdc4:XdBooleanListType ;
                         rdfs:range sdc4:BooleanListSimpleType ;
                         rdfs:comment "Space-delimited list of boolean values. Values should be 'true' or 'false' separated by single spaces." .


###  https://semanticdatacharter.com/ns/sdc4/xdcount-value
sdc4:xdcount-value rdf:type owl:DatatypeProperty ;
                   rdfs:domain sdc4:XdCountType ;
                   rdfs:range xsd:integer ;
                   rdfs:comment "Integer value of the counted items." ;
                   rdfs:label "xdcount-value" .


###  https://semanticdatacharter.com/ns/sdc4/xddecimallist-value
sdc4:xddecimallist-value rdf:type owl:DatatypeProperty ;
                         rdfs:domain sdc4:XdDecimalListType ;
                         rdfs:range sdc4:DecimalListSimpleType ;
                         rdfs:comment "Space-delimited list of decimal values. Values should be valid decimal numbers separated by single spaces." .


###  https://semanticdatacharter.com/ns/sdc4/xddouble-value
sdc4:xddouble-value rdf:type owl:DatatypeProperty ;
                    rdfs:comment "Double value. This type accepts several \"special\" values: positive zero (0), negative zero (-0) (which is greater than positive 0 but less than any negative value), infinity (INF) (which is greater than any value), negative infinity (-INF) (which is less than any float, and \"not a number\" (NaN)" .


###  https://semanticdatacharter.com/ns/sdc4/xddoublelist-value
sdc4:xddoublelist-value rdf:type owl:DatatypeProperty ;
                        rdfs:domain sdc4:XdDoubleListType ;
                        rdfs:range sdc4:DoubleListSimpleType ;
                        rdfs:comment "Space-delimited list of double precision values. Values should be valid double numbers separated by single spaces." .


###  https://semanticdatacharter.com/ns/sdc4/xdfile-language
sdc4:xdfile-language rdf:type owl:DatatypeProperty ;
                     rdfs:domain sdc4:XdFileType ;
                     rdfs:range xsd:language ;
                     rdfs:comment "Optional indicator of the localised language of the content. Typically remains optional in the CMC and used at runtime when the content is in a different language from the enclosing CMC." .


###  https://semanticdatacharter.com/ns/sdc4/xdfloat-value
sdc4:xdfloat-value rdf:type owl:DatatypeProperty ;
                   rdfs:domain sdc4:XdFloatType ;
                   rdfs:range xsd:float ;
                   rdfs:comment "Float value. This type accepts several \"special\" values: positive zero (0), negative zero (-0) (which is greater than positive 0 but less than any negative value), infinity (INF) (which is greater than any value), negative infinity (-INF) (which is less than any float, and \"not a number\" (NaN)" .


###  https://semanticdatacharter.com/ns/sdc4/xdintegerlist-value
sdc4:xdintegerlist-value rdf:type owl:DatatypeProperty ;
                         rdfs:domain sdc4:XdIntegerListType ;
                         rdfs:range sdc4:IntegerListSimpleType ;
                         rdfs:comment "Space-delimited list of integer values. Values should be valid integers separated by single spaces." .


###  https://semanticdatacharter.com/ns/sdc4/xdnonnegativeintegerlist-value
sdc4:xdnonnegativeintegerlist-value rdf:type owl:DatatypeProperty ;
                                    rdfs:domain sdc4:XdNonNegativeIntegerListType ;
                                    rdfs:range sdc4:NonNegativeIntegerListSimpleType ;
                                    rdfs:comment "Space-delimited list of non-negative integer values. Values should be valid non-negative integers separated by single spaces." .


###  https://semanticdatacharter.com/ns/sdc4/xdpositiveintegerlist-value
sdc4:xdpositiveintegerlist-value rdf:type owl:DatatypeProperty ;
                                 rdfs:domain sdc4:XdPositiveIntegerListType ;
                                 rdfs:range sdc4:PositiveIntegerListSimpleType ;
                                 rdfs:comment "Space-delimited list of positive integer values. Values should be valid positive integers separated by single spaces." .


###  https://semanticdatacharter.com/ns/sdc4/xdquantity-value
sdc4:xdquantity-value rdf:type owl:DatatypeProperty ;
                      rdfs:domain sdc4:XdQuantityType ;
                      rdfs:range xsd:decimal ;
                      rdfs:comment "Numeric decimal value of the quantity." .


###  https://semanticdatacharter.com/ns/sdc4/xdstring-language
sdc4:xdstring-language rdf:type owl:DatatypeProperty ;
                       rdfs:domain sdc4:XdStringType ;
                       rdfs:range xsd:language ;
                       rdfs:comment "Optional indicator of the localised language in which this data-type is written. Used when the language used here is different from the enclosing Data Model." .


###  https://semanticdatacharter.com/ns/sdc4/xdstring-value
sdc4:xdstring-value rdf:type owl:DatatypeProperty ;
                    rdfs:domain sdc4:XdStringType ;
                    rdfs:range xsd:string ;
                    rdfs:comment "The string value of the item." .


###  https://semanticdatacharter.com/ns/sdc4/xdstringlist-value
sdc4:xdstringlist-value rdf:type owl:DatatypeProperty ;
                        rdfs:domain sdc4:XdStringListType ;
                        rdfs:range sdc4:StringListSimpleType ;
                        rdfs:comment "Space-delimited list of string values. Values should be valid strings separated by single spaces." .


###  https://semanticdatacharter.com/ns/sdc4/xdtemporal-date
sdc4:xdtemporal-date rdf:type owl:DatatypeProperty ;
                     rdfs:domain sdc4:XdTemporalType ;
                     rdfs:range xsd:date ;
                     rdfs:comment "Represents a specific calendar date (YYYY-MM-DD), with an optional timezone." .


###  https://semanticdatacharter.com/ns/sdc4/xdtemporal-datetime
sdc4:xdtemporal-datetime rdf:type owl:DatatypeProperty ;
                         rdfs:domain sdc4:XdTemporalType ;
                         rdfs:range xsd:dateTime ;
                         rdfs:comment "Represents a specific instant in time (YYYY-MM-DDThh:mm:ss.sss), with an optional timezone." .


###  https://semanticdatacharter.com/ns/sdc4/xdtemporal-day
sdc4:xdtemporal-day rdf:type owl:DatatypeProperty ;
                    rdfs:domain sdc4:XdTemporalType ;
                    rdfs:range xsd:gDay ;
                    rdfs:comment "Represents a recurring Gregorian day (---DD)." .


###  https://semanticdatacharter.com/ns/sdc4/xdtemporal-duration
sdc4:xdtemporal-duration rdf:type owl:DatatypeProperty ;
                         rdfs:domain sdc4:XdTemporalType ;
                         rdfs:range xsd:duration ;
                         rdfs:comment "Represents a duration of time as defined by ISO 8601 (e.g., P1Y2M3D)." .


###  https://semanticdatacharter.com/ns/sdc4/xdtemporal-month
sdc4:xdtemporal-month rdf:type owl:DatatypeProperty ;
                      rdfs:domain sdc4:XdTemporalType ;
                      rdfs:range xsd:gMonth ;
                      rdfs:comment "Represents a recurring Gregorian month (--MM--)." .


###  https://semanticdatacharter.com/ns/sdc4/xdtemporal-month-day
sdc4:xdtemporal-month-day rdf:type owl:DatatypeProperty ;
                          rdfs:domain sdc4:XdTemporalType ;
                          rdfs:range xsd:gMonthDay ;
                          rdfs:comment "Represents a recurring Gregorian day in a recurring month (--MM-DD)." .


###  https://semanticdatacharter.com/ns/sdc4/xdtemporal-time
sdc4:xdtemporal-time rdf:type owl:DatatypeProperty ;
                     rdfs:domain sdc4:XdTemporalType ;
                     rdfs:range xsd:time ;
                     rdfs:comment "Represents a recurring time of day (hh:mm:ss.sss), with an optional timezone." .


###  https://semanticdatacharter.com/ns/sdc4/xdtemporal-year
sdc4:xdtemporal-year rdf:type owl:DatatypeProperty ;
                     rdfs:domain sdc4:XdTemporalType ;
                     rdfs:range xsd:gYear ;
                     rdfs:comment "Represents a specific Gregorian calendar year (YYYY)." .


###  https://semanticdatacharter.com/ns/sdc4/xdtemporal-year-month
sdc4:xdtemporal-year-month rdf:type owl:DatatypeProperty ;
                           rdfs:domain sdc4:XdTemporalType ;
                           rdfs:range xsd:gYearMonth ;
                           rdfs:comment "Represents a specific Gregorian month in a specific year (YYYY-MM)." .


###  https://semanticdatacharter.com/ns/sdc4/xdtoken-language
sdc4:xdtoken-language rdf:type owl:DatatypeProperty ;
                      rdfs:domain sdc4:XdTokenType ;
                      rdfs:range xsd:language ;
                      rdfs:comment "Optional indicator of the localised language in which this data-type is written. Used when the language used here is different from the enclosing Data Model." .


###  https://semanticdatacharter.com/ns/sdc4/xdtoken-value
sdc4:xdtoken-value rdf:type owl:DatatypeProperty ;
                   rdfs:domain sdc4:XdTokenType ;
                   rdfs:range xsd:token ;
                   rdfs:comment "The token value of the item. This is a normalized string where leading and trailing whitespace is removed and internal whitespace is normalized to single spaces." .


###  https://semanticdatacharter.com/ns/sdc4/xdtokenlist-value
sdc4:xdtokenlist-value rdf:type owl:DatatypeProperty ;
                       rdfs:domain sdc4:XdTokenListType ;
                       rdfs:range sdc4:TokenListSimpleType ;
                       rdfs:comment "Space-delimited list of normalized token values. Values should be valid tokens separated by single spaces. Token values have leading and trailing whitespace removed and internal whitespace normalized to single spaces." .


#################################################################
#    Classes
#################################################################

###  https://semanticdatacharter.com/ns/sdc4/ASKRType
sdc4:ASKRType rdf:type owl:Class ;
              rdfs:subClassOf sdc4:ExceptionalValueType ;
              rdfs:comment "Asked and Refused : Information was sought but refused to be provided (e.g., patient was asked but refused to answer)." .


###  https://semanticdatacharter.com/ns/sdc4/ASKUType
sdc4:ASKUType rdf:type owl:Class ;
              rdfs:subClassOf sdc4:ExceptionalValueType ;
              rdfs:comment "Asked but Unknown : Information was sought but not found (e.g., patient was asked but did not know)" .


###  https://semanticdatacharter.com/ns/sdc4/AttestationType
sdc4:AttestationType rdf:type owl:Class ;
                     rdfs:subClassOf sdc4:CMC ;
                     rdfs:comment "Record an attestation by a party of the DM content. The type of attestation is recorded by the reason attribute, which my be coded." .


###  https://semanticdatacharter.com/ns/sdc4/AuditType
sdc4:AuditType rdf:type owl:Class ;
               rdfs:subClassOf sdc4:CMC ;
               rdfs:comment "AuditType provides a mechanism to identify the who/where/when tracking of instances as they move from system to system." .


###  https://semanticdatacharter.com/ns/sdc4/CMC
sdc4:CMC rdf:type owl:Class ;
         rdfs:comment "The abstract superclass for all components in the SDC4 Reference Model. All SDC4 complexTypes are subclasses of CMC."@en-us ;
         rdfs:label "Conceptual Model Component"@en-us .


###  https://semanticdatacharter.com/ns/sdc4/ClusterType
sdc4:ClusterType rdf:type owl:Class ;
                 rdfs:subClassOf sdc4:ItemType ;
                 rdfs:comment """A structural component for grouping other items.
The grouping component, which may contain further instances of itself or any eXtended datatype wrapped in an XdAdapterType, in an ordered list. This can serve as the root component for arbitrarily complex structures."""@en-us .


###  https://semanticdatacharter.com/ns/sdc4/DERType
sdc4:DERType rdf:type owl:Class ;
             rdfs:subClassOf sdc4:ExceptionalValueType ;
             rdfs:comment "Derived : An actual value may exist, but it must be derived from the provided information; usually an expression is provided directly." .


###  https://semanticdatacharter.com/ns/sdc4/DMType
sdc4:DMType rdf:type owl:Class ;
            rdfs:subClassOf sdc4:CMC ;
            rdfs:comment "The root node of a Data Model (DM) instance."@en-us .


###  https://semanticdatacharter.com/ns/sdc4/ExceptionalValueType
sdc4:ExceptionalValueType rdf:type owl:Class ;
                          rdfs:subClassOf sdc4:CMC ;
                          rdfs:comment """The superclass for all exceptional values used to explain missing or invalid data.
Subtypes are used to indicate why a value is missing (Null) or is outside a measurable range. The element ev-name is fixed in restricted types to a descriptive string. The subtypes defined in the reference model are considered sufficiently generic to be
        useful in many instances. Data Models may contain additional ExceptionalValueType restrictions to allow for domain related reasons for errant or missing data."""@en-us .


###  https://semanticdatacharter.com/ns/sdc4/INVType
sdc4:INVType rdf:type owl:Class ;
             rdfs:subClassOf sdc4:ExceptionalValueType ;
             rdfs:comment "Invalid : The value as represented in the instance is not a member of the set of permitted data values in the constrained value domain of a variable." .


###  https://semanticdatacharter.com/ns/sdc4/InvlType
sdc4:InvlType rdf:type owl:Class ;
              rdfs:subClassOf owl:Thing ;
              rdfs:comment "Defines the set of permissible, comparable datatypes that can be used as the boundary for an interval. In a Data Model, this type is constrained to a single choice (e.g., only 'invl-decimal')." .


###  https://semanticdatacharter.com/ns/sdc4/InvlUnits
sdc4:InvlUnits rdf:type owl:Class ;
               rdfs:comment "The units designation for an Interval. This is composed of a units name and a URI because a ReferenceRange can contain intervals with different units (e.g., a temperature range in Celsius and another in Fahrenheit)." .


###  https://semanticdatacharter.com/ns/sdc4/ItemType
sdc4:ItemType rdf:type owl:Class ;
              rdfs:subClassOf sdc4:CMC ;
              rdfs:comment "The abstract parent of ClusterType and XdAdapterType."@en-us .


###  https://semanticdatacharter.com/ns/sdc4/MSKType
sdc4:MSKType rdf:type owl:Class ;
             rdfs:subClassOf sdc4:ExceptionalValueType ;
             rdfs:comment "Masked : There is information on this item available but it has not been provided by the sender due to security, privacy or other reasons. There may be an alternate mechanism for gaining access to this information. Warning: Using this exceptional value does provide information that may be a breach of confidentiality, even though no detail data is provided. Its primary purpose is for those circumstances where it is necessary to inform the receiver that the information does exist without providing any detail." .


###  https://semanticdatacharter.com/ns/sdc4/MagnitudeStatus
sdc4:MagnitudeStatus rdf:type owl:Class ;
                     rdfs:subClassOf owl:Thing ;
                     rdfs:comment "MagnitudeStatus provides a general indication of the accuracy of the magnitude expressed in the XdQuantified subtypes. Should be used to inform users and not for decision support uses." .


###  https://semanticdatacharter.com/ns/sdc4/NASKType
sdc4:NASKType rdf:type owl:Class ;
              rdfs:subClassOf sdc4:ExceptionalValueType ;
              rdfs:comment "Not Asked : This information has not been sought (e.g., patient was not asked)" .


###  https://semanticdatacharter.com/ns/sdc4/NAType
sdc4:NAType rdf:type owl:Class ;
            rdfs:subClassOf sdc4:ExceptionalValueType ;
            rdfs:comment "Not Applicable : No proper value is applicable in this context e.g.,the number of cigarettes smoked per day by a non-smoker subject." .


###  https://semanticdatacharter.com/ns/sdc4/NAVType
sdc4:NAVType rdf:type owl:Class ;
             rdfs:subClassOf sdc4:ExceptionalValueType ;
             rdfs:comment "Not Available: This information is not available and the specific reason is not known." .


###  https://semanticdatacharter.com/ns/sdc4/NINFType
sdc4:NINFType rdf:type owl:Class ;
              rdfs:subClassOf sdc4:ExceptionalValueType ;
              rdfs:comment "Negative Infinity : Negative infinity of numbers" .


###  https://semanticdatacharter.com/ns/sdc4/NIType
sdc4:NIType rdf:type owl:Class ;
            rdfs:subClassOf sdc4:ExceptionalValueType ;
            rdfs:comment "No Information : The value is exceptional (missing, omitted, incomplete, improper). No information as to the reason for being an exceptional value is provided. This is the most general exceptional value. It is also the default exceptional value." .


###  https://semanticdatacharter.com/ns/sdc4/OTHType
sdc4:OTHType rdf:type owl:Class ;
             rdfs:subClassOf sdc4:ExceptionalValueType ;
             rdfs:comment "Other: The actual value is not a member of the permitted data values in the variable. (e.g., when the value of the variable is not by the coding system)" .


###  https://semanticdatacharter.com/ns/sdc4/PINFType
sdc4:PINFType rdf:type owl:Class ;
              rdfs:subClassOf sdc4:ExceptionalValueType ;
              rdfs:comment "Positive Infinity : Positive infinity of numbers" .


###  https://semanticdatacharter.com/ns/sdc4/ParticipationType
sdc4:ParticipationType rdf:type owl:Class ;
                       rdfs:subClassOf sdc4:CMC ;
                       rdfs:comment "Model of a participation of a Party (any Actor or Role) in an activity. Used to represent any participation of a Party in some activity, which is not explicitly in the model, e.g. assisting nurse. Can be used to record past or future participations." .


###  https://semanticdatacharter.com/ns/sdc4/PartyType
sdc4:PartyType rdf:type owl:Class ;
               rdfs:subClassOf sdc4:CMC ;
               rdfs:comment """Description of a party, including an optional external link to data for this party in a demographic or other identity management system. An additional details element provides for the inclusion of information related to this party directly. If the party
        information is to be anonymous then do not include the details element.""" .


###  https://semanticdatacharter.com/ns/sdc4/QSType
sdc4:QSType rdf:type owl:Class ;
            rdfs:subClassOf sdc4:ExceptionalValueType ;
            rdfs:comment "Sufficient Quantity : The specific quantity is not known, but is known to non-zero and it is not specified because it makes up the bulk of the material; Add 10mg of ingredient X, 50mg of ingredient Y and sufficient quantity of water to 100mL." .


###  https://semanticdatacharter.com/ns/sdc4/ReferenceRangeType
sdc4:ReferenceRangeType rdf:type owl:Class ;
                        rdfs:subClassOf sdc4:XdAnyType .


###  https://semanticdatacharter.com/ns/sdc4/TRCType
sdc4:TRCType rdf:type owl:Class ;
             rdfs:subClassOf sdc4:ExceptionalValueType ;
             rdfs:comment "Trace : The content is greater or less than zero but too small to be quantified." .


###  https://semanticdatacharter.com/ns/sdc4/UNCType
sdc4:UNCType rdf:type owl:Class ;
             rdfs:subClassOf sdc4:ExceptionalValueType ;
             rdfs:comment "Unencoded : No attempt has been made to encode the information correctly but the raw source information is represented, usually in free text." .


###  https://semanticdatacharter.com/ns/sdc4/UNKType
sdc4:UNKType rdf:type owl:Class ;
             rdfs:subClassOf sdc4:ExceptionalValueType ;
             rdfs:comment "Unknown : A proper value is applicable, but not known." .


###  https://semanticdatacharter.com/ns/sdc4/XdAdapterType
sdc4:XdAdapterType rdf:type owl:Class ;
                   rdfs:subClassOf sdc4:ItemType ;
                   rdfs:comment "A leaf node in a structure that holds a data-typed value."@en-us .


###  https://semanticdatacharter.com/ns/sdc4/XdAnyType
sdc4:XdAnyType rdf:type owl:Class ;
               rdfs:subClassOf sdc4:CMC ;
               rdfs:comment "Serves as the common ancestor of all eXtended data-types (Xd*) in the Semantic Data Charter. It is an abstract class and should not be instantiated directly."@en-us .


###  https://semanticdatacharter.com/ns/sdc4/XdBooleanListType
sdc4:XdBooleanListType rdf:type owl:Class ;
                       rdfs:subClassOf sdc4:XdAnyType ;
                       rdfs:comment """A data type for a white space-delimited list of boolean values. 
        This type provides efficient storage and transmission of multiple boolean values in a single field.
        Useful for scientific measurements, batch processing results, and other scenarios where multiple
        related boolean values need to be transmitted together.""" .


###  https://semanticdatacharter.com/ns/sdc4/XdBooleanType
sdc4:XdBooleanType rdf:type owl:Class ;
                   rdfs:subClassOf sdc4:XdAnyType ;
                   rdfs:comment """An enumerated type which represents boolean decisions. 
Such as true/false or yes/no answers. Useful where it is essential to devise the meanings (often questions in subjective data) carefully so that the only allowed result values result in one the options; true or false but are presented to the user as a list of options. 
The possible choices for True or False are enumerations in the DM. 
The reference model defines 'true-value' and 'false-value' in an xsd:choice so only one or the other may be present in the instance data. 
        
The XdBooleanType should not be used as a replacement for enumerated choice types such as male/female, or similar choice sets. Such values should be modeled as XdStrings with enumerations and may reference a controlled vocabulary. In any case, the choice set often has more than two values. 
        
The elements, 'true-value' and 'false-value' are contained in an xsd:choice and only one or the other is instantiated in the instance data with its value coming from the enumerations defined in a Data Model.""" .


###  https://semanticdatacharter.com/ns/sdc4/XdCountType
sdc4:XdCountType rdf:type owl:Class ;
                 rdfs:subClassOf sdc4:XdQuantifiedType ;
                 rdfs:comment "Countable quantities. Used for countable types such as pregnancies and steps (taken by a physiotherapy patient), number of cigarettes smoked in a day, etc. The thing(s) being counted must be represented in the units element. Misuse:Not used for amounts of physical entities (which all have standardized units)." .


###  https://semanticdatacharter.com/ns/sdc4/XdDecimalListType
sdc4:XdDecimalListType rdf:type owl:Class ;
                       rdfs:subClassOf sdc4:XdQuantifiedType ;
                       rdfs:comment """A data type for a white space-delimited list of decimal values. 
        This type provides efficient storage and transmission of multiple decimal values in a single field.
        Useful for scientific measurements, statistical data, and other scenarios where multiple related
        decimal values need to be transmitted together. All values in the list share the same units.""" .


###  https://semanticdatacharter.com/ns/sdc4/XdDoubleListType
sdc4:XdDoubleListType rdf:type owl:Class ;
                      rdfs:subClassOf sdc4:XdQuantifiedType ;
                      rdfs:comment """A data type for a white space-delimited list of double precision values. 
        This type provides efficient storage and transmission of multiple double values in a single field.
        Useful for scientific measurements, mathematical computations, and other scenarios where multiple
        related double precision values need to be transmitted together. All values in the list share the same units.""" .


###  https://semanticdatacharter.com/ns/sdc4/XdDoubleType
sdc4:XdDoubleType rdf:type owl:Class ;
                  rdfs:subClassOf sdc4:XdQuantifiedType ;
                  rdfs:comment "Quantified type representing specific a value as a 64 bit number and optional units. This is a xsd:double." .


###  https://semanticdatacharter.com/ns/sdc4/XdFileType
sdc4:XdFileType rdf:type owl:Class ;
                rdfs:subClassOf sdc4:XdAnyType ;
                rdfs:comment "A type to use for encapsulated content (aka. files) for image, audio and other media types with a defined MIME type. This type provides a choice of embedding the content into the data or using a URL to point to the content." .


###  https://semanticdatacharter.com/ns/sdc4/XdFloatType
sdc4:XdFloatType rdf:type owl:Class ;
                 rdfs:subClassOf sdc4:XdQuantifiedType ;
                 rdfs:comment "Quantified type representing specific a value as a floating point (32 bit) number and optional units. This is a xsd:float." .


###  https://semanticdatacharter.com/ns/sdc4/XdIntegerListType
sdc4:XdIntegerListType rdf:type owl:Class ;
                       rdfs:subClassOf sdc4:XdQuantifiedType ;
                       rdfs:comment """A data type for a white space-delimited list of integer values. 
        This type provides efficient storage and transmission of multiple integer values in a single field.
        Useful for counts, indices, and other scenarios where multiple related integer values need to be
        transmitted together. All values in the list share the same units.""" .


###  https://semanticdatacharter.com/ns/sdc4/XdIntervalType
sdc4:XdIntervalType rdf:type owl:Class ;
                    rdfs:subClassOf sdc4:XdAnyType ;
                    rdfs:comment "A generic type for defining an interval (i.e., range) of ordered values. It is primarily used to define reference ranges for quantified data." .


###  https://semanticdatacharter.com/ns/sdc4/XdLinkType
sdc4:XdLinkType rdf:type owl:Class ;
                rdfs:subClassOf sdc4:XdAnyType ;
                rdfs:comment "Used to specify a Universal Resource Identifier. Set the pattern facet to accommodate your needs in the DM. Intended use is to provide a mechanism that can be used to link together Data Models. The relation element allows for the use of a descriptive term for the link with an optional URI pointing to the source vocabulary. In most usecases the modeler will define all three of these using the 'fixed' attribute. Other usecases will have the 'relation' and 'relation-uri' elements fixed and the application will provide the 'link-value'." .


###  https://semanticdatacharter.com/ns/sdc4/XdNonNegativeIntegerListType
sdc4:XdNonNegativeIntegerListType rdf:type owl:Class ;
                                  rdfs:subClassOf sdc4:XdQuantifiedType ;
                                  rdfs:comment """A data type for a white space-delimited list of non-negative integer values. 
        This type provides efficient storage and transmission of multiple non-negative integer values in a single field.
        Useful for counts, indices, and other scenarios where multiple related non-negative integer values need to be
        transmitted together. All values in the list share the same units.""" .


###  https://semanticdatacharter.com/ns/sdc4/XdOrderedType
sdc4:XdOrderedType rdf:type owl:Class ;
                   rdfs:subClassOf sdc4:XdAnyType ;
                   rdfs:comment "Abstract type defining the concept of ordered values, which includes ordinals as well as true quantities. The implementations require the functions '&lt;', ''>' and is_strictly_comparable_to ('==')." .


###  https://semanticdatacharter.com/ns/sdc4/XdOrdinalType
sdc4:XdOrdinalType rdf:type owl:Class ;
                   rdfs:subClassOf sdc4:XdOrderedType ;
                   rdfs:comment """Models rankings and scores, e.g., pain, Apgar values, educational level, and the Likert Scale where there is;
        
        * implied ordering,
        * no implication that the distance between each value is constant, and
        * the total number of values is finite.
        
        Note that the term 'ordinal' in mathematics means natural numbers only. In this case, any decimal is allowed since negative, and zero values are used by medical and other professionals for centering values around a neutral point. Also, decimal values are sometimes used such as 0.5 or .25
        
        Examples of sets of ordinal values are;
        
        * -3, -2, -1, 0, 1, 2, 3 -- reflex response values
        * 0, 1, 2 -- Apgar values
        
        Also used for recording any clinical or other data which is customarily recorded using symbolic values. Examples;
        
        * the results on a urinalysis strip, e.g. {neg, trace, +, ++, +++} are used for leukocytes, protein, nitrites etc;
        * for non-haemolysed blood {neg, trace, moderate};
        * for haemolysed blood {neg, trace, small, moderate, large}.
        
        Elements *ordinal* and *symbol* MUST have the same number of enumerations in the RMC.""" .


###  https://semanticdatacharter.com/ns/sdc4/XdPositiveIntegerListType
sdc4:XdPositiveIntegerListType rdf:type owl:Class ;
                               rdfs:subClassOf sdc4:XdQuantifiedType ;
                               rdfs:comment """A data type for a white space-delimited list of positive integer values. 
        This type provides efficient storage and transmission of multiple positive integer values in a single field.
        Useful for counts, indices, and other scenarios where multiple related positive integer values need to be
        transmitted together. All values in the list share the same units.""" .


###  https://semanticdatacharter.com/ns/sdc4/XdQuantifiedType
sdc4:XdQuantifiedType rdf:type owl:Class ;
                      rdfs:subClassOf sdc4:XdOrderedType ;
                      rdfs:comment "Abstract type defining the concept of true quantified values, i.e. values which are not only ordered, but which have a precise magnitude." .


###  https://semanticdatacharter.com/ns/sdc4/XdQuantityType
sdc4:XdQuantityType rdf:type owl:Class ;
                    rdfs:subClassOf sdc4:XdQuantifiedType ;
                    rdfs:comment "Quantified type representing specific quantities, i.e. quantities expressed as a magnitude and units. Can also be used for time durations, where it is more convenient to treat these as simply a number of individual seconds, minutes, hours, days, months, years, etc. when no temporal calculation is to be performed." .


###  https://semanticdatacharter.com/ns/sdc4/XdStringListType
sdc4:XdStringListType rdf:type owl:Class ;
                      rdfs:subClassOf sdc4:XdAnyType ;
                      rdfs:comment """A data type for a white space-delimited list of string values. 
        This type provides efficient storage and transmission of multiple string values in a single field.
        Useful for identifiers, codes, and other scenarios where multiple related string values need to be
        transmitted together.""" .


###  https://semanticdatacharter.com/ns/sdc4/XdStringType
sdc4:XdStringType rdf:type owl:Class ;
                  rdfs:subClassOf sdc4:XdAnyType ;
                  rdfs:comment "The string data type can contain characters, line feeds, carriage returns, and tab characters. The use cases are for any free form text entry or for any enumerated lists. Additionally the minimum and maximum lengths may be set and regular expression patterns may be specified." .


###  https://semanticdatacharter.com/ns/sdc4/XdTemporalType
sdc4:XdTemporalType rdf:type owl:Class ;
                    rdfs:subClassOf sdc4:XdOrderedType ;
                    rdfs:comment """Type defining a temporal value. It allows for varying levels of precision by offering a choice of exactly one temporal representation, from a full dateTime to a partial date like a year-month.
In a Data Model, this type is constrained via restriction to a subset of the choices, allowing the modeler to define precisely which temporal representations are permitted for a given field (e.g., allowing only xsd:date or xsd:gYearMonth for a date of birth).""" .


###  https://semanticdatacharter.com/ns/sdc4/XdTokenListType
sdc4:XdTokenListType rdf:type owl:Class ;
                     rdfs:subClassOf sdc4:XdAnyType ;
                     rdfs:comment """A data type for a white space-delimited list of normalized token values. 
        This type provides efficient storage and transmission of multiple normalized token values in a single field.
        Useful for identifiers, codes, and other scenarios where multiple related normalized token values need to be
        transmitted together. Token values have leading and trailing whitespace removed and internal whitespace
        normalized to single spaces.""" .


###  https://semanticdatacharter.com/ns/sdc4/XdTokenType
sdc4:XdTokenType rdf:type owl:Class ;
                 rdfs:subClassOf sdc4:XdAnyType ;
                 rdfs:comment "The token data type represents normalized strings where leading and trailing whitespace is removed and internal whitespace is normalized to single spaces. This type is useful for identifiers, codes, and other normalized text values that should not contain excessive whitespace." .


#################################################################
#    Individuals
#################################################################

###  https://semanticdatacharter.com/ns/sdc4/approximate
sdc4:approximate rdf:type owl:NamedIndividual ,
                          sdc4:MagnitudeStatus ;
                 rdfs:comment "value is the approximately the magnitude" .


###  https://semanticdatacharter.com/ns/sdc4/equal
sdc4:equal rdf:type owl:NamedIndividual ,
                    sdc4:MagnitudeStatus ;
           rdfs:comment "magnitude is a point value" .


###  https://semanticdatacharter.com/ns/sdc4/greater_than
sdc4:greater_than rdf:type owl:NamedIndividual ,
                           sdc4:MagnitudeStatus ;
                  rdfs:comment "value is greater than the magnitude" .


###  https://semanticdatacharter.com/ns/sdc4/greater_than_or_equal
sdc4:greater_than_or_equal rdf:type owl:NamedIndividual ,
                                    sdc4:MagnitudeStatus ;
                           rdfs:comment "value is greater than or equal to the magnitude" .


###  https://semanticdatacharter.com/ns/sdc4/less_than
sdc4:less_than rdf:type owl:NamedIndividual ,
                        sdc4:MagnitudeStatus ;
               rdfs:comment "value is less than the magnitude" .


###  https://semanticdatacharter.com/ns/sdc4/less_than_or_equal
sdc4:less_than_or_equal rdf:type owl:NamedIndividual ,
                                 sdc4:MagnitudeStatus ;
                        rdfs:comment "value is less than or equal to the magnitude" .


###  Generated by the OWL API (version 4.5.29.2024-05-13T12:11:03Z) https://github.com/owlcs/owlapi
